Restructure files and update soundness theorems with sems

src/SmallStep.v
@@ -1,48 +1,59 @@
-From TLC Require Import LibLN.
-From MCore Require Import Syntax Typing Tactics.
+From TLC Require Import LibList LibLN.
+From MCore Require Import Syntax SyntaxProps Typing TypingProps.
 
 Module SmallStep (P : PAT).
-  Module T := Typing P.
-  Export T.
-
-  Inductive is_value : term -> Prop :=
-  | VLam   : forall ty t,
-      is_value (TmLam ty t)
-  | VTyLam : forall k t,
-      is_value (TmTyLam k t)
-  | VProd : forall v1 v2,
-      is_value v1 ->
-      is_value v2 ->
-      is_value (TmProd v1 v2)
-  | VCon : forall K ty v,
-      is_value v ->
-      is_value (TmCon K ty v)
-  | VSem : forall ty p t,
-      is_value (TmSem ty p t)
-  | VComp : forall v1 v2,
-      is_value v1 ->
-      is_value v2 ->
-      is_value (TmComp v1 v2).
-  #[export]
-   Hint Constructors is_value : mcore.
-
-  Fixpoint push_value (f : term -> term) (t : term) : term :=
-    match t with
-    | TmLam ty t' => TmLam ty (f t')
-    | TmTyLam k t' => TmTyLam k (f t')
-    | TmProd t1 t2 => TmProd (f t1) (f t2)
-    | TmCon K ty t' => TmCon K ty (f t')
-    | TmSem ty p t' => TmSem ty p (f t')
-    | TmComp t1 t2 => TmComp (f t1) (f t2)
-    | _ => arbitrary
-    end.
+  Module TP := TypingProps P.
+  Export TP.
 
   Module Type MATCH.
     Parameter match1 : term -> pat -> option term.
+    Parameter matchN : term -> list pat -> option (term * nat).
   End MATCH.
 
-  Module SmallStep (M : MATCH).
+  Module SmallStep1 (M : MATCH).
     Export M.
+
+    Inductive is_value : term -> Prop :=
+    | VLam   : forall ty t,
+        is_value (TmLam ty t)
+    | VTyLam : forall k t,
+        is_value (TmTyLam k t)
+    | VProd : forall v1 v2,
+        is_value v1 ->
+        is_value v2 ->
+        is_value (TmProd v1 v2)
+    | VCon : forall K ty v,
+        is_value v ->
+        is_value (TmCon K ty v)
+    | VSem : forall ty p t,
+        is_value (TmSem ty p t)
+    | VComp : forall v1 v2,
+        is_value v1 ->
+        is_value v2 ->
+        is_value (TmComp v1 v2).
+    #[export]
+     Hint Constructors is_value : mcore.
+
+    Fixpoint push_value (f : term -> term) (t : term) : term :=
+      match t with
+      | TmLam ty t' => TmLam ty (f t')
+      | TmTyLam k t' => TmTyLam k (f t')
+      | TmProd t1 t2 => TmProd (push_value f t1) (push_value f t2)
+      | TmCon K ty t' => TmCon K ty (push_value f t')
+      | TmSem ty p t' => TmSem ty p (f t')
+      | TmComp t1 t2 => TmComp (push_value f t1) (push_value f t2)
+      | _ => arbitrary
+      end.
+
+    Fixpoint get_cases (t : term) :=
+      match t with
+      | TmSem ty p t' => (p :: nil , t' :: nil)
+      | TmComp t1 t2  =>
+          let (ps1 , ts1) := get_cases t1 in
+          let (ps2 , ts2) := get_cases t2 in
+          (ps1 ++ ps2, ts1 ++ ts2)
+      | _ => (nil, nil)
+      end.
 
     Inductive is_context : (term -> term) -> Prop :=
     | CAppL : forall t', is_context (fun t => TmApp t t')
@@ -67,7 +78,7 @@ Module SmallStep (P : PAT).
         is_value v ->
         is_context (TmSemApp v).
     #[export]
-    Hint Constructors is_context : mcore.
+     Hint Constructors is_context : mcore.
 
     Reserved Notation "t1 --> t2" (at level 50).
     Inductive eval_step : term -> term -> Prop :=
@@ -112,21 +123,20 @@ Module SmallStep (P : PAT).
     (* | EComp : forall {cases1 cases2 : list (pat * term)} {ty : type}, *)
     (*     eval_step (TmComp (TmSem ty cases1) (TmSem ty cases2)) *)
     (*               (TmSem ty (cases1 ++ cases2)) *)
-    (* | ESemApp : forall {v : term} {ty : type} *)
-    (*                    {cases : list (pat * term)} *)
-    (*                    {i : nat} {theta : list term} *)
-    (*                    (vval : is_value v), *)
-    (*     match_n vval (map fst cases) = Some (i, theta) -> *)
-    (*     eval_step (TmSemApp (TmSem ty cases) v) *)
-    (*               (tm_subst_n (nth i (map snd cases)) theta) *)
+    | ESemApp : forall v1 v2 v2' i ps bs,
+        is_value v1 ->
+        is_value v2 ->
+        get_cases v1 = (ps , bs) ->
+        matchN v2 ps = Some (v2', i) ->
+        TmSemApp v1 v2 --> [0 ~> v2'](nth i bs)
     | ECong : forall {f},
         is_context f ->
         forall t1 t2,
-            t1 --> t2   ->
+          t1 --> t2   ->
           f t1 --> f t2
     where "t1 --> t2" := (eval_step t1 t2).
     #[export]
-    Hint Constructors eval_step : mcore.
+     Hint Constructors eval_step : mcore.
 
     Definition econg_CAppL t2 := ECong (CAppL t2).
     #[export] Hint Resolve econg_CAppL : mcore.
@@ -149,134 +159,5 @@ Module SmallStep (P : PAT).
     Definition econg_CSemAppR v Hv := ECong (CSemAppR v Hv).
     #[export] Hint Resolve econg_CSemAppR : mcore.
 
-    Lemma Topen_is_value :
-      forall i T v,
-        is_value (Topen_t i T v) ->
-        is_value v.
-    Proof.
-      introv Hval.
-      induction v ; inverts* Hval.
-    Qed.
-
-    Lemma is_value_Tsubst :
-      forall X T v,
-        is_value v ->
-        is_value (Tsubst_t X T v).
-    Proof.
-      introv Hval.
-      induction v ; inverts* Hval.
-    Qed.
-
-    Lemma push_Tsubst :
-      forall f f' X T t1 t2,
-        (forall t, Tsubst_t X T (f t) = f' (Tsubst_t X T t)) ->
-        is_value t1 ->
-        push_value f t1 = t2 ->
-        push_value f' (Tsubst_t X T t1) = Tsubst_t X T t2.
-    Proof.
-      introv Heq Hval Hpush. gen t2.
-      induction Hval ; intros ; destruct t2 ; inverts Hpush ;
-        simpls ; rewrite_all~ Heq.
-    Qed.
-
-    Lemma step_Tsubst :
-      forall X T t1 t2,
-        t1 --> t2 ->
-        Tsubst_t X (FTName T) t1 --> Tsubst_t X (FTName T) t2.
-    Proof.
-      introv Hstep.
-      induction Hstep ; simpls.
-      - rewrite Tsubst_t_open_distr.
-        forwards* Hval: is_value_Tsubst H.
-      - rewrite* Tsubst_t_topen_distr.
-      - rewrite Tsubst_t_open_distr. simpls*.
-      - forwards Hval: is_value_Tsubst H.
-        forwards* Hval': is_value_Tsubst H0.
-      - forwards Hval: is_value_Tsubst H.
-        forwards* Hval': is_value_Tsubst H0.
-      - forwards Hval: is_value_Tsubst H.
-        forwards* Hpush: push_Tsubst TmType H. rewrite* <- Hpush.
-      - forwards Hval: is_value_Tsubst H.
-        forwards* Hpush: push_Tsubst (TmConDef d ty T0) H. rewrite* <- Hpush.
-      - apply_fresh ETypeCong. rewrite_all~ Tsubst_t_Topen_comm.
-      - apply_fresh EConDefCong. rewrite_all~ Tsubst_t_Kopen_comm.
-      - inverts H ; simpls* ; forwards* Hval: is_value_Tsubst H0.
-    Qed.
-
-    Lemma Topen_step_change :
-      forall i T U t1 t2,
-        T \notin Tfv_t t1 \u Tfv_t t2 ->
-        Topen_t i (FTName T) t1 --> Topen_t i (FTName T) t2 ->
-        Topen_t i (FTName U) t1 --> Topen_t i (FTName U) t2.
-    Proof.
-      introv Hfresh. rewrite_all~ (Tsubst_t_intro T (FTName U)).
-      apply step_Tsubst.
-    Qed.
-
-
-    Lemma Kopen_is_value :
-      forall i K v,
-        is_value (Kopen_t i K v) ->
-        is_value v.
-    Proof.
-      introv Hval.
-      induction v ; inverts* Hval.
-    Qed.
-
-    Lemma is_value_Ksubst :
-      forall X K v,
-        is_value v ->
-        is_value (Ksubst_t X K v).
-    Proof.
-      introv Hval.
-      induction v ; inverts* Hval.
-    Qed.
-
-    Lemma push_Ksubst :
-      forall f f' X T t1 t2,
-        (forall t, Ksubst_t X T (f t) = f' (Ksubst_t X T t)) ->
-        is_value t1 ->
-        push_value f t1 = t2 ->
-        push_value f' (Ksubst_t X T t1) = Ksubst_t X T t2.
-    Proof.
-      introv Heq Hval Hpush. gen t2.
-      induction Hval ; intros ; destruct t2 ; inverts Hpush ;
-        simpls ; rewrite_all~ Heq.
-    Qed.
-
-    Lemma step_Ksubst :
-      forall X K t1 t2,
-        t1 --> t2 ->
-        Ksubst_t X (FCon K) t1 --> Ksubst_t X (FCon K) t2.
-    Proof.
-      introv Hstep.
-      induction Hstep ; simpls.
-      - rewrite Ksubst_t_open_distr.
-        forwards* Hval: is_value_Ksubst H.
-      - rewrite* Ksubst_t_topen_distr.
-      - rewrite Ksubst_t_open_distr. simpls*.
-      - forwards Hval: is_value_Ksubst H.
-        forwards* Hval': is_value_Ksubst H0.
-      - forwards Hval: is_value_Ksubst H.
-        forwards* Hval': is_value_Ksubst H0.
-      - forwards Hval: is_value_Ksubst H.
-        forwards* Hpush: push_Ksubst TmType H. rewrite* <- Hpush.
-      - forwards Hval: is_value_Ksubst H.
-        forwards* Hpush: push_Ksubst (TmConDef d ty T) H. rewrite* <- Hpush.
-      - apply_fresh ETypeCong. rewrite_all~ Ksubst_t_Topen_comm.
-      - apply_fresh EConDefCong. rewrite_all~ Ksubst_t_Kopen_comm.
-      - inverts H ; simpls* ; forwards* Hval: is_value_Ksubst H0.
-    Qed.
-
-    Lemma Kopen_step_change :
-      forall i K U t1 t2,
-        K \notin Kfv_t t1 \u Kfv_t t2 ->
-        Kopen_t i (FCon K) t1 --> Kopen_t i (FCon K) t2 ->
-        Kopen_t i (FCon U) t1 --> Kopen_t i (FCon U) t2.
-    Proof.
-      introv Hfresh. rewrite_all~ (Ksubst_t_intro K (FCon U)).
-      apply step_Ksubst.
-    Qed.
-
-  End SmallStep.
+  End SmallStep1.
 End SmallStep.
