src/SmallStepProps.v
@@ -1,0 +1,387 @@
+From TLC Require Import LibString LibNat LibList LibLN.
+From MCore Require Import
+     Syntax SyntaxProps Typing TypingProps
+     SmallStep Tactics.
+Import LibListNotation.
+
+Module SmallStepProps (P : PAT).
+  Module S := SmallStep P.
+  Export S.
+
+  Module SmallStepProps1 (PC : PATCHECK) (M : MATCH).
+    Module TP1 := TypingProps1 PC.
+    Module S1 := SmallStep1 M.
+    Export TP1 S1.
+
+    Module Type MATCHPROPS.
+      Parameter matchN_length :
+        forall t ps t' i,
+          matchN t ps = Some (t', i) -> i < length ps.
+
+      Parameter matchN_Tsubst :
+        forall t ps t' i X T,
+          matchN t ps = Some (t', i) ->
+          matchN (Tsubst_t X T t) ps = Some (Tsubst_t X T t', i).
+
+      Parameter matchN_Ksubst :
+        forall t ps t' i X T,
+          matchN t ps = Some (t', i) ->
+          matchN (Ksubst_t X T t) ps = Some (Ksubst_t X T t', i).
+
+      Parameter matchN_ok_pat :
+        forall Gamma ps v v' ty ty' i,
+          matchN v ps = Some (v', i) ->
+          ok_pat Gamma (nth i ps) ty ty' ->
+          Gamma |= v' ~: ty'.
+
+      Parameter exhaustive_has_match :
+        forall Gamma ty ps v,
+          Gamma |= v ~: ty ->
+          pats_exhaustive ps ty ->
+          is_value v ->
+          exists i v',
+            matchN v ps = Some (v', i).
+    End MATCHPROPS.
+
+    Module SmallStepProps2 (PCP : PATCHECKPROPS) (MP : MATCHPROPS).
+      Module TP2 := TypingProps2 PCP.
+      Export MP TP2.
+
+      Lemma get_cases_length :
+        forall ps bs t,
+          get_cases t = (ps, bs) ->
+          length ps = length bs.
+      Proof.
+        introv Heq. gen ps bs.
+        induction t ; intros ; inverts~ Heq.
+        destruct (get_cases t1). destruct (get_cases t2).
+        inverts H0. rew_listx. fequals~.
+      Qed.
+
+      Lemma get_cases_Tsubst :
+        forall ps bs X T t,
+          get_cases t = (ps, bs) ->
+          get_cases (Tsubst_t X T t) = (ps, LibList.map (Tsubst_t X T) bs).
+      Proof.
+        introv Heq. gen ps bs.
+        induction t ; intros ; simpls ; inverts~ Heq.
+        destruct (get_cases t1). destruct (get_cases t2).
+        destruct (get_cases (Tsubst_t X T t1)). destruct (get_cases (Tsubst_t X T t2)).
+        inverts H0. rew_listx. forwards~ Heq1 : IHt1. forwards~ Heq2 : IHt2.
+        fequals.
+      Qed.
+
+      Lemma Topen_is_value :
+        forall i T v,
+          is_value (Topen_t i T v) ->
+          is_value v.
+      Proof.
+        introv Hval.
+        induction v ; inverts* Hval.
+      Qed.
+
+      Lemma is_value_Tsubst :
+        forall X T v,
+          is_value v ->
+          is_value (Tsubst_t X T v).
+      Proof.
+        introv Hval.
+        induction v ; inverts* Hval.
+      Qed.
+
+      Lemma push_Tsubst :
+        forall f f' X T t1 t2,
+          (forall t, Tsubst_t X T (f t) = f' (Tsubst_t X T t)) ->
+          is_value t1 ->
+          push_value f t1 = t2 ->
+          push_value f' (Tsubst_t X T t1) = Tsubst_t X T t2.
+      Proof.
+        introv Heq Hval Hpush. gen t2.
+        induction Hval ; intros ; destruct t2 ; inverts Hpush ;
+          simpls ; try rewrite~ Heq.
+        - erewrite~ IHHval1. erewrite~ IHHval2.
+        - erewrite~ IHHval.
+        - erewrite~ IHHval1. erewrite~ IHHval2.
+      Qed.
+
+      Lemma step_Tsubst :
+        forall X T t1 t2,
+          t1 --> t2 ->
+          Tsubst_t X (FTName T) t1 --> Tsubst_t X (FTName T) t2.
+      Proof.
+        introv Hstep.
+        induction Hstep ; simpls.
+        - rewrite Tsubst_t_open_distr.
+          forwards* Hval: is_value_Tsubst H.
+        - rewrite* Tsubst_t_topen_distr.
+        - rewrite Tsubst_t_open_distr. simpls*.
+        - forwards Hval: is_value_Tsubst H. forwards* Hval': is_value_Tsubst H0.
+        - forwards Hval: is_value_Tsubst H. forwards* Hval': is_value_Tsubst H0.
+        - forwards Hval: is_value_Tsubst H.
+          forwards* Hpush: push_Tsubst TmType H. rewrite* <- Hpush.
+        - forwards Hval: is_value_Tsubst H.
+          forwards* Hpush: push_Tsubst (TmConDef d ty T0) H. rewrite* <- Hpush.
+        - apply_fresh ETypeCong. rewrite_all~ Tsubst_t_Topen_comm.
+        - apply_fresh EConDefCong. rewrite_all~ Tsubst_t_Kopen_comm.
+        - forwards Hval: is_value_Tsubst H. forwards Hval': is_value_Tsubst H0.
+          rewrite Tsubst_t_open_distr. rewrite <- nth_map.
+          constructors*.
+          + apply* get_cases_Tsubst.
+          + apply* matchN_Tsubst.
+          + rewrite~ lt_peano. rewrite~ <- (get_cases_length ps bs v1).
+            apply* matchN_length.
+        - inverts H ; simpls* ; forwards* Hval: is_value_Tsubst H0.
+      Qed.
+
+      Lemma Topen_step_change :
+        forall i T U t1 t2,
+          T \notin Tfv_t t1 \u Tfv_t t2 ->
+          Topen_t i (FTName T) t1 --> Topen_t i (FTName T) t2 ->
+          Topen_t i (FTName U) t1 --> Topen_t i (FTName U) t2.
+      Proof.
+        introv Hfresh. rewrite_all~ (Tsubst_t_intro T (FTName U)).
+        apply step_Tsubst.
+      Qed.
+
+
+      Lemma get_cases_Ksubst :
+        forall ps bs X K t,
+          get_cases t = (ps, bs) ->
+          get_cases (Ksubst_t X K t) = (ps, LibList.map (Ksubst_t X K) bs).
+      Proof.
+        introv Heq. gen ps bs.
+        induction t ; intros ; simpls ; inverts~ Heq.
+        destruct (get_cases t1). destruct (get_cases t2).
+        destruct (get_cases (Ksubst_t X K t1)). destruct (get_cases (Ksubst_t X K t2)).
+        inverts H0. rew_listx. forwards~ Heq1 : IHt1. forwards~ Heq2 : IHt2.
+        fequals.
+      Qed.
+
+      Lemma Kopen_is_value :
+        forall i K v,
+          is_value (Kopen_t i K v) ->
+          is_value v.
+      Proof.
+        introv Hval.
+        induction v ; inverts* Hval.
+      Qed.
+
+      Lemma is_value_Ksubst :
+        forall X K v,
+          is_value v ->
+          is_value (Ksubst_t X K v).
+      Proof.
+        introv Hval.
+        induction v ; inverts* Hval.
+      Qed.
+
+      Lemma push_Ksubst :
+        forall f f' X T t1 t2,
+          (forall t, Ksubst_t X T (f t) = f' (Ksubst_t X T t)) ->
+          is_value t1 ->
+          push_value f t1 = t2 ->
+          push_value f' (Ksubst_t X T t1) = Ksubst_t X T t2.
+      Proof.
+        introv Heq Hval Hpush. gen t2.
+        induction Hval ; intros ; destruct t2 ; inverts Hpush ;
+          simpls ; try rewrite~ Heq.
+        - erewrite~ IHHval1. erewrite~ IHHval2.
+        - erewrite~ IHHval.
+        - erewrite~ IHHval1. erewrite~ IHHval2.
+      Qed.
+
+      Lemma step_Ksubst :
+        forall X K t1 t2,
+          t1 --> t2 ->
+          Ksubst_t X (FCon K) t1 --> Ksubst_t X (FCon K) t2.
+      Proof.
+        introv Hstep.
+        induction Hstep ; simpls.
+        - rewrite Ksubst_t_open_distr.
+          forwards* Hval: is_value_Ksubst H.
+        - rewrite* Ksubst_t_topen_distr.
+        - rewrite Ksubst_t_open_distr. simpls*.
+        - forwards Hval: is_value_Ksubst H. forwards* Hval': is_value_Ksubst H0.
+        - forwards Hval: is_value_Ksubst H. forwards* Hval': is_value_Ksubst H0.
+        - forwards Hval: is_value_Ksubst H.
+          forwards* Hpush: push_Ksubst TmType H. rewrite* <- Hpush.
+        - forwards Hval: is_value_Ksubst H.
+          forwards* Hpush: push_Ksubst (TmConDef d ty T) H. rewrite* <- Hpush.
+        - apply_fresh ETypeCong. rewrite_all~ Ksubst_t_Topen_comm.
+        - apply_fresh EConDefCong. rewrite_all~ Ksubst_t_Kopen_comm.
+        - forwards Hval: is_value_Ksubst H. forwards Hval': is_value_Ksubst H0.
+          rewrite Ksubst_t_open_distr. rewrite <- nth_map.
+          constructors*.
+          + apply* get_cases_Ksubst.
+          + apply* matchN_Ksubst.
+          + rewrite~ lt_peano. rewrite~ <- (get_cases_length ps bs v1).
+            apply* matchN_length.
+        - inverts H ; simpls* ; forwards* Hval: is_value_Ksubst H0.
+      Qed.
+
+      Lemma Kopen_step_change :
+        forall i K U t1 t2,
+          K \notin Kfv_t t1 \u Kfv_t t2 ->
+          Kopen_t i (FCon K) t1 --> Kopen_t i (FCon K) t2 ->
+          Kopen_t i (FCon U) t1 --> Kopen_t i (FCon U) t2.
+      Proof.
+        introv Hfresh. rewrite_all~ (Ksubst_t_intro K (FCon U)).
+        apply step_Ksubst.
+      Qed.
+
+      Lemma ok_term_get_cases_eq :
+        forall Gamma ty1 ty2 ps ps' bs v,
+          Gamma |= v ~: TySem ty1 ty2 ps ->
+          is_value v ->
+          get_cases v = (ps', bs) ->
+          ps' = ps.
+      Admitted.
+
+      Lemma ok_term_get_cases_inv :
+        forall Gamma ty1 ty2 ps ps' bs v i,
+          Gamma |= v ~: TySem ty1 ty2 ps ->
+          is_value v ->
+          get_cases v = (ps', bs) ->
+          i < length ps' ->
+          exists L ty1',
+            ok_pat Gamma (nth i ps') ty1 ty1' /\
+              (forall x, x \notin L ->
+                    Gamma & x ~ BindVar ty1' |= [0 ~> TmFVar x] nth i bs ~: ty2).
+      Admitted.
+
+      Lemma ok_term_Topen_push :
+        forall T Gamma t ty,
+          is_value t ->
+          T \notin dom Gamma \u Tfv_t t \u Tfv_ty ty ->
+          Gamma & T ~ BindTName |= Topen_t 0 (FTName T) t ~: ty ->
+          Gamma |= push_value TmType t ~: ty.
+      Proof with eauto with mcore.
+        introv Hval Hfresh Htype. gen ty.
+        induction Hval ; intros ; inverts Htype ; simpls.
+        { Case "TmLam". rewrite notin_Topen_ty in *...
+          assert (Gamma |= ty ~:: KiType)
+            by (apply_empty~ (ok_type_tname_strengthening T) ; apply* ok_env_push).
+          apply_fresh* TLam as x. apply_fresh TType as T'...
+          applys~ ok_term_Topen_change T.
+          - rewrite notin_union. rewrite~ open_notin_T.
+          - rewrite* Topen_t_open_comm. apply_empty ok_term_comm... }
+        { Case "TmTyLam". rewrite notin_Topen_k in *...
+          assert (ok_kind Gamma k) by apply_empty~ (ok_kind_tname_strengthening T).
+          apply_fresh* TTyLam as X. apply_fresh TType as T'...
+          applys~ ok_term_Topen_change T.
+          - rewrite notin_union. rewrite topen_t_notin_T. rewrite topen_notin_T ; simpls~.
+          - rewrite* Topen_t_topen_comm. apply_empty~ ok_term_comm.
+            constructor~. constructor~. apply* ok_env_push. }
+        { Case "TmProd". constructor~. }
+        { Case "TmCon". rewrite notin_Topen_ty in *...
+          constructors.
+          + binds_cases H2...
+          + apply_empty (ok_type_tname_strengthening T) ; auto ; apply* ok_env_push.
+          + apply_empty (ok_type_tname_strengthening T) ; auto ; apply* ok_env_push.
+          + apply~ IHHval. assert (T \notin Tfv_ty ({0 ~> ty} ty1))...
+            rewrite~ topen_notin_T. binds_cases H2.
+            forwards (L'&?&?&?&Htk&?): ok_env_binds_con_inv B. apply* ok_env_push.
+            pick_fresh X. forwards~ Hnin: ok_type_notin_T T (Htk X).
+            rewrite topen_notin_T in Hnin ; simpls~. }
+        { Case "TmSem". rewrite notin_Topen_ty in *...
+          assert (Gamma |= ty ~:: KiType)
+            by (apply_empty~ (ok_type_tname_strengthening T) ; apply* ok_env_push).
+          apply_fresh* TSem as x.
+          - apply_empty* (ok_pat_tname_strengthening T).
+          - apply_fresh TType as T'... applys~ ok_term_Topen_change T.
+            + rewrite notin_union. rewrite~ open_notin_T.
+            + rewrite* Topen_t_open_comm. apply_empty~ ok_term_comm.
+              constructor~. constructor~. apply* ok_env_push.
+              applys ok_pat_ok_type.
+              apply_empty* (ok_pat_tname_strengthening T) ; auto. }
+        { Case "TmComp". constructor~. apply IHHval1 ; simpls~. apply IHHval2 ; simpls~. }
+      Qed.
+
+      Lemma ok_term_Kopen_push :
+        forall K Gamma d ty' T t ty,
+          is_value t ->
+          K \notin dom Gamma \u Kfv_t t \u Kfv_ty ty ->
+          Gamma & K ~ BindCon d ty' T |= Kopen_t 0 (FCon K) t ~: ty ->
+          Gamma |= push_value (TmConDef d ty' T) t ~: ty.
+      Proof with eauto with mcore.
+        introv Hval Hfresh Htype. gen ty.
+        induction Hval ; intros ;
+          forwards Henv : ok_term_ok_env Htype ;
+          forwards (L0 & T' & Heq & Hd & Htk & HT): ok_env_con_inv Henv ;
+          inverts Htype ; substs ; simpls.
+        { Case "TmLam". rewrite notin_Kopen_ty in *...
+          assert (Gamma |= ty ~:: KiType)
+            by (apply_empty~ (ok_type_con_strengthening K) ; eauto ; apply* ok_env_push).
+          assert (Hty' : forall x X,
+                     X \notin L0 \u dom Gamma \u \{x} ->
+                     x # Gamma ->
+                     Gamma & x ~ BindVar ty & X ~ BindTVar (KiData d) |= {0 ~> TyFVar X} ty' ~:: KiType).
+          { introv Hnin Hfr. forwards~ Htk' : Htk X. apply~ ok_type_weakening.
+            constructor*. constructor~. apply_empty~ ok_data_weakening. constructor*. }
+          apply_fresh* TLam as x. apply_fresh TConDef as K'...
+          - apply_empty ok_data_weakening...
+          - applys~ ok_term_Kopen_change K.
+            + rewrite notin_union. rewrite~ open_notin_K.
+            + rewrite* Kopen_t_open_comm. apply_empty~ ok_term_comm.
+              apply_fresh EnvCon as X... apply_empty~ ok_data_weakening. constructor... }
+        { Case "TmTyLam". rewrite notin_Kopen_k in *...
+          assert (ok_kind Gamma k) by apply_empty* (ok_kind_con_strengthening K).
+          assert (Heq' : forall x, {1 ~> TyFVar x}ty' = ty').
+          { intros. pick_fresh y. apply topen_neq with (J := 0) (V := TyFVar y)...
+            rewrite~ topen_lct. apply* ok_type_lct. }
+          assert (Hty' : forall x X,
+                     X \notin L0 \u dom Gamma \u \{x} ->
+                     x # Gamma ->
+                     Gamma & x ~ BindTVar k & X ~ BindTVar (KiData d) |= {0 ~> TyFVar X} ty' ~:: KiType).
+          { introv Hnin Hfr. forwards~ Htk' : Htk X. apply~ ok_type_weakening.
+            constructor*. constructor~. apply_empty~ ok_data_weakening. constructor*. }
+          apply_fresh* TTyLam as X. apply_fresh TConDef as K'...
+          - apply_empty ok_data_weakening...
+          - rewrite~ Heq'.
+          - rewrite Heq'. applys~ ok_term_Kopen_change K.
+            + rewrite notin_union. rewrite topen_t_notin_K. rewrite topen_notin_K ; simpls~.
+            + rewrite* Kopen_t_topen_comm. apply_empty~ ok_term_comm.
+              apply_fresh EnvCon as X... apply_empty~ ok_data_weakening. constructor... }
+        { Case "TmProd". constructor~. }
+        { Case "TmCon". rewrite notin_Kopen_ty in *...
+          assert (Htk1 : Gamma |= ty ~:: KiData [ (FTName T0, FCon K1 :: []) ]).
+          { apply_empty* (ok_type_con_strengthening K). }
+          assert (Hneq : K1 <> K).
+          { intro ; subst. forwards~ Hk : ok_type_ok_kind Htk1.
+            inverts Hk as Hd'. inverts Hd'. inverts H11.
+            assert (K \indom Gamma) by applys get_some_inv H14.
+            assert (K # Gamma) by apply* ok_push_inv... }
+          replaces K0 with (FCon K1). { destruct K0 ; solve_var. }
+          constructors~.
+          + binds_cases H2...
+          + apply_empty (ok_type_con_strengthening K) ; eauto ; apply* ok_env_push.
+          + apply~ IHHval. assert (K \notin Kfv_ty ({0 ~> ty} ty1))...
+            rewrite~ topen_notin_K. binds_cases H2.
+            forwards (L'&?&?&?&Htk'&?): ok_env_binds_con_inv B. apply* ok_env_push.
+            pick_fresh X. forwards~ Hnin': ok_type_notin_K K (Htk' X).
+            rewrite~ topen_notin_K in Hnin'. simpls~. }
+        { Case "TmSem". rewrite notin_Kopen_ty in *...
+          assert (Gamma |= ty ~:: KiType)
+            by (apply_empty~ (ok_type_con_strengthening K) ; eauto ; apply* ok_env_push).
+          assert (Gamma |= ty1' ~:: KiType)
+            by (applys ok_pat_ok_type ; apply_empty* (ok_pat_con_strengthening K) ; auto).
+          assert (Hty' : forall x X,
+                     X \notin L0 \u dom Gamma \u \{x} ->
+                     x # Gamma ->
+                     Gamma & x ~ BindVar ty1' & X ~ BindTVar (KiData d) |= {0 ~> TyFVar X} ty' ~:: KiType).
+          { introv Hnin Hfr. forwards~ Htk' : Htk X. apply~ ok_type_weakening.
+            constructor*. constructor~. apply_empty~ ok_data_weakening. constructor*. }
+          apply_fresh* TSem as x.
+          - apply_empty* (ok_pat_con_strengthening K).
+          - apply_fresh TConDef as T'...
+            + apply_empty~ ok_data_weakening. constructor~. apply* ok_env_concat.
+            + applys~ ok_term_Kopen_change K.
+              * rewrite notin_union. rewrite~ open_notin_K.
+              * rewrite* Kopen_t_open_comm. apply_empty~ ok_term_comm.
+                constructors... apply_empty~ ok_data_weakening. constructor~. apply* ok_env_concat. }
+        { Case "TmComp". constructor~. apply IHHval1 ; simpls~. apply IHHval2 ; simpls~. }
+      Qed.
+
+    End SmallStepProps2.
+  End SmallStepProps1.
+End SmallStepProps.
