src/Soundness.v
@@ -1,204 +1,116 @@
 From TLC Require Import LibString LibList LibLN.
-From MCore Require Import Syntax Typing SmallStep Tactics.
-Import LibListNotation.
+From MCore Require Import
+     Syntax SyntaxProps Typing TypingProps
+     SmallStep SmallStepProps Tactics.
 
 Module Soundness (P : PAT).
-  Module S := SmallStep P.
-  Import S.
+  Module SP := SmallStepProps P.
+  Import SP.
 
-  Module Soundness (PC : PATCHECK) (M : MATCH).
-    Module Typing := Typing PC.
-    Module SmallStep := SmallStep M.
-    Import Typing SmallStep.
+  Module Soundness1 (PC : PATCHECK) (M : MATCH).
+    Module SP1 := SmallStepProps1 PC M.
+    Import SP1.
 
-    Lemma ok_term_Topen_push :
-      forall T Gamma t ty,
-        is_value t ->
-        T \notin dom Gamma \u Tfv_t t \u Tfv_ty ty ->
-        Gamma & T ~ BindTName |= Topen_t 0 (FTName T) t ~: ty ->
-        Gamma |= push_value TmType t ~: ty.
-    Proof with eauto with mcore.
-      introv Hval Hfresh Htype. destruct Hval ; inverts Htype ; simpls.
-      { Case "TmLam". rewrite notin_Topen_ty in *...
-        assert (Gamma |= ty0 ~:: KiType)
-          by (apply_empty~ (ok_type_tname_strengthening T) ; apply* ok_env_push).
-        apply_fresh* TLam as x.
-        forwards~ Htype': H4 x. apply_fresh TType as T'...
-        applys~ ok_term_Topen_change T.
-        - rewrite notin_union. rewrite~ open_notin_T.
-        - rewrite* Topen_t_open_comm. apply_empty* ok_term_comm. }
-      { Case "TmTyLam". rewrite notin_Topen_k in *...
-        assert (ok_kind Gamma k) by apply_empty~ (ok_kind_tname_strengthening T).
-        apply_fresh* TTyLam as X.
-        forwards~ Htype': H4 X. apply_fresh TType as T'...
-        applys~ ok_term_Topen_change T.
-        - rewrite notin_union. rewrite topen_t_notin_T. rewrite topen_notin_T ; simpls~.
-        - rewrite* Topen_t_topen_comm. apply_empty~ ok_term_comm.
-          constructor~. constructor~. apply* ok_env_push. }
-      { Case "TmProd".
-        constructor ; apply_fresh TType as T' ; applys~ ok_term_Topen_change T. }
-      { Case "TmCon". rewrite notin_Topen_ty in *...
-        constructors.
-        + binds_cases H2...
-        + apply_empty (ok_type_tname_strengthening T) ; auto ; apply* ok_env_push.
-        + apply_empty (ok_type_tname_strengthening T) ; auto ; apply* ok_env_push.
-        + apply_fresh TType as T'. applys~ ok_term_Topen_change T.
-          assert (T \notin Tfv_ty ({0 ~> ty0} ty1))...
-          rewrite~ topen_notin_T. binds_cases H2.
-          forwards (L'&?&?&?&Htk&?): ok_env_binds_con_inv B. apply* ok_env_push.
-          pick_fresh X. forwards~ Hnin: ok_type_notin_T T (Htk X).
-          rewrite topen_notin_T in Hnin ; simpls~. }
-    Qed.
+    Module Soundness2 (PCP : PATCHECKPROPS) (MP : MATCHPROPS).
+      Module SP2 := SmallStepProps2 PCP MP.
+      Import SP2.
 
-    Lemma ok_term_Kopen_push :
-      forall K Gamma d ty' T t ty,
-        is_value t ->
-        K \notin dom Gamma \u Kfv_t t \u Kfv_ty ty ->
-        Gamma & K ~ BindCon d ty' T |= Kopen_t 0 (FCon K) t ~: ty ->
-        Gamma |= push_value (TmConDef d ty' T) t ~: ty.
-    Proof with eauto with mcore.
-      introv Hval Hfresh Htype. forwards Henv : ok_term_ok_env Htype.
-      forwards (L0 & T' & Heq & Hd & Htk & HT): ok_env_con_inv Henv.
-      destruct Hval ; inverts Htype ; substs ; simpls.
-      { Case "TmLam". assert (Heq: Kopen_ty 0 (FCon K) ty0 = ty0) by apply~ notin_Kopen_ty.
-        rewrite Heq in *.
-        assert (Gamma |= ty0 ~:: KiType)
-          by (apply_empty~ (ok_type_con_strengthening K) ; eauto ; apply* ok_env_push).
-        assert (Hty' : forall x X,
-                   X \notin L0 \u dom Gamma \u \{x} ->
-                   x # Gamma ->
-                   Gamma & x ~ BindVar ty0 & X ~ BindTVar (KiData d) |= {0 ~> TyFVar X} ty' ~:: KiType).
-        { introv Hnin Hfr. forwards~ Htk' : Htk X. apply~ ok_type_weakening.
-          constructor*. constructor~. apply_empty~ ok_data_weakening. constructor*. }
-        apply_fresh* TLam as x.
-        forwards~ Htype': H4 x. apply_fresh TConDef as K'...
-        - apply_empty ok_data_weakening...
-        - applys~ ok_term_Kopen_change K.
-          + rewrite notin_union. rewrite~ open_notin_K.
-          + rewrite* Kopen_t_open_comm. apply_empty~ ok_term_comm.
-            apply_fresh EnvCon as X... apply_empty~ ok_data_weakening. constructor... }
-      { Case "TmTyLam". assert (Heq: Kopen_k 0 (FCon K) k = k) by apply~ notin_Kopen_k.
-        rewrite Heq in *.
-        assert (ok_kind Gamma k) by apply_empty* (ok_kind_con_strengthening K).
-        assert (Heq' : forall x, {1 ~> TyFVar x}ty' = ty').
-        { intros. pick_fresh y. apply topen_neq with (J := 0) (V := TyFVar y)...
-          rewrite~ topen_lct. apply* ok_type_lct. }
-        assert (Hty' : forall x X,
-                   X \notin L0 \u dom Gamma \u \{x} ->
-                   x # Gamma ->
-                   Gamma & x ~ BindTVar k & X ~ BindTVar (KiData d) |= {0 ~> TyFVar X} ty' ~:: KiType).
-        { introv Hnin Hfr. forwards~ Htk' : Htk X. apply~ ok_type_weakening.
-          constructor*. constructor~. apply_empty~ ok_data_weakening. constructor*. }
-        apply_fresh* TTyLam as X.
-        forwards~ Htype': H4 X. apply_fresh TConDef as K'...
-        - apply_empty ok_data_weakening...
-        - rewrite~ Heq'.
-        - rewrite Heq'. applys~ ok_term_Kopen_change K.
-          + rewrite notin_union. rewrite topen_t_notin_K. rewrite topen_notin_K ; simpls~.
-          + rewrite* Kopen_t_topen_comm. apply_empty~ ok_term_comm.
-            apply_fresh EnvCon as X... apply_empty~ ok_data_weakening. constructor... }
-      { Case "TmProd". constructor ; apply_fresh* TConDef as K' ; applys~ ok_term_Kopen_change K. }
-      { Case "TmCon". assert (Heq: Kopen_ty 0 (FCon K) ty0 = ty0) by apply~ notin_Kopen_ty.
-        rewrite Heq in *.
-        assert (Htk1 : Gamma |= ty0 ~:: KiData [ (FTName T0, FCon K1 :: []) ]).
-        { apply_empty* (ok_type_con_strengthening K). }
-        assert (Hneq : K1 <> K).
-        { intro ; subst. forwards~ Hk : ok_type_ok_kind Htk1.
-          inverts Hk as Hd'. inverts Hd'. inverts H11.
-          assert (K \indom Gamma) by applys get_some_inv H14.
-          assert (K # Gamma) by apply* ok_push_inv... }
-        replaces K0 with (FCon K1). { destruct K0 ; solve_var. }
-        constructors~.
-        + binds_cases H2...
-        + apply_empty (ok_type_con_strengthening K) ; eauto ; apply* ok_env_push.
-        + apply_fresh TConDef as K'... applys~ ok_term_Kopen_change K.
-          assert (K \notin Kfv_ty ({0 ~> ty0} ty1))...
-          rewrite~ topen_notin_K. binds_cases H2.
-          forwards (L'&?&?&?&Htk'&?): ok_env_binds_con_inv B. apply* ok_env_push.
-          pick_fresh X. forwards~ Hnin': ok_type_notin_K K (Htk' X).
-          rewrite~ topen_notin_K in Hnin'. simpls~. }
-    Qed.
+      Theorem preservation :
+        forall Gamma t t' ty,
+          Gamma |= t ~: ty ->
+          t --> t' ->
+          Gamma |= t' ~: ty.
+      Proof.
+        introv hasType Hstep.
+        gen t'.
+        induction hasType; intros; inverts Hstep ;
+          try (with_hyp (is_context _) as ctx ; with_hyp (_ = _) as eq
+               ; inverts ctx ; inverts* eq).
+        { Case "TmApp". inverts hasType1.
+          pick_fresh x. rewrite~ (subst_intro x).
+          apply_empty~ ok_term_subst. }
+        { Case "TmTyApp". inverts hasType.
+          pick_fresh X.
+          rewrite* (tsubst_intro X).
+          rewrite* (tsubst_t_intro X).
+          apply_empty~ ok_term_tsubst. }
+        { Case "TmFix". inverts hasType.
+          pick_fresh x. rewrite~ (subst_intro x).
+          apply_empty* ok_term_subst. }
+        { Case "TmProj1". inverts* hasType. }
+        { Case "TmProj2". inverts* hasType. }
+        { Case "TmType". pick_fresh T. applys* ok_term_Topen_push T t. }
+        { Case "TmTypeCong". apply_fresh TType as T' ; auto. }
+        { Case "TmConDef". pick_fresh K. applys* ok_term_Kopen_push K t. }
+        { Case "TmConDefCong". apply_fresh TConDef as K' ; auto. }
+        { Case "TmSemApp".
+          assert (i < length ps0) by apply* matchN_length.
+          forwards* (L&ty1'&Hpat&Htype) : ok_term_get_cases_inv i.
+          remember (nth i bs) ; pick_fresh x ; substs. rewrite~ (subst_intro x).
+          apply_empty~ ok_term_subst.
+          apply* matchN_ok_pat. }
+      Qed.
 
-    Theorem preservation :
-      forall Gamma t t' ty,
-        Gamma |= t ~: ty ->
-        t --> t' ->
-        Gamma |= t' ~: ty.
-    Proof.
-      introv hasType Hstep.
-      gen t'.
-      induction hasType; intros; inverts Hstep ;
-        try (with_hyp (is_context _) as ctx ; with_hyp (_ = _) as eq
-             ; inverts ctx ; inverts* eq).
-      { Case "TmApp". inverts hasType1.
-        pick_fresh x. rewrite~ (subst_intro x).
-        apply_empty~ ok_term_subst. }
-      { Case "TmTyApp". inverts hasType.
-        pick_fresh X.
-        rewrite* (tsubst_intro X).
-        rewrite* (tsubst_t_intro X).
-        apply_empty~ ok_term_tsubst. }
-      { Case "TmFix". inverts hasType.
-        pick_fresh x. rewrite~ (subst_intro x).
-        apply_empty* ok_term_subst. }
-      { Case "TmProj1". inverts* hasType. }
-      { Case "TmProj2". inverts* hasType. }
-      { Case "TmType". pick_fresh T. applys* ok_term_Topen_push T t. }
-      { Case "TmTypeCong". apply_fresh TType as T' ; auto. }
-      { Case "TmConDef". pick_fresh K. applys* ok_term_Kopen_push K t. }
-      { Case "TmConDefCong". apply_fresh TConDef as K' ; auto. }
-    Qed.
+      Definition no_vars (Gamma : env) : Prop :=
+        forall x ty, binds x (BindVar ty) Gamma -> False.
 
-    Definition no_vars (Gamma : env) : Prop :=
-      forall x ty, binds x (BindVar ty) Gamma -> False.
+      Theorem progress :
+        forall Gamma t ty,
+          no_vars Gamma ->
+          Gamma |= t ~: ty ->
+          is_value t \/ exists t', t --> t'.
+      Proof.
+        introv Hnv hasType.
+        induction hasType; substs*.
+        { Case "TmFVar". false. apply* Hnv. }
+        { Case "TmApp". right.
+          forwards* [Hval1 | (t1' & Hstep1)]: IHhasType1.
+          forwards* [Hval2 | (t2' & Hstep2)]: IHhasType2.
+          inverts Hval1; inverts* hasType1. }
+        { Case "TmTyApp". right.
+          forwards* [Hval | (t1 & Hstep)]: IHhasType.
+          inverts Hval; inverts* hasType. }
+        { Case "TmFix". right.
+          forwards* [Hval1 | (t1' & Hstep1)]: IHhasType.
+          inverts Hval1; inverts* hasType. }
+        { Case "TmProd".
+          forwards* [Hval1 | (t1' & Hstep1)]: IHhasType1.
+          forwards* [Hval2 | (t2' & Hstep2)]: IHhasType2. }
+        { Case "TmProj1".
+          forwards* [Hval1 | (t1' & Hstep1)]: IHhasType.
+          inverts Hval1; inverts* hasType. }
+        { Case "TmProj2".
+          forwards* [Hval1 | (t1' & Hstep1)]: IHhasType.
+          inverts Hval1; inverts* hasType. }
+        { Case "TmCon".
+          forwards* [Hval | (t' & Hstep)]: IHhasType. }
+        { Case "TmType". right. pick_fresh T.
+          forwards* [Hval | (t' & Hstep)]: H0 T.
+          + introv Hb. binds_cases Hb. apply* Hnv.
+          + forwards* Hval' : Topen_is_value Hval.
+          + rewrite <- (Topen_t_Tclose 0 T t') in Hstep.
+            * eexists. apply_fresh ETypeCong.
+              apply* Topen_step_change. lets~ ?: Tclose_t_notin T 0 t'.
+            * lets* ?: preservation Hstep. }
+        { Case "TmConDef". right. pick_fresh K.
+          forwards* [Hval | (t' & Hstep)]: H3 K.
+          + introv Hb. binds_cases Hb. apply* Hnv.
+          + forwards* Hval' : Kopen_is_value Hval.
+          + rewrite <- (Kopen_t_Kclose 0 K t') in Hstep.
+            * eexists. apply_fresh EConDefCong.
+              apply* Kopen_step_change. lets~ ?: Kclose_t_notin K 0 t'.
+            * lets* ?: preservation Hstep. }
+        { Case "TmComp".
+          forwards* [Hval1 | (t1' & Hstep1)]: IHhasType1.
+          forwards* [Hval2 | (t2' & Hstep2)]: IHhasType2. }
+        { Case "TmSemApp". right.
+          forwards* [Hval1 | (t1' & Hstep1)]: IHhasType1.
+          forwards* [Hval2 | (t2' & Hstep2)]: IHhasType2.
+          forwards* (i&v'&Hmatch): exhaustive_has_match hasType2.
+          destruct (get_cases t1) as (ps0&bs) eqn:Hget.
+          forwards* Heq : ok_term_get_cases_eq ; substs*. }
+      Qed.
 
-    Theorem progress :
-      forall Gamma t ty,
-        no_vars Gamma ->
-        Gamma |= t ~: ty ->
-        is_value t \/ exists t', t --> t'.
-    Proof.
-      introv Hnv hasType.
-      induction hasType; substs*.
-      { Case "TmFVar". false. apply* Hnv. }
-      { Case "TmApp". right.
-        forwards* [Hval1 | (t1' & Hstep1)]: IHhasType1.
-        forwards* [Hval2 | (t2' & Hstep2)]: IHhasType2.
-        inverts Hval1; inverts* hasType1. }
-      { Case "TmTyApp". right.
-        forwards* [Hval | (t1 & Hstep)]: IHhasType.
-        inverts Hval; inverts* hasType. }
-      { Case "TmFix". right.
-        forwards* [Hval1 | (t1' & Hstep1)]: IHhasType.
-        inverts Hval1; inverts* hasType. }
-      { Case "TmProd".
-        forwards* [Hval1 | (t1' & Hstep1)]: IHhasType1.
-        forwards* [Hval2 | (t2' & Hstep2)]: IHhasType2. }
-      { Case "TmProj1".
-        forwards* [Hval1 | (t1' & Hstep1)]: IHhasType.
-        inverts Hval1; inverts* hasType. }
-      { Case "TmProj2".
-        forwards* [Hval1 | (t1' & Hstep1)]: IHhasType.
-        inverts Hval1; inverts* hasType. }
-      { Case "TmCon".
-        forwards* [Hval | (t' & Hstep)]: IHhasType. }
-      { Case "TmType". right. pick_fresh T.
-        forwards* [Hval | (t' & Hstep)]: H0 T.
-        + introv Hb. binds_cases Hb. apply* Hnv.
-        + forwards* Hval' : Topen_is_value Hval.
-        + rewrite <- (Topen_t_Tclose 0 T t') in Hstep.
-          * eexists. apply_fresh ETypeCong.
-            apply* Topen_step_change. lets~ ?: Tclose_t_notin T 0 t'.
-          * lets* ?: preservation Hstep. }
-      { Case "TmConDef". right. pick_fresh K.
-        forwards* [Hval | (t' & Hstep)]: H3 K.
-        + introv Hb. binds_cases Hb. apply* Hnv.
-        + forwards* Hval' : Kopen_is_value Hval.
-        + rewrite <- (Kopen_t_Kclose 0 K t') in Hstep.
-          * eexists. apply_fresh EConDefCong.
-            apply* Kopen_step_change. lets~ ?: Kclose_t_notin K 0 t'.
-          * lets* ?: preservation Hstep. }
-    Qed.
-
-  End Soundness.
+    End Soundness2.
+  End Soundness1.
 End Soundness.
