src/SyntaxProps.v
@@ -1,0 +1,2001 @@
+From TLC Require Import LibList LibLN.
+From MCore Require Import Syntax Tactics.
+
+Module SyntaxProps (P : PAT).
+  Module S := Syntax P.
+  Export S.
+
+  (****************************************)
+  (** PROPERTIES OF OPERATIONS ON SYNTAX **)
+  (****************************************)
+
+  Lemma topen_neq :
+    forall I J U V T,
+      I <> J ->
+      {I ~> U}({J ~> V}T) = {J ~> V}T ->
+      {I ~> U}T = T.
+  Proof.
+    introv Hneq Heq. gen I J.
+    solve_eq T; inverts* Heq.
+  Qed.
+
+  Lemma topen_lct :
+    forall K U T,
+      lct T ->
+      {K ~> U}T = T.
+  Proof.
+    introv Hlct. gen K.
+    solve_eq Hlct.
+    - pick_fresh x.
+      rewrite topen_neq with (J := 0) (V := TyFVar x);
+        auto.
+  Qed.
+
+  Lemma tsubst_topen_distr :
+    forall X U k T1 T2,
+      lct U ->
+      {X => U} ({k ~> T2}T1) = {k ~> {X => U}T2} ({X => U}T1).
+  Proof.
+    introv Hlct. gen k.
+    solve_eq T1. rewrite* topen_lct.
+  Qed.
+
+  Lemma tsubst_fresh :
+    forall X T U,
+      X \notin tfv T ->
+      {X => U}T = T.
+  Proof. introv Hfv ; solve_eq T. Qed.
+
+  Lemma tsubst_intro :
+    forall X T U n,
+      X \notin tfv T ->
+      {n ~> U} T = {X => U}({n ~> TyFVar X}T).
+  Proof. introv Hfv. gen n. solve_eq T. Qed.
+
+  Lemma tsubst_topen_comm :
+    forall X Y U T n,
+      X <> Y ->
+      lct U ->
+      {n ~> TyFVar Y} ({X => U}T) = {X => U}({n ~> TyFVar Y} T).
+  Proof.
+    introv Hneq Hlct. gen n.
+    solve_eq T ; rewrite* topen_lct.
+  Qed.
+
+  Lemma tsubst_lct :
+    forall X U T,
+      lct T ->
+      lct U ->
+      lct ({X => U}T).
+  Proof.
+    introv Hlct1 Hlct2.
+    induction* Hlct1; solve_var.
+    - apply_fresh* LCTAll.
+      rewrite* tsubst_topen_comm.
+  Qed.
+
+  Lemma open_neq :
+    forall i j u v t,
+      i <> j ->
+      [i ~> u]([j ~> v]t) = [j ~> v]t ->
+      [i ~> u]t = t.
+  Proof.
+    introv Hneq Heq. gen i j. solve_eq t ; inverts* Heq.
+  Qed.
+
+  Lemma open_topen_neq :
+    forall i u J V t,
+      [i ~> u]([{J ~> V}]t) = [{J ~> V}] t ->
+      [i ~> u]t = t.
+  Proof.
+    introv Heq. gen i J. solve_eq t ; inverts* Heq.
+  Qed.
+
+  Lemma open_Topen_rec :
+    forall i u J V t,
+      [i ~> u](Topen_t J V t) = Topen_t J V t ->
+      [i ~> u]t = t.
+  Proof.
+    introv Heq. gen i J. solve_eq t ; inverts* Heq.
+  Qed.
+
+  Lemma open_Kopen_rec :
+    forall i u J V t,
+      [i ~> u](Kopen_t J V t) = Kopen_t J V t ->
+      [i ~> u]t = t.
+  Proof.
+    introv Heq. gen i J. solve_eq t ; inverts* Heq.
+  Qed.
+
+  Lemma open_lc :
+    forall k u t,
+      lc t ->
+      [k ~> u]t = t.
+  Proof.
+    introv Hlc. gen k.
+    solve_eq Hlc.
+    - pick_fresh x.
+      rewrite open_neq with (j := 0) (v := TmFVar x);
+        auto.
+    - pick_fresh X.
+      rewrite open_topen_neq with (J := 0) (V := TyFVar X);
+        auto.
+    - pick_fresh X.
+      rewrite open_Topen_rec with (J := 0) (V := FTName X);
+        auto.
+    - pick_fresh X.
+      rewrite open_Kopen_rec with (J := 0) (V := FCon X);
+        auto.
+    - pick_fresh x.
+      rewrite open_neq with (j := 0) (v := TmFVar x);
+        auto.
+  Qed.
+
+  Lemma subst_open_distr :
+    forall x u n t1 t2,
+      lc u ->
+      [x => u] ([n ~> t2] t1) = [n ~> [x => u]t2]([x => u]t1).
+  Proof.
+    introv Hlc. gen n.
+    solve_eq t1. rewrite* open_lc.
+  Qed.
+
+  Lemma subst_open_comm :
+    forall x y n u t,
+      x <> y ->
+      lc u ->
+      [n ~> TmFVar y]([x => u]t) = [x => u] ([n ~> TmFVar y]t).
+  Proof.
+    introv Hneq Hlc. gen n.
+    solve_eq t. apply* open_lc.
+  Qed.
+
+  Lemma subst_fresh :
+    forall x t u,
+      x \notin fv t ->
+      [x => u]t = t.
+  Proof. solve_eq t. Qed.
+
+  Lemma subst_intro :
+    forall x t u n,
+      x \notin fv t ->
+      [n ~> u] t = [x => u]([n ~> TmFVar x]t).
+  Proof. introv Hfv. gen n. solve_eq t. Qed.
+
+  Lemma tsubst_t_topen_distr :
+    forall X U n T t,
+      lct U ->
+      [{X => U}] ([{n ~> T}] t) = [{n ~> {X => U}T}] ([{X => U}]t).
+  Proof.
+    introv Hlct.
+    gen n. solve_eq t ;
+      apply* tsubst_topen_distr.
+  Qed.
+
+  Lemma tsubst_t_fresh :
+    forall X t U,
+      X \notin tfv_t t ->
+      [{X => U}]t = t.
+  Proof.
+    introv Hfv.
+    solve_eq t; apply* tsubst_fresh.
+  Qed.
+
+  Lemma tsubst_t_intro :
+    forall X U t,
+      X \notin tfv_t t ->
+      lct U ->
+      [{0 ~> U}]t = [{X => U}] ([{0 ~> TyFVar X}]t).
+  Proof.
+    introv Hftv Hlc.
+    rewrite* tsubst_t_topen_distr.
+    solve_var. rewrite* tsubst_t_fresh.
+  Qed.
+
+  Lemma topen_open_rec :
+    forall i j T t u,
+      [{i ~> T}] ([j ~> u] t) = [j ~> u]t ->
+      [{i ~> T}] t = t.
+  Proof.
+    introv Heq. gen i j.
+    solve_eq t ; inverts* Heq.
+  Qed.
+
+  Lemma topen_t_neq :
+    forall I J T U t,
+      I <> J ->
+      [{I ~> T}] ([{J ~> U}] t) = [{J ~> U}] t ->
+      [{I ~> T}]t = t.
+  Proof.
+    introv Hneq Heq. gen I J.
+    solve_eq t ; inverts* Heq; eauto using topen_neq.
+  Qed.
+
+  Lemma topen_Topen_rec :
+    forall i j T U T',
+      {i ~> T} (Topen_ty j T' U) = Topen_ty j T' U ->
+      {i ~> T}U = U.
+  Proof.
+    introv Heq. gen i.
+    solve_eq U ; inverts* Heq.
+  Qed.
+
+  Lemma topen_t_Topen_rec :
+    forall i j T t T',
+      [{i ~> T}] (Topen_t j T' t) = Topen_t j T' t ->
+      [{i ~> T}]t = t.
+  Proof.
+    introv Heq. gen i j.
+    solve_eq t ; inverts* Heq ; apply* topen_Topen_rec.
+  Qed.
+
+  Lemma topen_Kopen_rec :
+    forall i j T U K,
+      {i ~> T} (Kopen_ty j K U) = Kopen_ty j K U ->
+      {i ~> T}U = U.
+  Proof.
+    introv Heq. gen i.
+    solve_eq U ; inverts* Heq.
+  Qed.
+
+  Lemma topen_t_Kopen_rec :
+    forall i j T t K,
+      [{i ~> T}] (Kopen_t j K t) = Kopen_t j K t ->
+      [{i ~> T}]t = t.
+  Proof.
+    introv Heq. gen i j.
+    solve_eq t ; inverts* Heq ; apply* topen_Kopen_rec.
+  Qed.
+
+  Lemma topen_t_lc :
+    forall X t n,
+      lc t ->
+      [{n ~> TyFVar X}]t = t.
+  Proof.
+    introv Hlc. gen n.
+    solve_eq Hlc ; try solve [ rewrite~ topen_lct ] ; pick_fresh_gen L x.
+    - apply* topen_open_rec.
+    - apply* (topen_t_neq (S n) 0 (TyFVar X) (TyFVar x)).
+    - apply* topen_t_Topen_rec.
+    - apply topen_neq with (J := 0) (V := TyFVar x) ; auto.
+      apply* topen_lct.
+    - apply* topen_t_Kopen_rec.
+    - apply* topen_open_rec.
+  Qed.
+
+  Lemma topen_t_subst_comm :
+    forall X x n t1 t2,
+      X \notin tfv_t t2 ->
+      lc t2 ->
+      [{n ~> TyFVar X}] ([x => t2]t1) = [x => t2]([{n ~> TyFVar X}] t1).
+  Proof.
+    introv Hnin Hlc. gen n.
+    solve_eq t1. rewrite* topen_t_lc.
+  Qed.
+
+  Lemma tsubst_t_open_comm :
+    forall X x n U t,
+      [n ~> TmFVar x] ([{X => U}]t) = [{X => U}] ([n ~> TmFVar x]t).
+  Proof. intros. gen n. solve_eq t. Qed.
+
+  Lemma topen_notin :
+    forall T X Y n,
+      X \notin tfv ({n ~> TyFVar Y}T) ->
+      X \notin tfv T.
+  Proof.
+    introv Hnin. gen n.
+    induction T; intros; simpls* ;
+      apply notin_union_r in Hnin as (Hnin1 & Hnin2) ; eauto.
+  Qed.
+
+  Lemma topen_t_tsubst_comm :
+    forall X Y T n t,
+      X <> Y ->
+      lct T ->
+      [{n ~> TyFVar Y}] ([{X => T}]t) =
+        [{X => T}]([{n ~> TyFVar Y}] t).
+  Proof.
+    introv Hneq Hlct. gen n.
+    solve_eq t ; rewrite* tsubst_topen_comm.
+  Qed.
+
+  Lemma Topen_Topen_neq :
+    forall i j T T' T0,
+      i <> j ->
+      Topen i T (Topen j T' T0) = Topen j T' T0 ->
+      Topen i T T0 = T0.
+  Proof. introv Hneq Heq. solve_eq T0. Qed.
+
+  Lemma Topen_d_lcd :
+    forall j T d,
+      lcd d ->
+      Topen_d j T d = d.
+  Proof.
+    introv Hlcd.
+    solve_eq Hlcd. unfolds Topen_d. rew_listx.
+    destruct x. destruct H.
+    inverts H. rewrite~ IHHlcd.
+  Qed.
+
+  Lemma Topen_Topen_d_neq :
+    forall i j T T' d,
+      i <> j ->
+      Topen_d i T (Topen_d j T' d) = Topen_d j T' d ->
+      Topen_d i T d = d.
+  Proof.
+    introv Hneq Heq. unfolds Topen_d.
+    induction~ d.
+    rew_listx in *. destruct a. inverts Heq.
+    rewrite Topen_Topen_neq with (j := j) (T' := T') ; auto.
+    rewrite~ IHd.
+  Qed.
+
+  Lemma Topen_Kopen_d_rec :
+    forall i j T K d,
+      Topen_d i T (Kopen_d j K d) = Kopen_d j K d ->
+      Topen_d i T d = d.
+  Proof.
+    introv Heq. unfolds Topen_d. unfolds Kopen_d.
+    induction~ d.
+    rew_listx in *. destruct a. injection Heq ; intros. rewrite H0.
+    rewrite~ IHd.
+  Qed.
+
+  Lemma Topen_k_lck :
+    forall j T k,
+      lck k ->
+      Topen_k j T k = k.
+  Proof.
+    introv Hlck. solve_eq Hlck. rewrite~ Topen_d_lcd.
+  Qed.
+
+  Lemma Topen_Topen_k_neq :
+    forall i j T T' k,
+      i <> j ->
+      Topen_k i T (Topen_k j T' k) = Topen_k j T' k ->
+      Topen_k i T k = k.
+  Proof.
+    introv Hneq Heq.
+    solve_eq k. inverts Heq. apply Topen_Topen_d_neq with (j := j) (T' := T') ; auto.
+  Qed.
+
+  Lemma Topen_Kopen_k_rec :
+    forall i j T K k,
+      Topen_k i T (Kopen_k j K k) = Kopen_k j K k ->
+      Topen_k i T k = k.
+  Proof.
+    introv Heq. solve_eq k ; inverts Heq. apply* Topen_Kopen_d_rec.
+  Qed.
+
+  Lemma Topen_topen_rec :
+    forall i j T U ty,
+      Topen_ty i T ({j ~> U} ty) = {j ~> U}ty ->
+      Topen_ty i T ty = ty.
+  Proof.
+    introv Heq. gen j.
+    solve_eq ty ; inverts* Heq.
+  Qed.
+
+  Lemma Topen_ty_lct :
+    forall k T ty,
+      lct ty ->
+      Topen_ty k T ty = ty.
+  Proof.
+    introv Hlct.
+    solve_eq Hlct ;
+      try solve [ apply* Topen_d_lcd
+                | apply* Topen_k_lck ] ;
+      pick_fresh_gen L x.
+    - apply* Topen_topen_rec.
+  Qed.
+
+  Lemma Topen_Topen_ty_neq :
+    forall i j T T' ty,
+      i <> j ->
+      Topen_ty i T (Topen_ty j T' ty) = Topen_ty j T' ty ->
+      Topen_ty i T ty = ty.
+  Proof.
+    introv Hneq Heq. gen i j.
+    solve_eq ty ; inverts* Heq.
+    - apply Topen_Topen_k_neq with (j := j) (T' := T') ; auto.
+    - apply Topen_Topen_neq with (j := j) (T' := T') ; auto.
+    - apply Topen_Topen_d_neq with (j := j) (T' := T') ; auto.
+  Qed.
+
+  Lemma Topen_Kopen_ty_rec :
+    forall i j T K ty,
+      Topen_ty i T (Kopen_ty j K ty) = Kopen_ty j K ty ->
+      Topen_ty i T ty = ty.
+  Proof.
+    introv Heq.
+    solve_eq ty ; inverts* Heq.
+    - apply* Topen_Kopen_k_rec.
+    - apply* Topen_Kopen_d_rec.
+  Qed.
+
+  Lemma Topen_open_rec :
+    forall i j T u t,
+      Topen_t i T ([j ~> u] t) = [j ~> u]t ->
+      Topen_t i T t = t.
+  Proof.
+    introv Heq. gen i j.
+    solve_eq t ; inverts* Heq.
+  Qed.
+
+  Lemma Topen_topen_t_rec :
+    forall i j T ty t,
+      Topen_t i T ([{j ~> ty}] t) = [{j ~> ty}] t ->
+      Topen_t i T t = t.
+  Proof.
+    introv Heq. gen i j.
+    solve_eq t ; inverts* Heq ; apply* Topen_topen_rec.
+  Qed.
+
+  Lemma Topen_Topen_t_neq :
+    forall i j T T' t,
+      i <> j ->
+      Topen_t i T (Topen_t j T' t) = Topen_t j T' t ->
+      Topen_t i T t = t.
+  Proof.
+    introv Hneq Heq. gen i j.
+    solve_eq t ; inverts* Heq ;
+      solve [ apply Topen_Topen_neq with (j := j) (T' := T') ; auto
+            | apply Topen_Topen_d_neq with (j := j) (T' := T') ; auto
+            | apply Topen_Topen_k_neq with (j := j) (T' := T') ; auto
+            | apply Topen_Topen_ty_neq with (j := j) (T' := T') ; auto ].
+  Qed.
+
+  Lemma Topen_Kopen_t_rec :
+    forall i j T K t,
+      Topen_t i T (Kopen_t j K t) = Kopen_t j K t ->
+      Topen_t i T t = t.
+  Proof.
+    introv Heq. gen i j.
+    solve_eq t ; inverts* Heq ;
+      solve [ apply* Topen_Kopen_d_rec
+            | apply* Topen_Kopen_k_rec
+            | apply* Topen_Kopen_ty_rec ].
+  Qed.
+
+  Lemma Topen_t_lc :
+    forall k T t,
+      lc t ->
+      Topen_t k T t = t.
+  Proof.
+    introv Hlc. gen k.
+    solve_eq Hlc ;
+      try solve [ apply* Topen_d_lcd
+                | apply* Topen_k_lck
+                | apply* Topen_ty_lct ] ;
+      pick_fresh_gen L x.
+    - apply* Topen_open_rec.
+    - apply* Topen_topen_t_rec.
+    - apply* (Topen_Topen_t_neq (S k) 0 T (FTName x)).
+    - apply* Topen_topen_rec.
+      apply* Topen_ty_lct.
+    - apply* Topen_Kopen_t_rec.
+    - apply* Topen_open_rec.
+  Qed.
+
+  Lemma Topen_t_subst_comm :
+    forall x n T t1 t2,
+      lc t2 ->
+      Topen_t n T ([x => t2]t1) = [x => t2] (Topen_t n T t1).
+  Proof.
+    introv Hlc. gen n. solve_eq t1. apply* Topen_t_lc.
+  Qed.
+
+  Lemma Topen_tsubst_comm :
+    forall X n T U ty,
+      lct U ->
+      Topen_ty n T ({X => U}ty) = {X => U} (Topen_ty n T ty).
+  Proof.
+    introv Hlct. gen n. solve_eq ty ; apply* Topen_ty_lct.
+  Qed.
+
+  Lemma Topen_t_tsubst_comm :
+    forall X n T U t,
+      lct U ->
+      Topen_t n T ([{X => U}]t) = [{X => U}] (Topen_t n T t).
+  Proof.
+    introv Hlc. gen n. solve_eq t ; apply* Topen_tsubst_comm.
+  Qed.
+
+
+  Lemma Kopen_Kopen_neq :
+    forall i j K K' K0,
+      i <> j ->
+      Kopen i K (Kopen j K' K0) = Kopen j K' K0 ->
+      Kopen i K K0 = K0.
+  Proof. introv Hneq Heq. solve_eq K0. Qed.
+
+  Lemma Kopen_d_lcd :
+    forall j T d,
+      lcd d ->
+      Kopen_d j T d = d.
+  Proof.
+    introv Hlcd.
+    solve_eq Hlcd. unfolds Kopen_d. rew_listx.
+    destruct x. destruct H. rewrite~ IHHlcd.
+    induction~ l0. rew_listx in *. destruct H0. inverts H0. simpls.
+    apply IHl0 in H1. injection H1 ; intros. rewrite* H0.
+  Qed.
+
+  Lemma Kopen_Kopen_d_neq :
+    forall i j K K' d,
+      i <> j ->
+      Kopen_d i K (Kopen_d j K' d) = Kopen_d j K' d ->
+      Kopen_d i K d = d.
+  Proof.
+    introv Hneq Heq. unfolds Kopen_d.
+    induction~ d.
+    rew_listx in *. destruct a. inverts Heq.
+    rewrite~ IHd. repeat fequals.
+    induction~ l. rew_listx in *. inverts H0. rewrite~ IHl.
+    rewrite Kopen_Kopen_neq with (j := j) (K' := K') ; auto.
+  Qed.
+
+  Lemma Kopen_Topen_d_rec :
+    forall i j T K d,
+      Kopen_d i K (Topen_d j T d) = Topen_d j T d ->
+      Kopen_d i K d = d.
+  Proof.
+    introv Heq. unfolds Kopen_d. unfolds Topen_d.
+    induction~ d.
+    rew_listx in *. destruct a. injection Heq ; intros. rewrite H0.
+    rewrite~ IHd.
+  Qed.
+
+  Lemma Kopen_k_lck :
+    forall j T k,
+      lck k ->
+      Kopen_k j T k = k.
+  Proof.
+    introv Hlck. solve_eq Hlck. rewrite~ Kopen_d_lcd.
+  Qed.
+
+  Lemma Kopen_Kopen_k_neq :
+    forall i j K K' k,
+      i <> j ->
+      Kopen_k i K (Kopen_k j K' k) = Kopen_k j K' k ->
+      Kopen_k i K k = k.
+  Proof.
+    introv Hneq Heq.
+    solve_eq k. inverts Heq. apply Kopen_Kopen_d_neq with (j := j) (K' := K') ; auto.
+  Qed.
+
+  Lemma Kopen_Topen_k_rec :
+    forall i j T K k,
+      Kopen_k i K (Topen_k j T k) = Topen_k j T k ->
+      Kopen_k i K k = k.
+  Proof.
+    introv Heq. solve_eq k ; inverts Heq. apply* Kopen_Topen_d_rec.
+  Qed.
+
+  Lemma Kopen_topen_rec :
+    forall i j T U ty,
+      Kopen_ty i T ({j ~> U} ty) = {j ~> U}ty ->
+      Kopen_ty i T ty = ty.
+  Proof.
+    introv Heq. gen j.
+    solve_eq ty ; inverts* Heq.
+  Qed.
+
+  Lemma Kopen_ty_lct :
+    forall k T ty,
+      lct ty ->
+      Kopen_ty k T ty = ty.
+  Proof.
+    introv Hlct.
+    solve_eq Hlct ;
+      try solve [ apply* Kopen_d_lcd
+                | apply* Kopen_k_lck ] ;
+      pick_fresh_gen L x.
+    - apply* Kopen_topen_rec.
+  Qed.
+
+  Lemma Kopen_Kopen_ty_neq :
+    forall i j K K' ty,
+      i <> j ->
+      Kopen_ty i K (Kopen_ty j K' ty) = Kopen_ty j K' ty ->
+      Kopen_ty i K ty = ty.
+  Proof.
+    introv Hneq Heq. gen i j.
+    solve_eq ty ; inverts* Heq.
+    - apply Kopen_Kopen_k_neq with (j := j) (K' := K') ; auto.
+    - apply Kopen_Kopen_d_neq with (j := j) (K' := K') ; auto.
+  Qed.
+
+  Lemma Kopen_Topen_ty_rec :
+    forall i j T K ty,
+      Kopen_ty i K (Topen_ty j T ty) = Topen_ty j T ty ->
+      Kopen_ty i K ty = ty.
+  Proof.
+    introv Heq.
+    solve_eq ty ; inverts* Heq.
+    - apply* Kopen_Topen_k_rec.
+    - apply* Kopen_Topen_d_rec.
+  Qed.
+
+  Lemma Kopen_open_rec :
+    forall i j T u t,
+      Kopen_t i T ([j ~> u] t) = [j ~> u]t ->
+      Kopen_t i T t = t.
+  Proof.
+    introv Heq. gen i j.
+    solve_eq t ; inverts* Heq.
+  Qed.
+
+  Lemma Kopen_topen_t_rec :
+    forall i j T ty t,
+      Kopen_t i T ([{j ~> ty}] t) = [{j ~> ty}] t ->
+      Kopen_t i T t = t.
+  Proof.
+    introv Heq. gen i j.
+    solve_eq t ; inverts* Heq ; apply* Kopen_topen_rec.
+  Qed.
+
+  Lemma Kopen_Kopen_t_neq :
+    forall i j K K' t,
+      i <> j ->
+      Kopen_t i K (Kopen_t j K' t) = Kopen_t j K' t ->
+      Kopen_t i K t = t.
+  Proof.
+    introv Hneq Heq. gen i j.
+    solve_eq t ; inverts* Heq ;
+      try solve [ apply Kopen_Kopen_neq with (j := j) (K' := K') ; auto
+                | apply Kopen_Kopen_d_neq with (j := j) (K' := K') ; auto
+                | apply Kopen_Kopen_k_neq with (j := j) (K' := K') ; auto
+                | apply Kopen_Kopen_ty_neq with (j := j) (K' := K') ; auto ].
+  Qed.
+
+  Lemma Kopen_Topen_t_rec :
+    forall i j T K t,
+      Kopen_t i K (Topen_t j T t) = Topen_t j T t ->
+      Kopen_t i K t = t.
+  Proof.
+    introv Heq. gen i j.
+    solve_eq t ; inverts* Heq ;
+      solve [ apply* Kopen_Topen_d_rec
+            | apply* Kopen_Topen_k_rec
+            | apply* Kopen_Topen_ty_rec ].
+  Qed.
+
+  Lemma Kopen_t_lc :
+    forall k K t,
+      lc t ->
+      Kopen_t k K t = t.
+  Proof.
+    introv Hlc. gen k.
+    solve_eq Hlc ;
+      try solve [ apply* Kopen_d_lcd
+                | apply* Kopen_k_lck
+                | apply* Kopen_ty_lct ] ;
+      pick_fresh_gen L x.
+    - apply* Kopen_open_rec.
+    - apply* Kopen_topen_t_rec.
+    - apply* Kopen_Topen_t_rec.
+    - apply* Kopen_topen_rec.
+      apply* Kopen_ty_lct.
+    - apply* (Kopen_Kopen_t_neq (S k) 0 K (FCon x)).
+    - apply* Kopen_open_rec.
+  Qed.
+
+  Lemma Kopen_t_subst_comm :
+    forall x n K t1 t2,
+      lc t2 ->
+      Kopen_t n K ([x => t2]t1) = [x => t2] (Kopen_t n K t1).
+  Proof.
+    introv Hlc. gen n. solve_eq t1 ; apply* Kopen_t_lc.
+  Qed.
+
+  Lemma Kopen_tsubst_comm :
+    forall X n T U ty,
+      lct U ->
+      Kopen_ty n T ({X => U}ty) = {X => U} (Kopen_ty n T ty).
+  Proof.
+    introv Hlct. gen n. solve_eq ty ; apply* Kopen_ty_lct.
+  Qed.
+
+  Lemma Kopen_t_tsubst_comm :
+    forall X n T U t,
+      lct U ->
+      Kopen_t n T ([{X => U}]t) = [{X => U}] (Kopen_t n T t).
+  Proof.
+    introv Hlc. gen n. solve_eq t ; apply* Kopen_tsubst_comm.
+  Qed.
+
+  Lemma Topen_t_open_comm :
+    forall i n T v t,
+      lc v ->
+      Topen_t i T ([n ~> v] t) = [n ~> v] (Topen_t i T t).
+  Proof.
+    introv Hlc. gen n i. solve_eq t. apply* Topen_t_lc.
+  Qed.
+
+  Lemma Tclose_d_fresh :
+    forall T i d,
+      T \notin Tfv_d d ->
+      Tclose_d T i d = d.
+  Proof.
+    introv Hfv. unfolds Tclose_d. unfolds Tfv_d.
+    induction~ d.
+    rew_listx in *. destruct a. rewrite~ IHd. destruct t ; solve_var.
+  Qed.
+
+  Lemma Tclose_k_fresh :
+    forall T i k,
+      T \notin Tfv_k k ->
+      Tclose_k T i k = k.
+  Proof. introv Hfv. solve_eq k ; apply~ Tclose_d_fresh. Qed.
+
+  Lemma Tclose_ty_fresh :
+    forall T i ty,
+      T \notin Tfv_ty ty ->
+      Tclose_ty T i ty = ty.
+  Proof.
+    introv Hfv. solve_eq ty.
+    - apply~ Tclose_k_fresh.
+    - destruct t ; solve_var.
+    - apply~ Tclose_d_fresh.
+  Qed.
+
+  Lemma Tclose_t_fresh :
+    forall T i t,
+      T \notin Tfv_t t ->
+      Tclose_t T i t = t.
+  Proof.
+    introv Hfv. gen i. solve_eq t ;
+      try solve [ apply~ Tclose_d_fresh
+                | apply~ Tclose_k_fresh
+                | apply~ Tclose_ty_fresh ].
+    destruct t0 ; solve_var.
+  Qed.
+
+  Lemma Tclose_t_open_comm :
+    forall i n T v t,
+      T \notin Tfv_t v ->
+      Tclose_t T i ([n ~> v] t) = [n ~> v] (Tclose_t T i t).
+  Proof.
+    introv. gen i n. solve_eq t ; apply* Tclose_t_fresh.
+  Qed.
+
+  Lemma Topen_ty_topen_comm :
+    forall i n T ty1 ty2,
+      lct ty1 ->
+      Topen_ty i T ({n ~> ty1} ty2) = {n ~> ty1} (Topen_ty i T ty2).
+  Proof.
+    introv. gen n. solve_eq ty2. apply* Topen_ty_lct.
+  Qed.
+
+  Lemma Topen_t_topen_comm :
+    forall i n T ty t,
+      lct ty ->
+      Topen_t i T ([{n ~> ty}] t) = [{n ~> ty}] (Topen_t i T t).
+  Proof.
+    introv. gen n i. solve_eq t ; apply* Topen_ty_topen_comm.
+  Qed.
+
+  Lemma Tclose_ty_topen_comm :
+    forall i n T ty1 ty2,
+      T \notin Tfv_ty ty1 ->
+      Tclose_ty T i ({n ~> ty1} ty2) = {n ~> ty1} (Tclose_ty T i ty2).
+  Proof.
+    introv. gen n. solve_eq ty2 ; apply* Tclose_ty_fresh.
+  Qed.
+
+  Lemma Tclose_t_topen_comm :
+    forall i n T ty t,
+      T \notin Tfv_ty ty ->
+      Tclose_t T i ([{n ~> ty}] t) = [{n ~> ty}] (Tclose_t T i t).
+  Proof.
+    introv. gen n i. solve_eq t ; apply* Tclose_ty_topen_comm.
+  Qed.
+
+  Lemma Topen_d_Topen_comm :
+    forall i j T T' d,
+      i <> j ->
+      Topen_d i (FTName T) (Topen_d j (FTName T') d) =
+        Topen_d j (FTName T') (Topen_d i (FTName T) d).
+  Proof.
+    introv Hneq. unfolds Topen_d.
+    induction~ d. destruct a. rew_listx. rewrite~ IHd.
+    destruct t ; solve_var.
+  Qed.
+
+  Lemma Topen_k_Topen_comm :
+    forall i j T T' k,
+      i <> j ->
+      Topen_k i (FTName T) (Topen_k j (FTName T') k) =
+        Topen_k j (FTName T') (Topen_k i (FTName T) k).
+  Proof. introv Hneq. solve_eq k ; apply~ Topen_d_Topen_comm. Qed.
+
+  Lemma Topen_ty_Topen_comm :
+    forall i j T T' ty,
+      i <> j ->
+      Topen_ty i (FTName T) (Topen_ty j (FTName T') ty) =
+        Topen_ty j (FTName T') (Topen_ty i (FTName T) ty).
+  Proof.
+    introv Hneq. solve_eq ty.
+    - apply~ Topen_k_Topen_comm.
+    - destruct t ; solve_var.
+    - apply~ Topen_d_Topen_comm.
+  Qed.
+
+  Lemma Topen_t_Topen_comm :
+    forall i j T T' t,
+      i <> j ->
+      Topen_t i (FTName T) (Topen_t j (FTName T') t) =
+        Topen_t j (FTName T') (Topen_t i (FTName T) t).
+  Proof.
+    introv Hneq. gen i j. solve_eq t ;
+      try solve [ apply~ Topen_d_Topen_comm
+                | apply~ Topen_k_Topen_comm
+                | apply~ Topen_ty_Topen_comm ].
+    destruct t0 ; solve_var.
+  Qed.
+
+  Lemma Topen_d_Tclose_comm :
+    forall i j T T' d,
+      i <> j ->
+      T <> T' ->
+      Topen_d i (FTName T) (Tclose_d T' j d) =
+        Tclose_d T' j (Topen_d i (FTName T) d).
+  Proof.
+    introv Hneq1 Hneq2. unfolds Topen_d. unfolds Tclose_d.
+    induction~ d. destruct a. rew_listx. rewrite~ IHd.
+    destruct t ; solve_var.
+  Qed.
+
+  Lemma Topen_k_Tclose_comm :
+    forall i j T T' k,
+      i <> j ->
+      T <> T' ->
+      Topen_k i (FTName T) (Tclose_k T' j k) =
+        Tclose_k T' j (Topen_k i (FTName T) k).
+  Proof. intros. solve_eq k ; apply~ Topen_d_Tclose_comm. Qed.
+
+  Lemma Topen_ty_Tclose_comm :
+    forall i j T T' ty,
+      i <> j ->
+      T <> T' ->
+      Topen_ty i (FTName T) (Tclose_ty T' j ty) =
+        Tclose_ty T' j (Topen_ty i (FTName T) ty).
+  Proof.
+    introv Hneq1 Hneq2. solve_eq ty.
+    - apply~ Topen_k_Tclose_comm.
+    - destruct t ; solve_var.
+    - apply~ Topen_d_Tclose_comm.
+  Qed.
+
+  Lemma Topen_t_Tclose_comm :
+    forall i j T T' t,
+      i <> j ->
+      T <> T' ->
+      Topen_t i (FTName T) (Tclose_t T' j t) = Tclose_t T' j (Topen_t i (FTName T) t).
+  Proof.
+    introv Hneq1 Hneq2. gen i j. solve_eq t ;
+      try solve [ apply~ Topen_d_Tclose_comm
+                | apply~ Topen_k_Tclose_comm
+                | apply~ Topen_ty_Tclose_comm ].
+    destruct t0 ; solve_var.
+  Qed.
+
+  Lemma Kopen_d_Topen_comm :
+    forall i j K T d,
+      Kopen_d i K (Topen_d j T d) = Topen_d j T (Kopen_d i K d).
+  Proof.
+    intros. unfolds Topen_d. unfolds Kopen_d.
+    induction~ d. destruct a. rew_listx. rewrite~ IHd.
+  Qed.
+
+  Lemma Kopen_k_Topen_comm :
+    forall i j K T k,
+      Kopen_k i K (Topen_k j T k) = Topen_k j T (Kopen_k i K k).
+  Proof. intros. solve_eq k ; apply~ Kopen_d_Topen_comm. Qed.
+
+  Lemma Kopen_ty_Topen_comm :
+    forall i j K T ty,
+      Kopen_ty i K (Topen_ty j T ty) = Topen_ty j T (Kopen_ty i K ty).
+  Proof.
+    intros. solve_eq ty.
+    - apply~ Kopen_k_Topen_comm.
+    - apply~ Kopen_d_Topen_comm.
+  Qed.
+
+  Lemma Kopen_t_Topen_comm :
+    forall i j K T t,
+      Kopen_t i K (Topen_t j T t) = Topen_t j T (Kopen_t i K t).
+  Proof.
+    intros. gen i j. solve_eq t ;
+      try solve [ apply~ Kopen_d_Topen_comm
+                | apply~ Kopen_k_Topen_comm
+                | apply~ Kopen_ty_Topen_comm ].
+  Qed.
+
+  Lemma Kopen_d_Tclose_comm :
+    forall i j K T d,
+      Kopen_d i K (Tclose_d T j d) = Tclose_d T j (Kopen_d i K d).
+  Proof.
+    intros. unfolds Tclose_d. unfolds Kopen_d.
+    induction~ d. destruct a. rew_listx. rewrite~ IHd.
+  Qed.
+
+  Lemma Kopen_k_Tclose_comm :
+    forall i j K T k,
+      Kopen_k i K (Tclose_k T j k) = Tclose_k T j (Kopen_k i K k).
+  Proof. intros. solve_eq k ; apply~ Kopen_d_Tclose_comm. Qed.
+
+  Lemma Kopen_ty_Tclose_comm :
+    forall i j K T ty,
+      Kopen_ty i K (Tclose_ty T j ty) = Tclose_ty T j (Kopen_ty i K ty).
+  Proof.
+    intros. solve_eq ty.
+    - apply~ Kopen_k_Tclose_comm.
+    - apply~ Kopen_d_Tclose_comm.
+  Qed.
+
+  Lemma Kopen_t_Tclose_comm :
+    forall i j K T t,
+      Kopen_t i K (Tclose_t T j t) = Tclose_t T j (Kopen_t i K t).
+  Proof.
+    intros. gen i j. solve_eq t ;
+      try solve [ apply~ Kopen_d_Tclose_comm
+                | apply~ Kopen_k_Tclose_comm
+                | apply~ Kopen_ty_Tclose_comm ].
+  Qed.
+
+  Lemma open_inj :
+    forall i x t1 t2,
+      x \notin fv t1 \u fv t2 ->
+      [i ~> TmFVar x] t1 = [i ~> TmFVar x] t2 ->
+      t1 = t2.
+  Proof.
+    introv Hfv Heq. gen i t2.
+    solve_eq t1 ; destruct t2 ; inverts Heq ; solve_var ; fequals*.
+    - inverts H0. notin_false.
+  Qed.
+
+  Lemma topen_inj :
+    forall i x ty1 ty2,
+      x \notin tfv ty1 \u tfv ty2 ->
+      {i ~> TyFVar x} ty1 = {i ~> TyFVar x} ty2 ->
+      ty1 = ty2.
+  Proof.
+    introv Hfv Heq. gen i ty2.
+    solve_eq ty1 ; destruct ty2 ; inverts Heq ; solve_var ; fequals*.
+    - inverts H0. notin_false.
+  Qed.
+
+  Lemma topen_t_inj :
+    forall i x t1 t2,
+      x \notin tfv_t t1 \u tfv_t t2 ->
+      [{i ~> TyFVar x}] t1 = [{i ~> TyFVar x}] t2 ->
+      t1 = t2.
+  Proof.
+    introv Hfv Heq. gen i t2.
+    solve_eq t1 ; destruct t2 ; inverts Heq ; solve_var ; fequals* ;
+      rewrite_all notin_union in Hfv ; apply* topen_inj.
+  Qed.
+
+  Lemma Topen_d_inj :
+    forall i X d1 d2,
+      X \notin Tfv_d d1 \u Tfv_d d2 ->
+      Topen_d i (FTName X) d1 = Topen_d i (FTName X) d2 ->
+      d1 = d2.
+  Proof.
+    introv. gen d2. unfolds Topen_d. unfolds Tfv_d.
+    induction d1 ; introv Hfv Heq ; destruct d2 ; inverts~ Heq.
+    destruct a ; destruct p ; rew_listx in *. rewrite~ (IHd1 d2).
+    do 2 fequals. inverts H0.
+    destruct t ; destruct t0 ; solve_var ; inverts H2 ; notin_false.
+  Qed.
+
+  Lemma Topen_k_inj :
+    forall i X k1 k2,
+      X \notin Tfv_k k1 \u Tfv_k k2 ->
+      Topen_k i (FTName X) k1 = Topen_k i (FTName X) k2 ->
+      k1 = k2.
+  Proof.
+    introv Hfv Heq. gen k2.
+    solve_eq k1 ; destruct k2 ; inverts Heq ; fequals ; apply* Topen_d_inj.
+  Qed.
+
+  Lemma Topen_ty_inj :
+    forall i X ty1 ty2,
+      X \notin Tfv_ty ty1 \u Tfv_ty ty2 ->
+      Topen_ty i (FTName X) ty1 = Topen_ty i (FTName X) ty2 ->
+      ty1 = ty2.
+  Proof.
+    introv Hfv Heq. gen i ty2.
+    solve_eq ty1 ; destruct ty2 ; inverts Heq ; solve_var ; fequals* ;
+      rewrite_all notin_union in Hfv.
+    - apply* Topen_k_inj.
+    - destruct Hfv as ((?&Hfv1)&(?&Hfv2)).
+      destruct t ; destruct t0 ; solve_var ; inverts H1 ; notin_false.
+    - apply* Topen_d_inj.
+  Qed.
+
+  Lemma Topen_t_inj :
+    forall i X t1 t2,
+      X \notin Tfv_t t1 \u Tfv_t t2 ->
+      Topen_t i (FTName X) t1 = Topen_t i (FTName X) t2 ->
+      t1 = t2.
+  Proof.
+    introv Hfv Heq. gen i t2.
+    solve_eq t1 ; destruct t2 ; inverts Heq ; solve_var ; fequals* ;
+      rewrite_all notin_union in Hfv ;
+      try solve [ apply* Topen_d_inj
+                | apply* Topen_k_inj
+                | apply* Topen_ty_inj ].
+    destruct Hfv as ((?&?&Hfv1&?)&(?&?&Hfv2&?)).
+    destruct t0 ; destruct t3 ; solve_var ; inverts H2 ; notin_false.
+  Qed.
+
+  Lemma Kopen_d_inj :
+    forall i X d1 d2,
+      X \notin Kfv_d d1 \u Kfv_d d2 ->
+      Kopen_d i (FCon X) d1 = Kopen_d i (FCon X) d2 ->
+      d1 = d2.
+  Proof.
+    introv. gen d2. unfolds Kopen_d. unfolds Kfv_d.
+    induction d1 ; introv Hfv Heq ; destruct d2 ; inverts~ Heq.
+    destruct a ; destruct p ; rew_listx in *.
+    fequals~. fequals. inverts H0.
+    gen l0. induction l ; introv Hfv Heq ; destruct l0 ; inverts~ Heq.
+    rew_listx in *. fequals~.
+    destruct a ; destruct c ; solve_var ; inverts H0 ; notin_false.
+  Qed.
+
+  Lemma Kopen_k_inj :
+    forall i X k1 k2,
+      X \notin Kfv_k k1 \u Kfv_k k2 ->
+      Kopen_k i (FCon X) k1 = Kopen_k i (FCon X) k2 ->
+      k1 = k2.
+  Proof.
+    introv Hfv Heq. gen k2.
+    solve_eq k1 ; destruct k2 ; inverts Heq ; fequals ; apply* Kopen_d_inj.
+  Qed.
+
+  Lemma Kopen_ty_inj :
+    forall i X ty1 ty2,
+      X \notin Kfv_ty ty1 \u Kfv_ty ty2 ->
+      Kopen_ty i (FCon X) ty1 = Kopen_ty i (FCon X) ty2 ->
+      ty1 = ty2.
+  Proof.
+    introv Hfv Heq. gen i ty2.
+    solve_eq ty1 ; destruct ty2 ; inverts Heq ; solve_var ; fequals* ;
+      rewrite_all notin_union in Hfv.
+    - apply* Kopen_k_inj.
+    - apply* Kopen_d_inj.
+  Qed.
+
+  Lemma Kopen_t_inj :
+    forall i X t1 t2,
+      X \notin Kfv_t t1 \u Kfv_t t2 ->
+      Kopen_t i (FCon X) t1 = Kopen_t i (FCon X) t2 ->
+      t1 = t2.
+  Proof.
+    introv Hfv Heq. gen i t2.
+    solve_eq t1 ; destruct t2 ; inverts Heq ; solve_var ; fequals* ;
+      rewrite_all notin_union in Hfv ;
+      try solve [ apply* Kopen_d_inj
+                | apply* Kopen_k_inj
+                | apply* Kopen_ty_inj ].
+    destruct Hfv as ((Hfv1&?&?)&(Hfv2&?&?)).
+    destruct c ; destruct c0 ; solve_var ; inverts H0 ; notin_false.
+  Qed.
+
+  Lemma Topen_d_Tclose :
+    forall i T d,
+      lcd d ->
+      Topen_d i (FTName T) (Tclose_d T i d) = d.
+  Proof.
+    introv Hlc. unfolds lcd. unfolds Topen_d. unfolds Tclose_d.
+    induction~ Hlc. rew_listx. destruct x. do 2 fequals.
+    destruct H as (HlcT&?).
+    destruct t ; solve_var ; inverts HlcT ; discriminate.
+  Qed.
+
+  Lemma Topen_k_Tclose :
+    forall i T k,
+      lck k ->
+      Topen_k i (FTName T) (Tclose_k T i k) = k.
+  Proof. introv Hlc. solve_eq Hlc. apply~ Topen_d_Tclose. Qed.
+
+  Lemma Topen_ty_Tclose :
+    forall i T ty,
+      lct ty ->
+      Topen_ty i (FTName T) (Tclose_ty T i ty) = ty.
+  Proof.
+    introv Hlc. solve_eq Hlc.
+    - apply~ Topen_k_Tclose.
+    - remember (Topen_ty i (FTName T) (Tclose_ty T i T0)).
+      pick_fresh X ; substs. applys~ topen_inj 0 X.
+      rewrite* <- Topen_ty_topen_comm. rewrite* <- Tclose_ty_topen_comm. simpls~.
+    - apply~ Topen_d_Tclose.
+  Qed.
+
+  Lemma Topen_t_Tclose :
+    forall i T t,
+      lc t ->
+      Topen_t i (FTName T) (Tclose_t T i t) = t.
+  Proof.
+    introv Hlc. gen i.
+    induction Hlc ; intros ; simpls ; fequals* ;
+      try solve [ apply~ Topen_d_Tclose
+                | apply~ Topen_k_Tclose
+                | apply~ Topen_ty_Tclose ].
+    - remember (Topen_t i (FTName T) (Tclose_t T i t)).
+      pick_fresh x ; substs. applys~ open_inj 0 x.
+      rewrite* <- Topen_t_open_comm. rewrite* <- Tclose_t_open_comm. simpls~.
+    - remember (Topen_t i (FTName T) (Tclose_t T i t)).
+      pick_fresh x ; substs. applys~ topen_t_inj 0 x.
+      rewrite* <- Topen_t_topen_comm. rewrite* <- Tclose_t_topen_comm. simpls~.
+    - remember (Topen_t (S i) (FTName T) (Tclose_t T (S i) t)).
+      pick_fresh X ; substs. applys~ Topen_t_inj 0 X.
+      rewrite~ Topen_t_Topen_comm. rewrite~ Topen_t_Tclose_comm.
+    - remember (Topen_ty i (FTName T) (Tclose_ty T i ty)).
+      pick_fresh X ; substs. applys~ topen_inj 0 X.
+      rewrite* <- Topen_ty_topen_comm. rewrite~ <- Tclose_ty_topen_comm ; simpls~.
+      apply* Topen_ty_Tclose.
+    - solve_var.
+    - remember (Topen_t i (FTName T) (Tclose_t T i t)).
+      pick_fresh X ; substs. applys~ Kopen_t_inj 0 X.
+      rewrite~ Kopen_t_Topen_comm. rewrite~ Kopen_t_Tclose_comm.
+    - remember (Topen_t i (FTName T) (Tclose_t T i t)).
+      pick_fresh x ; substs. applys~ open_inj 0 x.
+      rewrite* <- Topen_t_open_comm. rewrite* <- Tclose_t_open_comm. simpls~.
+  Qed.
+
+  Lemma Tclose_d_notin : forall T i d, T \notin Tfv_d (Tclose_d T i d).
+  Proof.
+    intros. unfolds Tclose_d. unfolds Tfv_d.
+    induction d ; rew_listx~. destruct a. rewrite notin_union. splits~.
+    destruct t ; solve_var.
+  Qed.
+
+  Lemma Tclose_k_notin : forall T i k, T \notin Tfv_k (Tclose_k T i k).
+  Proof. intros. induction k ; simpls~. apply~ Tclose_d_notin. Qed.
+
+  Lemma Tclose_ty_notin : forall T i ty, T \notin Tfv_ty (Tclose_ty T i ty).
+  Proof.
+    intros.
+    induction ty ; intros ; solve_var ; rewrite_all notin_union ; try split~.
+    - apply~ Tclose_k_notin.
+    - destruct t ; solve_var.
+    - apply~ Tclose_d_notin.
+  Qed.
+
+  Lemma Tclose_t_notin : forall T i t, T \notin Tfv_t (Tclose_t T i t).
+  Proof.
+    intros. gen i.
+    induction t ; intros ; solve_var ; rewrite_all notin_union ; splits~ ;
+      try solve [ apply~ Tclose_d_notin
+                | apply~ Tclose_k_notin
+                | apply~ Tclose_ty_notin ].
+    destruct t0 ; solve_var.
+  Qed.
+
+  Lemma Kopen_t_open_comm :
+    forall i n K v t,
+      lc v ->
+      Kopen_t i K ([n ~> v] t) = [n ~> v] (Kopen_t i K t).
+  Proof.
+    introv Hlc. gen n i. solve_eq t. apply* Kopen_t_lc.
+  Qed.
+
+  Lemma Kclose_d_fresh :
+    forall K i d,
+      K \notin Kfv_d d ->
+      Kclose_d K i d = d.
+  Proof.
+    introv Hfv. unfolds Kclose_d. unfolds Kfv_d.
+    induction~ d.
+    rew_listx in *. destruct a. do 2 fequals~.
+    induction~ l. rew_listx in *. fequals~.
+    destruct a ; solve_var.
+  Qed.
+
+  Lemma Kclose_k_fresh :
+    forall K i k,
+      K \notin Kfv_k k ->
+      Kclose_k K i k = k.
+  Proof. introv Hfv. solve_eq k ; apply~ Kclose_d_fresh. Qed.
+
+  Lemma Kclose_ty_fresh :
+    forall K i ty,
+      K \notin Kfv_ty ty ->
+      Kclose_ty K i ty = ty.
+  Proof.
+    introv Hfv. solve_eq ty.
+    - apply~ Kclose_k_fresh.
+    - apply~ Kclose_d_fresh.
+  Qed.
+
+  Lemma Kclose_t_fresh :
+    forall K i t,
+      K \notin Kfv_t t ->
+      Kclose_t K i t = t.
+  Proof.
+    introv Hfv. gen i. solve_eq t ;
+      try solve [ apply~ Kclose_d_fresh
+                | apply~ Kclose_k_fresh
+                | apply~ Kclose_ty_fresh ].
+    destruct c ; solve_var.
+  Qed.
+
+  Lemma Kclose_t_open_comm :
+    forall i n K v t,
+      K \notin Kfv_t v ->
+      Kclose_t K i ([n ~> v] t) = [n ~> v] (Kclose_t K i t).
+  Proof.
+    introv. gen i n. solve_eq t ; apply* Kclose_t_fresh.
+  Qed.
+
+  Lemma Kopen_ty_topen_comm :
+    forall i n K ty1 ty2,
+      lct ty1 ->
+      Kopen_ty i K ({n ~> ty1} ty2) = {n ~> ty1} (Kopen_ty i K ty2).
+  Proof.
+    introv. gen n. solve_eq ty2. apply* Kopen_ty_lct.
+  Qed.
+
+  Lemma Kopen_t_topen_comm :
+    forall i n K ty t,
+      lct ty ->
+      Kopen_t i K ([{n ~> ty}] t) = [{n ~> ty}] (Kopen_t i K t).
+  Proof.
+    introv. gen n i. solve_eq t ; apply* Kopen_ty_topen_comm.
+  Qed.
+
+  Lemma Kclose_ty_topen_comm :
+    forall i n K ty1 ty2,
+      K \notin Kfv_ty ty1 ->
+      Kclose_ty K i ({n ~> ty1} ty2) = {n ~> ty1} (Kclose_ty K i ty2).
+  Proof.
+    introv. gen n. solve_eq ty2 ; apply* Kclose_ty_fresh.
+  Qed.
+
+  Lemma Kclose_t_topen_comm :
+    forall i n K ty t,
+      K \notin Kfv_ty ty ->
+      Kclose_t K i ([{n ~> ty}] t) = [{n ~> ty}] (Kclose_t K i t).
+  Proof.
+    introv. gen n i. solve_eq t ; apply* Kclose_ty_topen_comm.
+  Qed.
+
+  Lemma Kopen_d_Kopen_comm :
+    forall i j K K' d,
+      i <> j ->
+      Kopen_d i (FCon K) (Kopen_d j (FCon K') d) =
+        Kopen_d j (FCon K') (Kopen_d i (FCon K) d).
+  Proof.
+    introv Hneq. unfolds Kopen_d.
+    induction~ d. destruct a. rew_listx. do 2 fequals~.
+    induction~ l. rew_listx. fequals~.
+    destruct a ; solve_var.
+  Qed.
+
+  Lemma Kopen_k_Kopen_comm :
+    forall i j K K' k,
+      i <> j ->
+      Kopen_k i (FCon K) (Kopen_k j (FCon K') k) =
+        Kopen_k j (FCon K') (Kopen_k i (FCon K) k).
+  Proof. introv Hneq. solve_eq k ; apply~ Kopen_d_Kopen_comm. Qed.
+
+  Lemma Kopen_ty_Kopen_comm :
+    forall i j K K' ty,
+      i <> j ->
+      Kopen_ty i (FCon K) (Kopen_ty j (FCon K') ty) =
+        Kopen_ty j (FCon K') (Kopen_ty i (FCon K) ty).
+  Proof.
+    introv Hneq. solve_eq ty.
+    - apply~ Kopen_k_Kopen_comm.
+    - apply~ Kopen_d_Kopen_comm.
+  Qed.
+
+  Lemma Kopen_t_Kopen_comm :
+    forall i j K K' t,
+      i <> j ->
+      Kopen_t i (FCon K) (Kopen_t j (FCon K') t) =
+        Kopen_t j (FCon K') (Kopen_t i (FCon K) t).
+  Proof.
+    introv Hneq. gen i j. solve_eq t ;
+      try solve [ apply~ Kopen_d_Kopen_comm
+                | apply~ Kopen_k_Kopen_comm
+                | apply~ Kopen_ty_Kopen_comm ].
+    destruct c ; solve_var.
+  Qed.
+
+  Lemma Kopen_d_Kclose_comm :
+    forall i j K K' d,
+      i <> j ->
+      K <> K' ->
+      Kopen_d i (FCon K) (Kclose_d K' j d) =
+        Kclose_d K' j (Kopen_d i (FCon K) d).
+  Proof.
+    introv Hneq1 Hneq2. unfolds Kopen_d. unfolds Kclose_d.
+    induction~ d. destruct a. rew_listx. do 2 fequals~.
+    induction~ l. rew_listx. fequals~.
+    destruct a ; solve_var.
+  Qed.
+
+  Lemma Kopen_k_Kclose_comm :
+    forall i j K K' k,
+      i <> j ->
+      K <> K' ->
+      Kopen_k i (FCon K) (Kclose_k K' j k) =
+        Kclose_k K' j (Kopen_k i (FCon K) k).
+  Proof. intros. solve_eq k ; apply~ Kopen_d_Kclose_comm. Qed.
+
+  Lemma Kopen_ty_Kclose_comm :
+    forall i j K K' ty,
+      i <> j ->
+      K <> K' ->
+      Kopen_ty i (FCon K) (Kclose_ty K' j ty) =
+        Kclose_ty K' j (Kopen_ty i (FCon K) ty).
+  Proof.
+    introv Hneq1 Hneq2. solve_eq ty.
+    - apply~ Kopen_k_Kclose_comm.
+    - apply~ Kopen_d_Kclose_comm.
+  Qed.
+
+  Lemma Kopen_t_Kclose_comm :
+    forall i j K K' t,
+      i <> j ->
+      K <> K' ->
+      Kopen_t i (FCon K) (Kclose_t K' j t) = Kclose_t K' j (Kopen_t i (FCon K) t).
+  Proof.
+    introv Hneq1 Hneq2. gen i j. solve_eq t ;
+      try solve [ apply~ Kopen_d_Kclose_comm
+                | apply~ Kopen_k_Kclose_comm
+                | apply~ Kopen_ty_Kclose_comm ].
+    destruct c ; solve_var.
+  Qed.
+
+  Lemma Kopen_d_Kclose :
+    forall i K d,
+      lcd d ->
+      Kopen_d i (FCon K) (Kclose_d K i d) = d.
+  Proof.
+    introv Hlc. unfolds lcd. unfolds Kopen_d. unfolds Kclose_d.
+    induction~ Hlc. rew_listx. destruct x. do 2 fequals.
+    destruct H as (?&HlcK).
+    induction~ l0. rew_listx in *. fequals*. destruct HlcK as (HlcK'&?).
+    destruct a ; solve_var ; inverts HlcK' ; discriminate.
+  Qed.
+
+  Lemma Kopen_k_Kclose :
+    forall i K k,
+      lck k ->
+      Kopen_k i (FCon K) (Kclose_k K i k) = k.
+  Proof. introv Hlc. solve_eq Hlc. apply~ Kopen_d_Kclose. Qed.
+
+  Lemma Kopen_ty_Kclose :
+    forall i K ty,
+      lct ty ->
+      Kopen_ty i (FCon K) (Kclose_ty K i ty) = ty.
+  Proof.
+    introv Hlc. solve_eq Hlc.
+    - apply~ Kopen_k_Kclose.
+    - remember (Kopen_ty i (FCon K) (Kclose_ty K i T)).
+      pick_fresh X ; substs. applys~ topen_inj 0 X.
+      rewrite* <- Kopen_ty_topen_comm. rewrite* <- Kclose_ty_topen_comm. simpls~.
+    - apply~ Kopen_d_Kclose.
+  Qed.
+
+  Lemma Topen_d_Kclose_comm :
+    forall i j K T d,
+      Topen_d i T (Kclose_d K j d) = Kclose_d K j (Topen_d i T d).
+  Proof.
+    intros. unfolds Kclose_d. unfolds Topen_d.
+    induction~ d. destruct a. rew_listx. fequals~.
+  Qed.
+
+  Lemma Topen_k_Kclose_comm :
+    forall i j K T k,
+      Topen_k i T (Kclose_k K j k) = Kclose_k K j (Topen_k i T k).
+  Proof. intros. solve_eq k ; apply~ Topen_d_Kclose_comm. Qed.
+
+  Lemma Topen_ty_Kclose_comm :
+    forall i j K T ty,
+      Topen_ty i T (Kclose_ty K j ty) = Kclose_ty K j (Topen_ty i T ty).
+  Proof.
+    intros. solve_eq ty.
+    - apply~ Topen_k_Kclose_comm.
+    - apply~ Topen_d_Kclose_comm.
+  Qed.
+
+  Lemma Topen_t_Kclose_comm :
+    forall i j K T t,
+      Topen_t i T (Kclose_t K j t) = Kclose_t K j (Topen_t i T t).
+  Proof.
+    intros. gen i j. solve_eq t ;
+      try solve [ apply~ Topen_d_Kclose_comm
+                | apply~ Topen_k_Kclose_comm
+                | apply~ Topen_ty_Kclose_comm ].
+  Qed.
+
+  Lemma Kopen_t_Kclose :
+    forall i K t,
+      lc t ->
+      Kopen_t i (FCon K) (Kclose_t K i t) = t.
+  Proof.
+    introv Hlc. gen i.
+    induction Hlc ; intros ; simpls ; fequals* ;
+      try solve [ apply~ Kopen_d_Kclose
+                | apply~ Kopen_k_Kclose
+                | apply~ Kopen_ty_Kclose ].
+    - remember (Kopen_t i (FCon K) (Kclose_t K i t)).
+      pick_fresh x ; substs. applys~ open_inj 0 x.
+      rewrite* <- Kopen_t_open_comm. rewrite* <- Kclose_t_open_comm. simpls~.
+    - remember (Kopen_t i (FCon K) (Kclose_t K i t)).
+      pick_fresh x ; substs. applys~ topen_t_inj 0 x.
+      rewrite* <- Kopen_t_topen_comm. rewrite* <- Kclose_t_topen_comm. simpls~.
+    - solve_var.
+    - remember (Kopen_t i (FCon K) (Kclose_t K i t)).
+      pick_fresh X ; substs. applys~ Topen_t_inj 0 X.
+      rewrite~ <- Kopen_t_Topen_comm. rewrite~ Topen_t_Kclose_comm.
+    - remember (Kopen_ty i (FCon K) (Kclose_ty K i ty)).
+      pick_fresh X ; substs. applys~ topen_inj 0 X.
+      rewrite* <- Kopen_ty_topen_comm. rewrite~ <- Kclose_ty_topen_comm ; simpls~.
+      apply* Kopen_ty_Kclose.
+    - remember (Kopen_t (S i) (FCon K) (Kclose_t K (S i) t)).
+      pick_fresh X ; substs. applys~ Kopen_t_inj 0 X.
+      rewrite~ Kopen_t_Kopen_comm. rewrite~ Kopen_t_Kclose_comm.
+    - remember (Kopen_t i (FCon K) (Kclose_t K i t)).
+      pick_fresh x ; substs. applys~ open_inj 0 x.
+      rewrite* <- Kopen_t_open_comm. rewrite* <- Kclose_t_open_comm. simpls~.
+  Qed.
+
+  Lemma Kclose_d_notin : forall K i d, K \notin Kfv_d (Kclose_d K i d).
+  Proof.
+    intros. unfolds Kclose_d. unfolds Kfv_d.
+    induction d ; rew_listx~. destruct a. rewrite notin_union. splits~.
+    induction l ; rew_listx~.
+    rewrite notin_union. splits~. destruct a ; solve_var.
+  Qed.
+
+  Lemma Kclose_k_notin : forall K i k, K \notin Kfv_k (Kclose_k K i k).
+  Proof. intros. induction k ; simpls~. apply~ Kclose_d_notin. Qed.
+
+  Lemma Kclose_ty_notin : forall K i ty, K \notin Kfv_ty (Kclose_ty K i ty).
+  Proof.
+    intros.
+    induction ty ; intros ; solve_var ; rewrite_all notin_union ; try split~.
+    - apply~ Kclose_k_notin.
+    - apply~ Kclose_d_notin.
+  Qed.
+
+  Lemma Kclose_t_notin : forall K i t, K \notin Kfv_t (Kclose_t K i t).
+  Proof.
+    intros. gen i.
+    induction t ; intros ; solve_var ; rewrite_all notin_union ; splits~ ;
+      try solve [ apply~ Kclose_d_notin
+                | apply~ Kclose_k_notin
+                | apply~ Kclose_ty_notin ].
+    destruct c ; solve_var.
+  Qed.
+
+  Lemma Tsubst_t_open_distr :
+    forall i X T t u,
+      Tsubst_t X T ([i ~> u] t) =
+        [i ~> Tsubst_t X T u] (Tsubst_t X T t).
+  Proof. introv. gen i. solve_eq t. Qed.
+
+  Lemma Tsubst_ty_topen_distr :
+    forall i X T ty U,
+      Tsubst_ty X T ({i ~> U} ty) =
+        {i ~> Tsubst_ty X T U} (Tsubst_ty X T ty).
+  Proof. introv. gen i. solve_eq ty. Qed.
+
+  Lemma Tsubst_t_topen_distr :
+    forall i X T t U,
+      Tsubst_t X T ([{i ~> U}] t) =
+        [{i ~> Tsubst_ty X T U}] (Tsubst_t X T t).
+  Proof. introv. gen i. solve_eq t ; apply Tsubst_ty_topen_distr. Qed.
+
+  Lemma Tsubst_t_open_comm :
+    forall i X T t x,
+      Tsubst_t X T ([i ~> TmFVar x] t) = [i ~> TmFVar x] (Tsubst_t X T t).
+  Proof. introv. gen i. solve_eq t. Qed.
+
+  Lemma Tsubst_ty_topen_comm :
+    forall i X T ty x,
+      Tsubst_ty X T ({i ~> TyFVar x} ty) =
+        {i ~> TyFVar x} (Tsubst_ty X T ty).
+  Proof. introv. gen i. solve_eq ty. Qed.
+
+  Lemma Tsubst_t_topen_comm :
+    forall i X T t x,
+      Tsubst_t X T ([{i ~> TyFVar x}] t) = [{i ~> TyFVar x}] (Tsubst_t X T t).
+  Proof. introv. gen i. solve_eq t ; apply Tsubst_ty_topen_comm. Qed.
+
+  Lemma Tsubst_d_Topen_comm :
+    forall i X T U d,
+      X <> T ->
+      Topen_d i (FTName T) (Tsubst_d X (FTName U) d) =
+        Tsubst_d X (FTName U) (Topen_d i (FTName T) d).
+  Proof.
+    introv Hneq. unfolds Topen_d. unfolds Tsubst_d.
+    induction~ d.
+    rew_listx in *. destruct a. rewrite~ IHd. destruct t ; solve_var.
+  Qed.
+
+  Lemma Tsubst_k_Topen_comm :
+    forall i X T U k,
+      X <> T ->
+      Topen_k i (FTName T) (Tsubst_k X (FTName U) k) =
+        Tsubst_k X (FTName U) (Topen_k i (FTName T) k).
+  Proof.
+    introv Hneq. solve_eq k. apply~ Tsubst_d_Topen_comm.
+  Qed.
+
+  Lemma Tsubst_ty_Topen_comm :
+    forall i X T U ty,
+      X <> T ->
+      Topen_ty i (FTName T) (Tsubst_ty X (FTName U) ty) =
+        Tsubst_ty X (FTName U) (Topen_ty i (FTName T) ty).
+  Proof.
+    introv Hneq. solve_eq ty.
+    - apply~ Tsubst_k_Topen_comm.
+    - destruct t ; solve_var.
+    - apply~ Tsubst_d_Topen_comm.
+  Qed.
+
+  Lemma Tsubst_t_Topen_comm :
+    forall i X T U t,
+      X <> T ->
+      Topen_t i (FTName T) (Tsubst_t X (FTName U) t) =
+        Tsubst_t X (FTName U) (Topen_t i (FTName T) t).
+  Proof.
+    introv Hneq. gen i. solve_eq t ;
+      try solve [ apply~ Tsubst_d_Topen_comm
+                | apply~ Tsubst_k_Topen_comm
+                | apply~ Tsubst_ty_Topen_comm ].
+    destruct t0 ; solve_var.
+  Qed.
+
+  Lemma Tsubst_d_Kopen_comm :
+    forall i X K U d,
+      Kopen_d i (FCon K) (Tsubst_d X (FTName U) d) =
+        Tsubst_d X (FTName U) (Kopen_d i (FCon K) d).
+  Proof.
+    intros. unfolds Kopen_d. unfolds Tsubst_d.
+    induction~ d.
+    rew_listx in *. destruct a. rewrite~ IHd.
+  Qed.
+
+  Lemma Tsubst_k_Kopen_comm :
+    forall i X K U k,
+      Kopen_k i (FCon K) (Tsubst_k X (FTName U) k) =
+        Tsubst_k X (FTName U) (Kopen_k i (FCon K) k).
+  Proof. intros. solve_eq k. apply~ Tsubst_d_Kopen_comm. Qed.
+
+  Lemma Tsubst_ty_Kopen_comm :
+    forall i X K U ty,
+      Kopen_ty i (FCon K) (Tsubst_ty X (FTName U) ty) =
+        Tsubst_ty X (FTName U) (Kopen_ty i (FCon K) ty).
+  Proof.
+    intros. solve_eq ty.
+    - apply~ Tsubst_k_Kopen_comm.
+    - apply~ Tsubst_d_Kopen_comm.
+  Qed.
+
+  Lemma Tsubst_t_Kopen_comm :
+    forall i X K U t,
+      Kopen_t i (FCon K) (Tsubst_t X (FTName U) t) =
+        Tsubst_t X (FTName U) (Kopen_t i (FCon K) t).
+  Proof.
+    introv. gen i. solve_eq t ;
+      try solve [ apply~ Tsubst_d_Kopen_comm
+                | apply~ Tsubst_k_Kopen_comm
+                | apply~ Tsubst_ty_Kopen_comm ].
+  Qed.
+
+  Lemma Tsubst_d_intro :
+    forall X U i d,
+      X \notin Tfv_d d ->
+      Topen_d i U d = Tsubst_d X U (Topen_d i (FTName X) d).
+  Proof.
+    introv Hfv. unfolds Topen_d. unfolds Tsubst_d. unfolds Tfv_d.
+    induction~ d.
+    rew_listx in *. destruct a. rewrite~ IHd. destruct t ; solve_var.
+  Qed.
+
+  Lemma Tsubst_k_intro :
+    forall X U i k,
+      X \notin Tfv_k k ->
+      Topen_k i U k = Tsubst_k X U (Topen_k i (FTName X) k).
+  Proof. introv Hfv. solve_eq k. apply~ Tsubst_d_intro. Qed.
+
+  Lemma Tsubst_ty_intro :
+    forall X U i ty,
+      X \notin Tfv_ty ty ->
+      Topen_ty i U ty = Tsubst_ty X U (Topen_ty i (FTName X) ty).
+  Proof.
+    introv Hfv. solve_eq ty.
+    - apply~ Tsubst_k_intro.
+    - destruct t ; solve_var.
+    - apply~ Tsubst_d_intro.
+  Qed.
+
+  Lemma Tsubst_t_intro :
+    forall X U i t,
+      X \notin Tfv_t t ->
+      Topen_t i U t = Tsubst_t X U (Topen_t i (FTName X) t).
+  Proof.
+    introv Hfv. gen i. solve_eq t ;
+      try solve [ apply~ Tsubst_d_intro
+                | apply~ Tsubst_k_intro
+                | apply~ Tsubst_ty_intro ].
+    destruct t0 ; solve_var.
+  Qed.
+
+  Lemma Ksubst_t_open_distr :
+    forall i X K t u,
+      Ksubst_t X K ([i ~> u] t) =
+        [i ~> Ksubst_t X K u] (Ksubst_t X K t).
+  Proof. introv. gen i. solve_eq t. Qed.
+
+  Lemma Ksubst_ty_topen_distr :
+    forall i X K ty U,
+      Ksubst_ty X K ({i ~> U} ty) =
+        {i ~> Ksubst_ty X K U} (Ksubst_ty X K ty).
+  Proof. introv. gen i. solve_eq ty. Qed.
+
+  Lemma Ksubst_t_topen_distr :
+    forall i X K t U,
+      Ksubst_t X K ([{i ~> U}] t) =
+        [{i ~> Ksubst_ty X K U}] (Ksubst_t X K t).
+  Proof. introv. gen i. solve_eq t ; apply Ksubst_ty_topen_distr. Qed.
+
+  Lemma Ksubst_t_open_comm :
+    forall i X K t x,
+      Ksubst_t X K ([i ~> TmFVar x] t) = [i ~> TmFVar x] (Ksubst_t X K t).
+  Proof. introv. gen i. solve_eq t. Qed.
+
+  Lemma Ksubst_ty_topen_comm :
+    forall i X K ty x,
+      Ksubst_ty X K ({i ~> TyFVar x} ty) =
+        {i ~> TyFVar x} (Ksubst_ty X K ty).
+  Proof. introv. gen i. solve_eq ty. Qed.
+
+  Lemma Ksubst_t_topen_comm :
+    forall i X K t x,
+      Ksubst_t X K ([{i ~> TyFVar x}] t) = [{i ~> TyFVar x}] (Ksubst_t X K t).
+  Proof. introv. gen i. solve_eq t ; apply Ksubst_ty_topen_comm. Qed.
+
+  Lemma Ksubst_d_Kopen_comm :
+    forall i X K U d,
+      X <> K ->
+      Kopen_d i (FCon K) (Ksubst_d X (FCon U) d) =
+        Ksubst_d X (FCon U) (Kopen_d i (FCon K) d).
+  Proof.
+    introv Hneq. unfolds Kopen_d. unfolds Ksubst_d.
+    induction~ d. rew_listx. destruct a. rewrite~ IHd.
+    induction~ l. rew_listx. inverts IHl. rewrite H0. destruct a ; solve_var.
+  Qed.
+
+  Lemma Ksubst_k_Kopen_comm :
+    forall i X K U k,
+      X <> K ->
+      Kopen_k i (FCon K) (Ksubst_k X (FCon U) k) =
+        Ksubst_k X (FCon U) (Kopen_k i (FCon K) k).
+  Proof.
+    introv Hneq. solve_eq k. apply~ Ksubst_d_Kopen_comm.
+  Qed.
+
+  Lemma Ksubst_ty_Kopen_comm :
+    forall i X K U ty,
+      X <> K ->
+      Kopen_ty i (FCon K) (Ksubst_ty X (FCon U) ty) =
+        Ksubst_ty X (FCon U) (Kopen_ty i (FCon K) ty).
+  Proof.
+    introv Hneq. solve_eq ty.
+    - apply~ Ksubst_k_Kopen_comm.
+    - apply~ Ksubst_d_Kopen_comm.
+  Qed.
+
+  Lemma Ksubst_t_Kopen_comm :
+    forall i X K U t,
+      X <> K ->
+      Kopen_t i (FCon K) (Ksubst_t X (FCon U) t) =
+        Ksubst_t X (FCon U) (Kopen_t i (FCon K) t).
+  Proof.
+    introv Hneq. gen i. solve_eq t ;
+      try solve [ apply~ Ksubst_d_Kopen_comm
+                | apply~ Ksubst_k_Kopen_comm
+                | apply~ Ksubst_ty_Kopen_comm ].
+    destruct c ; solve_var.
+  Qed.
+
+  Lemma Ksubst_d_Topen_comm :
+    forall i X T U d,
+      Topen_d i (FTName T) (Ksubst_d X (FCon U) d) =
+        Ksubst_d X (FCon U) (Topen_d i (FTName T) d).
+  Proof.
+    intros. unfolds Topen_d. unfolds Ksubst_d.
+    induction~ d.
+    rew_listx in *. destruct a. rewrite~ IHd.
+  Qed.
+
+  Lemma Ksubst_k_Topen_comm :
+    forall i X T U k,
+      Topen_k i (FTName T) (Ksubst_k X (FCon U) k) =
+        Ksubst_k X (FCon U) (Topen_k i (FTName T) k).
+  Proof. intros. solve_eq k. apply~ Ksubst_d_Topen_comm. Qed.
+
+  Lemma Ksubst_ty_Topen_comm :
+    forall i X T U ty,
+      Topen_ty i (FTName T) (Ksubst_ty X (FCon U) ty) =
+        Ksubst_ty X (FCon U) (Topen_ty i (FTName T) ty).
+  Proof.
+    intros. solve_eq ty.
+    - apply~ Ksubst_k_Topen_comm.
+    - apply~ Ksubst_d_Topen_comm.
+  Qed.
+
+  Lemma Ksubst_t_Topen_comm :
+    forall i X T U t,
+      Topen_t i (FTName T) (Ksubst_t X (FCon U) t) =
+        Ksubst_t X (FCon U) (Topen_t i (FTName T) t).
+  Proof.
+    introv. gen i. solve_eq t ;
+      try solve [ apply~ Ksubst_d_Topen_comm
+                | apply~ Ksubst_k_Topen_comm
+                | apply~ Ksubst_ty_Topen_comm ].
+  Qed.
+
+  Lemma Ksubst_d_intro :
+    forall X U i d,
+      X \notin Kfv_d d ->
+      Kopen_d i U d = Ksubst_d X U (Kopen_d i (FCon X) d).
+  Proof.
+    introv Hfv. unfolds Kopen_d. unfolds Ksubst_d. unfolds Kfv_d.
+    induction~ d. rew_listx in *. destruct a. rewrite~ IHd.
+    induction~ l. rew_listx in Hfv. rew_listx.
+    forwards~ IHl': IHl. inverts IHl'.
+    rewrite H0. destruct a ; solve_var.
+  Qed.
+
+  Lemma Ksubst_k_intro :
+    forall X U i k,
+      X \notin Kfv_k k ->
+      Kopen_k i U k = Ksubst_k X U (Kopen_k i (FCon X) k).
+  Proof. introv Hfv. solve_eq k. apply~ Ksubst_d_intro. Qed.
+
+  Lemma Ksubst_ty_intro :
+    forall X U i ty,
+      X \notin Kfv_ty ty ->
+      Kopen_ty i U ty = Ksubst_ty X U (Kopen_ty i (FCon X) ty).
+  Proof.
+    introv Hfv. solve_eq ty.
+    - apply~ Ksubst_k_intro.
+    - apply~ Ksubst_d_intro.
+  Qed.
+
+  Lemma Ksubst_t_intro :
+    forall X U i t,
+      X \notin Kfv_t t ->
+      Kopen_t i U t = Ksubst_t X U (Kopen_t i (FCon X) t).
+  Proof.
+    introv Hfv. gen i. solve_eq t ;
+      try solve [ apply~ Ksubst_d_intro
+                | apply~ Ksubst_k_intro
+                | apply~ Ksubst_ty_intro ].
+    destruct c ; solve_var.
+  Qed.
+
+  Lemma Tsubst_d_fresh :
+    forall T U d,
+      T \notin Tfv_d d ->
+      Tsubst_d T U d = d.
+  Proof.
+    introv Hfv. unfolds. unfolds Tfv_d.
+    induction~ d. destruct a.
+    rew_listx in *. do 2 fequals~. destruct t ; solve_var.
+  Qed.
+
+  Lemma Tsubst_k_fresh :
+    forall T U k,
+      T \notin Tfv_k k ->
+      Tsubst_k T U k = k.
+  Proof. introv Hfv. solve_eq k. apply~ Tsubst_d_fresh. Qed.
+
+  Lemma Tsubst_ty_fresh :
+    forall T U ty,
+      T \notin Tfv_ty ty ->
+      Tsubst_ty T U ty = ty.
+  Proof.
+    introv Hfv. solve_eq ty.
+    - apply~ Tsubst_k_fresh.
+    - destruct t ; solve_var.
+    - apply~ Tsubst_d_fresh.
+  Qed.
+
+  Lemma notin_Topen_d :
+    forall i T d,
+      T \notin Tfv_d (Topen_d i (FTName T) d) ->
+      Topen_d i (FTName T) d = d.
+  Proof.
+    introv Hfv. unfolds Topen_d. unfolds Tfv_d.
+    induction~ d. destruct a.
+    rew_listx in *. do 2 fequals~. destruct t ; solve_var.
+  Qed.
+
+  Lemma notin_Topen_k :
+    forall i T k,
+      T \notin Tfv_k (Topen_k i (FTName T) k) ->
+      Topen_k i (FTName T) k = k.
+  Proof.
+    introv Hfv. induction k ; simpls ; fequals.
+    apply~ notin_Topen_d.
+  Qed.
+
+  Lemma notin_Topen_ty :
+    forall i T ty,
+      T \notin Tfv_ty (Topen_ty i (FTName T) ty) ->
+      Topen_ty i (FTName T) ty = ty.
+  Proof.
+    introv Hfv.
+    induction ty ; simpls ; fequals*.
+    - apply~ notin_Topen_k.
+    - destruct t ; solve_var.
+    - apply~ notin_Topen_d.
+  Qed.
+
+  Lemma open_notin_T :
+    forall i x T t,
+      T \notin Tfv_t ([i ~> TmFVar x]t) = T \notin Tfv_t t.
+  Proof.
+    intros. rew_logic. splits ; gen i.
+    { induction t ; introv Hfv ; simpls ; rewrite_all notin_union in Hfv ; solve_var. }
+    { induction t ; introv Hfv ; simpls ; solve_var. }
+  Qed.
+
+  Lemma topen_notin_T :
+    forall T i ty1 ty2,
+      T \notin Tfv_ty ty1 ->
+      T \notin Tfv_ty ({i ~> ty1}ty2) = T \notin Tfv_ty ty2.
+  Proof.
+    intros. rew_logic. splits ; gen i.
+    { induction ty2 ; introv Hfv ; simpls ; rewrite_all notin_union in Hfv ; solve_var. }
+    { induction ty2 ; introv Hfv ; solve_var. }
+  Qed.
+
+  Lemma topen_t_notin_T :
+    forall i x T t,
+      T \notin Tfv_t ([{i ~> TyFVar x}]t) = T \notin Tfv_t t.
+  Proof.
+    intros. rew_logic. splits ; gen i.
+    { induction t ; introv Hfv ; simpls ; rewrite_all notin_union in Hfv ;
+        try rewrite topen_notin_T in Hfv; solve_var. }
+    { induction t ; introv Hfv ; simpls ; rewrite_all notin_union ; solve_var ;
+        try rewrite topen_notin_T ; simpls~. }
+  Qed.
+
+  Lemma Tsubst_inj :
+    forall S S' T T',
+      T' <> S ->
+      T' <> S' ->
+      Tsubst T (FTName T') (FTName S) = Tsubst T (FTName T') (FTName S') ->
+      S = S'.
+  Proof.
+    introv Hneq1 Hneq2 Heq.
+    solve_var ; inverts~ Heq.
+  Qed.
+
+  Lemma Ksubst_d_fresh :
+    forall K U d,
+      K \notin Kfv_d d ->
+      Ksubst_d K U d = d.
+  Proof.
+    introv Hfv. unfolds. unfolds Kfv_d.
+    induction~ d. destruct a.
+    rew_listx in *. do 2 fequals~.
+    induction~ l. rew_listx in *. fequals~.
+    destruct a ; solve_var.
+  Qed.
+
+  Lemma Ksubst_k_fresh :
+    forall K U k,
+      K \notin Kfv_k k ->
+      Ksubst_k K U k = k.
+  Proof. introv Hfv. solve_eq k. apply~ Ksubst_d_fresh. Qed.
+
+  Lemma Ksubst_ty_fresh :
+    forall K U ty,
+      K \notin Kfv_ty ty ->
+      Ksubst_ty K U ty = ty.
+  Proof.
+    introv Hfv. solve_eq ty.
+    - apply~ Ksubst_k_fresh.
+    - apply~ Ksubst_d_fresh.
+  Qed.
+
+  Lemma notin_Kopen_d :
+    forall i K d,
+      K \notin Kfv_d (Kopen_d i (FCon K) d) ->
+      Kopen_d i (FCon K) d = d.
+  Proof.
+    introv Hfv. unfolds Kopen_d. unfolds Kfv_d.
+    induction~ d. destruct a.
+    rew_listx in *. do 2 fequals~.
+    induction~ l. rew_listx in *. fequals~.
+    destruct a ; solve_var.
+  Qed.
+
+  Lemma notin_Kopen_k :
+    forall i K k,
+      K \notin Kfv_k (Kopen_k i (FCon K) k) ->
+      Kopen_k i (FCon K) k = k.
+  Proof.
+    introv Hfv. induction k ; simpls ; fequals.
+    apply~ notin_Kopen_d.
+  Qed.
+
+  Lemma notin_Kopen_ty :
+    forall i K ty,
+      K \notin Kfv_ty (Kopen_ty i (FCon K) ty) ->
+      Kopen_ty i (FCon K) ty = ty.
+  Proof.
+    introv Hfv.
+    induction ty ; simpls ; fequals*.
+    - apply~ notin_Kopen_k.
+    - apply~ notin_Kopen_d.
+  Qed.
+
+  Lemma open_notin_K :
+    forall i x K t,
+      K \notin Kfv_t ([i ~> TmFVar x]t) = K \notin Kfv_t t.
+  Proof.
+    intros. rew_logic. splits ; gen i.
+    { induction t ; introv Hfv ; simpls ; rewrite_all notin_union in Hfv ; solve_var. }
+    { induction t ; introv Hfv ; simpls ; solve_var. }
+  Qed.
+
+  Lemma topen_notin_K :
+    forall K i ty1 ty2,
+      K \notin Kfv_ty ty1 ->
+      K \notin Kfv_ty ({i ~> ty1}ty2) = K \notin Kfv_ty ty2.
+  Proof.
+    intros. rew_logic. splits ; gen i.
+    { induction ty2 ; introv Hfv ; simpls ; rewrite_all notin_union in Hfv ; solve_var. }
+    { induction ty2 ; introv Hfv ; solve_var. }
+  Qed.
+
+  Lemma topen_t_notin_K :
+    forall i x K t,
+      K \notin Kfv_t ([{i ~> TyFVar x}]t) = K \notin Kfv_t t.
+  Proof.
+    intros. rew_logic. splits ; gen i.
+    { induction t ; introv Hfv ; simpls ; rewrite_all notin_union in Hfv ;
+        try rewrite topen_notin_K in Hfv; solve_var. }
+    { induction t ; introv Hfv ; simpls ; rewrite_all notin_union ; solve_var ;
+        try rewrite topen_notin_K ; simpls~. }
+  Qed.
+
+  Lemma topen_topen_comm :
+    forall i j u1 u2 ty,
+      i <> j ->
+      lct u1 -> lct u2 ->
+      {i ~> u1} ({j ~> u2} ty) = {j ~> u2} ({i ~> u1} ty).
+  Proof.
+    introv Hneq Hlct1 Hlct2. gen i j.
+    solve_eq ty ; rewrite~ topen_lct.
+  Qed.
+
+  Lemma Ksubst_inj :
+    forall S S' K K',
+      K' <> S ->
+      K' <> S' ->
+      Ksubst K (FCon K') (FCon S) = Ksubst K (FCon K') (FCon S') ->
+      S = S'.
+  Proof.
+    introv Hneq1 Hneq2 Heq.
+    solve_var ; inverts~ Heq.
+  Qed.
+
+End SyntaxProps.
