src/TypingProps.v
@@ -1,0 +1,1460 @@
+From TLC Require Import LibString LibList LibLN.
+From MCore Require Import Syntax SyntaxProps Typing Tactics.
+Import LibListNotation.
+
+(**************************)
+(** PROPERTIES OF TYPING **)
+(**************************)
+
+Module TypingProps (P : PAT).
+  Module T := Typing P.
+  Export T.
+
+  Module TypingProps1 (PC : PATCHECK).
+    Module T1 := Typing1 PC.
+    Export T1.
+
+    Module Type PATCHECKPROPS.
+      Parameter ok_pat_ok_type :
+        forall Gamma p T T',
+          ok_pat Gamma p T T' ->
+          Gamma |= T' ~:: KiType.
+
+      Parameter ok_pat_weakening :
+        forall G3 G1 G2 p T T',
+          ok_pat (G1 & G3) p T T' ->
+          ok_env (G1 & G2 & G3) ->
+          ok_pat (G1 & G2 & G3) p T T'.
+
+      Parameter ok_pat_strengthening :
+        forall G1 G2 x p T1 T1' T2,
+          ok_pat (G1 & x ~ BindVar T2 & G2) p T1 T1' ->
+          ok_pat (G1 & G2) p T1 T1'.
+
+      Parameter ok_pat_bsubst :
+        forall G1 G2 p X U T T',
+          ok_pat (G1 & G2) p T T' ->
+          ok_pat (G1 & map (bsubst X U) G2) p ({X => U}T) ({X => U}T').
+
+      Parameter ok_pat_tvar_strengthening :
+        forall G1 G2 x k p T T',
+          ok_pat (G1 & x ~ BindTVar k & G2) p T T' ->
+          ok_pat (G1 & G2) p T T'.
+
+      Parameter pats_compatible_tsubst :
+        forall ps X U ty,
+          pats_compatible ps ty ->
+          pats_compatible ps ({X => U} ty).
+
+      Parameter pats_exhaustive_tsubst :
+        forall ps X U ty,
+          pats_exhaustive ps ty ->
+          pats_exhaustive ps ({X => U} ty).
+
+      Parameter ok_pat_comm :
+        forall G1 G2 x1 x2 b1 b2 p T T',
+          ok_pat (G1 & x1 ~ b1 & x2 ~ b2 & G2) p T T' ->
+          ok_env (G1 & x2 ~ b2 & x1 ~ b1 & G2) ->
+          ok_pat (G1 & x2 ~ b2 & x1 ~ b1 & G2) p T T'.
+
+      Parameter ok_pat_tname_strengthening :
+        forall T G2 G1 ty ty' p,
+          T \notin Tfv_ty ty ->
+          ok_pat (G1 & T ~ BindTName & G2) p ty ty' ->
+          ok_pat (G1 & G2) p ty ty'.
+
+      Parameter ok_pat_Tsubst :
+        forall G2 G1 T T' p ty ty',
+          ok_pat (G1 & T ~ BindTName & G2) p ty ty' ->
+          T' # G1 & T ~ BindTName & G2 ->
+          ok_env (G1 & T ~ BindTName & G2) ->
+          ok_pat (G1 & T' ~ BindTName & map (Tbsubst T (FTName T')) G2)
+                 p (Tsubst_ty T (FTName T') ty) (Tsubst_ty T (FTName T') ty').
+
+      Parameter pats_compatible_Tsubst :
+        forall ps T T' ty,
+          pats_compatible ps ty ->
+          pats_compatible ps (Tsubst_ty T (FTName T') ty).
+
+      Parameter pats_exhaustive_Tsubst :
+        forall ps T T' ty,
+          pats_exhaustive ps ty ->
+          pats_exhaustive ps (Tsubst_ty T (FTName T') ty).
+
+      Parameter ok_pat_con_strengthening :
+        forall K G2 G1 d0 ty0 T ty ty' p,
+          K \notin Kfv_ty ty ->
+          ok_pat (G1 & K ~ BindCon d0 ty0 T & G2) p ty ty' ->
+          ok_pat (G1 & G2) p ty ty'.
+
+      Parameter ok_pat_Ksubst :
+        forall G2 G1 K K' d0 ty0 T p ty ty',
+          ok_pat (G1 & K ~ BindCon d0 ty0 T & G2) p ty ty' ->
+          K' # G1 & K ~ BindCon d0 ty0 T & G2 ->
+          ok_env (G1 & K ~ BindCon d0 ty0 T & G2) ->
+          ok_pat (G1 & K' ~ BindCon d0 ty0 T & map (Kbsubst K (FCon K')) G2)
+                 p (Ksubst_ty K (FCon K') ty) (Ksubst_ty K (FCon K') ty').
+
+      Parameter pats_compatible_Ksubst :
+        forall ps K K' ty,
+          pats_compatible ps ty ->
+          pats_compatible ps (Ksubst_ty K (FCon K') ty).
+
+      Parameter pats_exhaustive_Ksubst :
+        forall ps K K' ty,
+          pats_exhaustive ps ty ->
+          pats_exhaustive ps (Ksubst_ty K (FCon K') ty).
+
+    End PATCHECKPROPS.
+
+    Module TypingProps2 (PCP : PATCHECKPROPS).
+      Export PCP.
+
+      Lemma ok_env_ok :
+        forall Gamma,
+          ok_env Gamma ->
+          ok Gamma.
+      Proof. introv Henv ; induction* Henv. Qed.
+      #[export]
+       Hint Resolve ok_env_ok : mcore.
+
+      Lemma ok_data_weakening :
+        forall G3 G1 G2 d,
+          ok_data (G1 & G3) d ->
+          ok_env  (G1 & G2 & G3) ->
+          ok_data (G1 & G2 & G3) d.
+      Proof.
+        introv Hd Henv.
+        remember (G1 & G3) as Gamma eqn:HGamma.
+        assert (Hok : ok (G1 & G2)) by applys* ok_concat_inv_l G3.
+        induction Hd ; constructor*.
+        - substs ; apply* binds_weaken.
+        - induction H1 ; substs ; constructors*.
+          apply* binds_weaken.
+      Qed.
+
+      Lemma ok_kind_weakening :
+        forall G3 G1 G2 k,
+          ok_kind (G1 & G3) k ->
+          ok_env  (G1 & G2 & G3) ->
+          ok_kind (G1 & G2 & G3) k.
+      Proof.
+        introv Hk.
+        remember (G1 & G3) as Gamma eqn:HGamma.
+        destruct Hk; subst*. constructor. apply* ok_data_weakening.
+      Qed.
+
+      Lemma ok_type_weakening :
+        forall G3 G1 G2 T k,
+          G1 & G3 |= T ~:: k ->
+          ok_env (G1 & G2 & G3) ->
+          G1 & G2 & G3 |= T ~:: k.
+      Proof.
+        introv Htk Henv.
+        remember (G1 & G3) as Gamma. gen G3.
+        induction* Htk; intros; substs.
+        { Case "TyFVar". constructors*. apply* binds_weaken. }
+        { Case "TyAll". apply_fresh* KAll. apply* ok_kind_weakening.
+          apply_ih_bind* H1.
+          constructor*. apply* ok_kind_weakening. }
+        { Case "TyData". constructors*. apply* ok_data_weakening. }
+      Qed.
+
+      Lemma ok_env_ok_type :
+        forall Gamma x T,
+          ok_env Gamma ->
+          binds x (BindVar T) Gamma ->
+          Gamma |= T ~:: KiType.
+      Proof.
+        introv Henv Hbind.
+        induction* Henv ; try (binds_cases Hbind ; apply_empty* ok_type_weakening).
+        { Case "EnvEmpty". false. apply* binds_empty_inv. }
+        { Case "EnvVar". inverts* EQ. }
+      Qed.
+
+      Lemma ok_data_lcd : forall Gamma d, ok_data Gamma d -> lcd d.
+      Proof.
+        introv Hd. unfolds.
+        induction Hd ; rew_listx*. splits*. splits*.
+        induction H1 ; rew_listx*.
+      Qed.
+      #[export]
+       Hint Resolve ok_data_lcd : mcore.
+
+      Lemma ok_kind_lck : forall Gamma k, ok_kind Gamma k -> lck k.
+      Proof. introv Hk. destruct* Hk. Qed.
+      #[export]
+       Hint Resolve ok_kind_lck : mcore.
+
+      Lemma ok_type_lct :
+        forall Gamma T k,
+          Gamma |= T ~:: k ->
+          lct T.
+      Proof. introv Htk ; induction* Htk. Qed.
+      #[export]
+       Hint Resolve ok_type_lct : mcore.
+
+      Lemma ok_term_lct :
+        forall Gamma t T,
+          Gamma |= t ~: T ->
+          lct T.
+      Proof with eauto using ok_env_ok_type, ok_type_lct.
+        introv hasType.
+        induction* hasType...
+        { Case "TmLam". constructors...
+          pick_fresh_gen L y... }
+        { Case "TmApp". inverts* IHhasType1. }
+        { Case "TmTyLam". inverts* IHhasType.
+          assert(Hlct: lct ty2)...
+          pick_fresh X. rewrite *(tsubst_intro X).
+          apply* tsubst_lct. }
+        { Case "TmFix". inverts* IHhasType. }
+        { Case "TmProj1". inverts* IHhasType. }
+        { Case "TmProj2". inverts* IHhasType. }
+        { Case "TmType". pick_fresh T. applys~ H0 T. }
+        { Case "TmConDef". pick_fresh K. applys~ H3 K. }
+        { Case "TmSem". constructors...
+          pick_fresh_gen L y... }
+        { Case "TmComp". inverts* IHhasType1. }
+        { Case "TmSemApp". inverts* IHhasType1. }
+      Qed.
+      #[export]
+       Hint Resolve ok_term_lct : mcore.
+
+      Lemma ok_term_lc :
+        forall Gamma t T,
+          Gamma |= t ~: T ->
+          lc t.
+      Proof. introv Htype; induction* Htype. Qed.
+      #[export]
+       Hint Resolve ok_term_lc : mcore.
+
+      Lemma ok_env_push :
+        forall G1 x b,
+          ok_env (G1 & x ~ b) ->
+          ok_env G1.
+      Proof.
+        introv Henv. inverts Henv ;
+          try (apply eq_push_inv in H; inverts H as []; substs~).
+        false. apply *empty_push_inv.
+      Qed.
+
+      Lemma ok_type_ok_env :
+        forall Gamma T k,
+          Gamma |= T ~:: k ->
+          ok_env Gamma.
+      Proof.
+        introv hasType.
+        induction* hasType ; pick_fresh_gen L x; eauto using ok_env_push.
+      Qed.
+      #[export]
+       Hint Resolve ok_type_ok_env : mcore.
+
+      Lemma ok_term_ok_env :
+        forall Gamma t T,
+          Gamma |= t ~: T ->
+          ok_env Gamma.
+      Proof.
+        introv hasType.
+        induction* hasType; pick_fresh_gen L x;
+          eauto using ok_env_push.
+      Qed.
+      #[export]
+       Hint Resolve ok_term_ok_env : mcore.
+
+      Lemma ok_term_weakening :
+        forall G3 G2 G1 t T,
+          G1 & G3 |= t ~: T ->
+          ok_env (G1 & G2 & G3) ->
+          G1 & G2 & G3 |= t ~: T.
+      Proof with eauto using ok_type_weakening, ok_kind_weakening, ok_data_weakening with mcore.
+        introv hasType Henv. remember (G1 & G3) as H. gen G3.
+        induction hasType; intros; substs...
+        { Case "TmFVar". constructors~. apply* binds_weaken. }
+        { Case "TmLam". apply_fresh* TLam as y...
+          apply_ih_bind H1 ; auto. constructor... }
+        { Case "TmTyLam". apply_fresh* TTyLam as X...
+          apply_ih_bind H1 ; auto. constructor... }
+        { Case "TmCon". constructors...
+          apply* binds_weaken. }
+        { Case "TmType". apply_fresh TType as T...
+          apply_ih_bind H0 ; auto. constructor... }
+        { Case "TmConDef". apply_fresh TConDef as K...
+          - apply_ih_bind ok_type_weakening...
+          - apply* binds_weaken.
+          - apply_ih_bind H3 ; auto.
+            apply_fresh EnvCon as X...
+            + apply_ih_bind ok_type_weakening...
+            + apply* binds_weaken. }
+        { Case "TmSem". apply_fresh* TSem as y... apply* ok_pat_weakening.
+          apply_ih_bind H2 ; auto. constructor...
+          apply~ ok_type_weakening. apply* ok_pat_ok_type. }
+      Qed.
+
+      Lemma ok_data_strengthening :
+        forall G1 G2 x T d,
+          ok_data (G1 & x ~ BindVar T & G2) d ->
+          ok_data (G1 & G2) d.
+      Proof.
+        introv Hd.
+        remember (G1 & x ~ BindVar T & G2) as Gamma.
+        induction Hd ; constructor*.
+        - substs ; binds_cases H0 ; auto.
+        - induction* H1 ; substs ; constructors*.
+          binds_cases H3 ; eauto.
+      Qed.
+
+      Lemma ok_kind_strengthening :
+        forall G1 G2 x T k,
+          ok_kind (G1 & x ~ BindVar T & G2) k ->
+          ok_kind (G1 & G2) k.
+      Proof.
+        introv Hk. remember (G1 & x ~ BindVar T & G2) as G.
+        destruct Hk ; substs*. constructor. apply* ok_data_strengthening.
+      Qed.
+
+      Lemma ok_type_strengthening :
+        forall G1 G2 x T1 T2 k,
+          G1 & x ~ BindVar T2 & G2 |= T1 ~:: k ->
+          ok_env (G1 & G2) ->
+          G1 & G2 |= T1 ~:: k.
+      Proof.
+        introv Htk. remember (G1 & x ~ BindVar T2 & G2) as G. gen G2.
+        induction Htk; intros; substs*.
+        { Case "TyFVar". constructors*.
+          binds_cases H0 ; auto. }
+        { Case "TyAll". apply_fresh* KAll as X.
+          apply* ok_kind_strengthening.
+          apply_ih_bind* H1. constructor*. apply* ok_kind_strengthening. }
+        { Case "TyData". constructor*. apply* ok_data_strengthening. }
+      Qed.
+
+      Lemma ok_env_con_inv :
+        forall Gamma K d ty T,
+          ok_env (Gamma & K ~ BindCon d ty T) ->
+          exists L T',
+            T = FTName T'
+            /\ ok_data Gamma d
+            /\ (forall X, X \notin L -> Gamma & X ~ BindTVar (KiData d) |= {0 ~> TyFVar X}ty ~:: KiType)
+            /\ binds T' BindTName Gamma.
+      Proof.
+        introv Henv.
+        inverts Henv ; try (apply eq_push_inv in H as (? & ? & ?)) ; try discriminate.
+        - false. apply* empty_push_inv.
+        - substs ; inverts* H5. exists* L T0.
+      Qed.
+
+      Lemma ok_env_tvar_inv :
+        forall Gamma X k,
+          ok_env (Gamma & X ~ BindTVar k) ->
+          ok_kind Gamma k.
+      Proof.
+        introv Henv.
+        inverts Henv ; try (apply eq_push_inv in H as (? & ? & ?); substs* ; fequals).
+        false. apply* empty_push_inv.
+      Qed.
+
+      Lemma ok_env_var_inv :
+        forall Gamma x T,
+          ok_env (Gamma & x ~ BindVar T) ->
+          Gamma |= T ~:: KiType.
+      Proof.
+        introv Henv.
+        inverts Henv ; try (apply eq_push_inv in H as (? & ? & ?); substs* ; fequals).
+        false. apply* empty_push_inv.
+      Qed.
+
+      Lemma ok_env_strengthening :
+        forall G1 x T G3,
+          ok_env (G1 & x ~ BindVar T & G3) ->
+          ok_env (G1 & G3).
+      Proof.
+        introv Henv. induction G3 using env_ind.
+        { Case "Empty". rewrite concat_empty_r in *. apply* ok_env_push. }
+        { Case "Push". rewrite concat_assoc in *.
+          specializes IHG3 (ok_env_push _ _ _ Henv).
+          lets [? Hdisj] : ok_push_inv (ok_env_ok _ Henv).
+          destruct v.
+          { SCase "BindTName". constructor~. }
+          { SCase "BindCon". forwards (L & T' & Heq & Hd & Htk & HT): ok_env_con_inv Henv.
+            substs. apply_fresh* EnvCon as K.
+            - apply* ok_data_strengthening.
+            - apply_ih_bind ok_type_strengthening ; eauto.
+              constructor~. constructor~. apply* ok_data_strengthening.
+            - binds_cases HT ; auto. }
+          { SCase "BindTVar". forwards Hk: ok_env_tvar_inv Henv.
+            constructor~. applys ok_kind_strengthening Hk. }
+          { SCase "BindVar". forwards Htk: ok_env_var_inv Henv.
+            constructor~. applys* ok_type_strengthening Htk. }
+          (* { SCase "BindMatch". constructor~. } *)
+        }
+      Qed.
+
+      Lemma ok_term_subst :
+        forall G2 G1 x T1 T2 t1 t2,
+          G1 & x ~ BindVar T2 & G2 |= t1 ~: T1 ->
+          G1 |= t2 ~: T2 ->
+          G1 & G2 |= [x => t2]t1 ~: T1.
+      Proof with eauto using ok_data_strengthening, ok_kind_strengthening,
+          ok_type_strengthening, ok_env_strengthening with mcore.
+        introv hasType1 hasType2.
+        remember (G1 & x ~ BindVar T2 & G2) as G. gen G2.
+        induction hasType1; intros; simpls; substs...
+        { Case "TmFVar". solve_var.
+          - binds_get H0... apply_empty ok_term_weakening...
+          - binds_cases H0... }
+        { Case "TmLam". apply_fresh* TLam as y...
+          rewrite subst_open_comm... apply_ih_bind* H1. }
+        { Case "TmTyLam". apply_fresh* TTyLam as X...
+          rewrite* topen_t_subst_comm. apply_ih_bind* H1. }
+        { Case "TmTyApp". constructors... }
+        { Case "TmCon". constructors... binds_cases H ; auto. }
+        { Case "TmType". apply_fresh* TType as T...
+          rewrite* Topen_t_subst_comm. apply_ih_bind* H0. }
+        { Case "TmConDef". apply_fresh* TConDef as K...
+          - apply_ih_bind ok_type_strengthening ; eauto. constructor...
+          - binds_cases H1; auto.
+          - rewrite* Kopen_t_subst_comm. apply_ih_bind* H3. }
+        { Case "TmSem". apply_fresh* TSem as y...
+          - apply* ok_pat_strengthening.
+          - rewrite subst_open_comm... apply_ih_bind* H2. }
+      Qed.
+
+      Lemma ok_data_tvar_strengthening :
+        forall G1 G2 x k d,
+          ok_data (G1 & x ~ BindTVar k & G2) d ->
+          ok_data (G1 & G2) d.
+      Proof.
+        introv Hd.
+        remember (G1 & x ~ BindTVar k & G2) as Gamma.
+        induction Hd ; constructor*.
+        - substs ; binds_cases H0 ; auto.
+        - induction* H1 ; substs ; constructors*.
+          binds_cases H3 ; eauto.
+      Qed.
+
+      Lemma ok_data_bsubst :
+        forall G1 G2 X T d,
+          ok_data (G1 & G2) d ->
+          ok_data (G1 & map (bsubst X T) G2) d.
+      Proof.
+        introv Hd.
+        remember (G1 & G2) as Gamma.
+        induction Hd ; constructor*.
+        - substs ; binds_cases H0 ; auto.
+          replaces BindTName with (bsubst X T BindTName) ; auto.
+        - induction* H1 ; substs.
+          binds_cases H3 ; constructors*.
+          replaces (BindCon d0 ({X => T} ty) T1) with (bsubst X T (BindCon d0 ty T1)) ; auto.
+      Qed.
+
+      Lemma ok_kind_tvar_strengthening :
+        forall G1 G2 x k' k,
+          ok_kind (G1 & x ~ BindTVar k' & G2) k ->
+          ok_kind (G1 & G2) k.
+      Proof.
+        introv Hk. remember (G1 & x ~ BindTVar k' & G2) as Gamma.
+        destruct* Hk. constructor. substs. apply* ok_data_tvar_strengthening.
+      Qed.
+
+      Lemma ok_kind_bsubst :
+        forall G1 G2 X T k,
+          ok_kind (G1 & G2) k ->
+          ok_kind (G1 & map (bsubst X T) G2) k.
+      Proof.
+        introv Hk. remember (G1 & G2) as Gamma.
+        destruct* Hk. constructor. substs. apply* ok_data_bsubst.
+      Qed.
+
+      Lemma ok_type_tsubst :
+        forall G1 G2 X T1 T2 k k',
+          G1 & X ~ BindTVar k' & G2 |= T1 ~:: k ->
+          G1 |= T2 ~:: k' ->
+          ok_env (G1 & map (bsubst X T2) G2) ->
+          G1 & map (bsubst X T2) G2 |= {X => T2} T1 ~:: k.
+      Proof with eauto using ok_data_bsubst, ok_kind_bsubst, ok_type_lct,
+          ok_data_tvar_strengthening, ok_kind_tvar_strengthening with mcore.
+        introv Htk1 Htk2 Henv.
+        remember (G1 & X ~ BindTVar k' & G2) as G. gen G2.
+        induction Htk1; intros; substs; simpls...
+        { Case "TyFVar". solve_var.
+          + binds_get H0. lets* [Hok ?] : ok_concat_inv (ok_env_ok _ Henv).
+            apply_empty* ok_type_weakening.
+          + constructors~. binds_cases H0...
+            replaces (BindTVar k) with (bsubst X T2 (BindTVar k))... }
+        { Case "TyAll". apply_fresh KAll... rewrite tsubst_topen_comm...
+          replaces (BindTVar k) with (bsubst X T2 (BindTVar k))...
+          apply_ih_map_bind H1 ; auto. constructor... }
+      Qed.
+
+      Lemma bsubst_ok_env :
+        forall G1 G2 X T2 k,
+          G1 |= T2 ~:: k ->
+          ok_env (G1 & X ~ BindTVar k & G2) ->
+          ok_env (G1 & map (bsubst X T2) G2).
+      Proof with eauto using ok_data_bsubst, ok_kind_bsubst, ok_type_lct,
+          ok_data_tvar_strengthening, ok_kind_tvar_strengthening with mcore.
+        introv Htk Henv.
+        induction G2 using env_ind.
+        { Case "Empty". autorewrite with rew_env_map rew_env_concat in *.
+          apply* ok_env_push. }
+        { Case "Push". autorewrite with rew_env_map rew_env_concat in *.
+          specializes IHG2 (ok_env_push _ _ _ Henv).
+          lets [? Hdisj] : ok_push_inv (ok_env_ok _ Henv).
+          destruct v.
+          { SCase "BindTName". constructor~. }
+          { SCase "BindCon". forwards (L & T' & Heq & Hd & Htk' & HT): ok_env_con_inv Henv.
+            substs. apply_fresh EnvCon as K...
+            - replaces (BindTVar (KiData d)) with (bsubst X T2 (BindTVar (KiData d))) ; auto.
+              rewrite tsubst_topen_comm...
+              apply_ih_map_bind ok_type_tsubst ; try rewrite* concat_assoc ; auto.
+              constructor~. constructor...
+            - binds_cases HT ; auto.
+              replaces BindTName with (bsubst X T2 BindTName) ; auto. }
+          { SCase "BindTVar". forwards Hk: ok_env_tvar_inv Henv. constructor... }
+          { SCase "BindVar". forwards Htk': ok_env_var_inv Henv.
+            constructor~. applys* ok_type_tsubst Htk'. }
+          (* { SCase "BindMatch". constructor~. } *)
+        }
+      Qed.
+
+      Lemma ok_env_concat :
+        forall G1 G2,
+          ok_env (G1 & G2) ->
+          ok_env G1.
+      Proof with eauto.
+        introv Henv.
+        induction G2 using env_ind.
+        { Case "Empty". rew_env_concat in *... }
+        { Case "Push". apply IHG2. rew_env_concat in *.
+          apply* ok_env_push. }
+      Qed.
+
+      Lemma ok_type_notin :
+        forall Gamma T k X,
+          Gamma |= T ~:: k ->
+          X # Gamma ->
+          X \notin tfv T.
+      Proof.
+        introv Htk Hfresh.
+        induction Htk; simpls*.
+        { Case "TyFVar". intros contra.
+          rewrite in_singleton in contra. substs.
+          apply get_none in Hfresh.
+          apply binds_get in H0.
+          fequals. }
+        { Case "TyAll". pick_fresh Y.
+          forwards~ Htk: H1 Y.
+          forwards~ Hnin1 : topen_notin Htk. }
+      Qed.
+
+      Lemma env_bsubst_fresh :
+        forall Gamma X T2,
+          ok_env Gamma ->
+          X # Gamma ->
+          Gamma = map (bsubst X T2) Gamma.
+      Proof with eauto using ok_env_push.
+        introv Henv Hfresh.
+        induction Gamma using env_ind.
+        { Case "Empty". rewrite~ map_empty. }
+        { Case "Push". autorewrite with rew_env_map.
+          rewrite <- IHGamma...
+          destruct~ v ; repeat fequals ; unfold bsubst ; rewrite* tsubst_fresh.
+          { SCase "BindCon".
+            apply ok_env_con_inv in Henv as (? & ? & ? & ? & Htk & ?).
+            pick_fresh X'. forwards~ Hnin : ok_type_notin X (Htk X').
+            applys~ topen_notin Hnin. }
+          { SCase "BindVar".
+            apply ok_env_var_inv in Henv.
+            apply* ok_type_notin. } }
+      Qed.
+
+      Lemma ok_term_tsubst :
+        forall G2 G1 t k T1 T2 X,
+          G1 & X ~ BindTVar k & G2 |= t ~: T1 ->
+          G1 |= T2 ~:: k ->
+          G1 & map (bsubst X T2) G2 |= [{X => T2}]t ~: ({X => T2}T1).
+      Proof with eauto using ok_env_strengthening, bsubst_ok_env, ok_type_lct with mcore.
+        introv hasType Henv.
+        remember (G1 & X ~ BindTVar k & G2) as G. gen G2.
+        induction hasType; intros; simpls; substs...
+        { Case "TmFVar". constructor...
+          replaces (BindVar ({X => T2} ty)) with (bsubst X T2 (BindVar ty))...
+          binds_cases H0 ; auto.
+          assert (X # G1) by (applys ok_push_inv ; applys* ok_concat_inv_l G2).
+          rewrite* (env_bsubst_fresh G1 X T2). }
+        { Case "TmLam". apply_fresh* TLam as x.
+          + applys ok_type_tsubst...
+          + replaces (BindVar ({X => T2}ty1)) with (bsubst X T2 (BindVar ty1))...
+            rewrite tsubst_t_open_comm. apply_ih_map_bind H1 ; auto. }
+        { Case "TmTyLam". apply_fresh* TTyLam.
+          + apply ok_kind_bsubst. apply* ok_kind_tvar_strengthening.
+          + replaces (BindTVar k0) with (bsubst X T2 (BindTVar k0))...
+            rewrite tsubst_topen_comm... rewrite topen_t_tsubst_comm...
+            apply_ih_map_bind H1 ; auto. }
+        { Case "TmTyApp".
+          rewrite tsubst_topen_distr... constructors*.
+          apply* ok_type_tsubst. }
+        { Case "TmCon".
+          apply TCon with (d := d) (ty1 := {X => T2}ty1) ; try apply* ok_type_tsubst.
+          - replaces (BindCon d ({X => T2} ty1) (FTName T)) with (bsubst X T2 (BindCon d ty1 (FTName T)))...
+            binds_cases H ; auto.
+            assert (X # G1) by (applys ok_push_inv ; applys* ok_concat_inv_l G2).
+            rewrite* (env_bsubst_fresh G1 X T2).
+          - rewrite <- tsubst_topen_distr... }
+        { Case "TmType". apply_fresh TType.
+          replaces BindTName with (bsubst X T2 BindTName)...
+          rewrite Topen_t_tsubst_comm... apply_ih_map_bind H0 ; auto. }
+        { Case "TmConDef".
+          apply_fresh TConDef.
+          - apply* ok_data_bsubst. apply* ok_data_tvar_strengthening.
+          - replaces (BindTVar (KiData d)) with (bsubst X T2 (BindTVar (KiData d)))...
+            rewrite tsubst_topen_comm...
+            apply_ih_map_bind ok_type_tsubst ; eauto ; try rewrite* concat_assoc.
+            apply_ih_map_bind bsubst_ok_env ; eauto ; try rewrite* concat_assoc.
+          - binds_cases H1 ; auto.
+            replaces BindTName with (bsubst X T2 BindTName) ; auto.
+          - replaces (BindCon d ({X => T2} ty1) (FTName T)) with (bsubst X T2 (BindCon d ty1 (FTName T)))...
+            rewrite Kopen_t_tsubst_comm... apply_ih_map_bind H3 ; auto. }
+        { Case "TmSem". apply_fresh* TSem as x.
+          + applys ok_type_tsubst...
+          + applys* ok_pat_bsubst. applys* ok_pat_tvar_strengthening.
+          + replaces (BindVar ({X => T2}ty1')) with (bsubst X T2 (BindVar ty1'))...
+            rewrite tsubst_t_open_comm. apply_ih_map_bind H2 ; auto. }
+        { Case "TmComp". constructors*. apply~ pats_compatible_tsubst. }
+        { Case "TmSemApp". constructors*. apply~ pats_exhaustive_tsubst. }
+      Qed.
+
+      Lemma ok_data_comm :
+        forall G2 G1 x1 x2 b1 b2 d,
+          ok_data (G1 & x1 ~ b1 & x2 ~ b2 & G2) d ->
+          ok_env (G1 & x2 ~ b2 & x1 ~ b1 & G2) ->
+          ok_data (G1 & x2 ~ b2 & x1 ~ b1 & G2) d.
+      Proof.
+        introv Hd Henv. remember (G1 & x1 ~ b1 & x2 ~ b2 & G2) as Gamma eqn:HGamma.
+        induction Hd ; substs ; constructor~.
+        - binds_cases H0 ; auto.
+          apply* binds_concat_left_ok. apply* binds_concat_left_ok.
+          applys* ok_concat_inv_l G2.
+        - induction* Ks. inverts H1.
+          constructors~. binds_cases H8 ; eauto.
+          apply* binds_concat_left_ok. apply* binds_concat_left_ok.
+          applys* ok_concat_inv_l G2.
+      Qed.
+
+      Lemma ok_kind_comm :
+        forall G2 G1 x1 x2 b1 b2 k,
+          ok_kind (G1 & x1 ~ b1 & x2 ~ b2 & G2) k ->
+          ok_env (G1 & x2 ~ b2 & x1 ~ b1 & G2) ->
+          ok_kind (G1 & x2 ~ b2 & x1 ~ b1 & G2) k.
+      Proof with eauto using ok_data_comm with mcore.
+        introv Hk Henv.
+        remember (G1 & x1 ~ b1 & x2 ~ b2 & G2) as Gamma eqn:HGamma.
+        induction Hk ; substs...
+      Qed.
+
+      Lemma ok_type_comm :
+        forall G2 G1 x1 x2 b1 b2 ty k,
+          G1 & x1 ~ b1 & x2 ~ b2 & G2 |= ty ~:: k ->
+          ok_env (G1 & x2 ~ b2 & x1 ~ b1 & G2) ->
+          G1 & x2 ~ b2 & x1 ~ b1 & G2 |= ty ~:: k.
+      Proof with eauto using ok_data_comm, ok_kind_comm with mcore.
+        introv Htk Henv.
+        remember (G1 & x1 ~ b1 & x2 ~ b2 & G2) as Gamma eqn:HGamma. gen G2.
+        induction Htk ; intros ; substs...
+        { Case "TyFVar". constructor~. binds_cases H0 ; auto.
+          apply* binds_concat_left_ok. apply* binds_concat_left_ok.
+          applys* ok_concat_inv_l G2. }
+        { Case "TyAll". apply_fresh KAll as X...
+          apply_ih_bind H1 ; auto. constructors... }
+      Qed.
+
+      Lemma ok_term_comm :
+        forall G2 G1 x1 x2 b1 b2 t ty,
+          G1 & x1 ~ b1 & x2 ~ b2 & G2 |= t ~: ty ->
+          ok_env (G1 & x2 ~ b2 & x1 ~ b1 & G2) ->
+          G1 & x2 ~ b2 & x1 ~ b1 & G2 |= t ~: ty.
+      Proof with eauto using ok_data_comm, ok_kind_comm, ok_type_comm with mcore.
+        introv Htype Henv.
+        remember (G1 & x1 ~ b1 & x2 ~ b2 & G2) as Gamma eqn:HGamma. gen G2.
+        induction Htype ; intros ; substs...
+        { Case "TmFVar". constructor~. binds_cases H0 ; auto.
+          apply* binds_concat_left_ok. apply* binds_concat_left_ok.
+          applys* ok_concat_inv_l G2. }
+        { Case "TmLam". apply_fresh TLam as x...
+          apply_ih_bind H1 ; auto. constructor... }
+        { Case "TmTyLam". apply_fresh TTyLam as X...
+          apply_ih_bind H1 ; auto. constructor... }
+        { Case "TmCon". constructors... binds_cases H...
+          apply* binds_concat_left_ok. apply* binds_concat_left_ok.
+          applys* ok_concat_inv_l G2. }
+        { Case "TmType". apply_fresh TType as T...
+          apply_ih_bind H0 ; auto. constructor... }
+        { Case "TmConDef".
+          assert (binds T BindTName (G1 & x2 ~ b2 & x1 ~ b1 & G2)).
+          { binds_cases H1...
+            apply* binds_concat_left_ok. apply* binds_concat_left_ok.
+            applys* ok_concat_inv_l G2. }
+          apply_fresh TConDef as X...
+          + apply_ih_bind ok_type_comm. eauto. constructor...
+          + apply_ih_bind H3 ; auto. apply_fresh EnvCon as X'...
+            apply_ih_bind ok_type_comm. eauto. constructor... }
+        { Case "TmLam". apply_fresh TSem as x...
+          + apply* ok_pat_comm.
+          + apply_ih_bind H2 ; auto. constructor... apply~ ok_type_comm. apply* ok_pat_ok_type. }
+      Qed.
+
+      Lemma ok_env_binds_con_inv :
+        forall Gamma K d ty T,
+          ok_env Gamma  ->
+          binds K (BindCon d ty T) Gamma ->
+          exists L T',
+            T = FTName T'
+            /\ ok_data Gamma d
+            /\ (forall X, X \notin L -> Gamma & X ~ BindTVar (KiData d) |= {0 ~> TyFVar X}ty ~:: KiType)
+            /\ binds T' BindTName Gamma.
+      Proof.
+        introv Henv Hbinds.
+        induction Gamma using env_ind.
+        - false. apply* binds_empty_inv.
+        - binds_cases Hbinds.
+          + destruct~ IHGamma as (L & T' & Heq & Hd & Htk & Hbinds'). apply* ok_env_push.
+            exists (L \u dom Gamma \u \{x}) T'. splits*. apply_empty~ ok_data_weakening.
+            introv Hfresh. apply~ ok_type_weakening. constructor~. constructor.
+            apply_empty~ ok_data_weakening. apply* binds_concat_left_ok.
+          + inverts EQ. forwards* (L & T' & Heq & Hd & Htk & Hbinds') : ok_env_con_inv.
+            exists (L \u dom Gamma \u \{K}) T'. splits~. apply_empty~ ok_data_weakening.
+            introv Hfresh. apply~ ok_type_weakening. constructor~. constructor.
+            apply_empty~ ok_data_weakening. apply* binds_concat_left_ok.
+      Qed.
+
+      Lemma ok_env_binds_tvar_inv :
+        forall Gamma X k,
+          ok_env Gamma ->
+          binds X (BindTVar k) Gamma ->
+          ok_kind Gamma k.
+      Proof.
+        introv Henv Hbinds.
+        induction Gamma using env_ind.
+        - false. apply* binds_empty_inv.
+        - binds_cases Hbinds.
+          + apply_empty~ ok_kind_weakening. apply~ IHGamma. apply* ok_env_push.
+          + substs. forwards* Hk: ok_env_tvar_inv. apply_empty~ ok_kind_weakening.
+      Qed.
+
+      Lemma ok_type_ok_kind :
+        forall Gamma T k,
+          Gamma |= T ~:: k ->
+          ok_kind Gamma k.
+      Proof. introv Htk. induction* Htk. apply* ok_env_binds_tvar_inv. Qed.
+
+      Lemma ok_data_tname_strengthening :
+        forall G2 G1 T d,
+          T \notin Tfv_d d ->
+          ok_data (G1 & T ~ BindTName & G2) d ->
+          ok_data (G1 & G2) d.
+      Proof.
+        introv Hfv Hd. remember (G1 & T ~ BindTName & G2) as Gamma eqn:HGamma.
+        unfolds Tfv_d. induction Hd ; substs ; constructor ; rew_listx~ in Hfv.
+        - binds_cases H0 ; auto. notin_false.
+        - induction* Ks. inverts H1.
+          constructors~. binds_cases H8 ; eauto.
+      Qed.
+
+      Lemma ok_kind_tname_strengthening :
+        forall T G2 G1 k,
+          T \notin Tfv_k k ->
+          ok_kind (G1 & T ~ BindTName & G2) k ->
+          ok_kind (G1 & G2) k.
+      Proof with eauto using ok_data_tname_strengthening with mcore.
+        introv Hfv Hk.
+        remember (G1 & T ~ BindTName & G2) as Gamma eqn:HGamma.
+        induction Hk ; substs...
+      Qed.
+
+      Lemma ok_type_tname_strengthening :
+        forall T G2 G1 ty k,
+          T \notin Tfv_ty ty ->
+          G1 & T ~ BindTName & G2 |= ty ~:: k ->
+          ok_env (G1 & G2) ->
+          G1 & G2 |= ty ~:: k.
+      Proof with eauto using ok_data_tname_strengthening, ok_kind_tname_strengthening with mcore.
+        introv Hfv Htk Henv.
+        remember (G1 & T ~ BindTName & G2) as Gamma eqn:HGamma. gen G2.
+        induction Htk ; intros ; simpls ; substs...
+        { Case "TyFVar". constructor~. binds_cases H0 ; auto. }
+        { Case "TyAll". rewrite notin_union in Hfv ; destruct Hfv.
+          apply_fresh KAll as X...
+          apply_ih_bind H1 ; auto. rewrite topen_notin_T ; simpls~. constructors... }
+      Qed.
+
+      Lemma ok_data_notin_T :
+        forall Gamma d X,
+          ok_data Gamma d ->
+          X # Gamma ->
+          X \notin Tfv_d d.
+      Proof.
+        introv Hd Hfresh. unfolds Tfv_d.
+        induction Hd ; rew_listx~.
+        rewrite notin_union. splits*.
+        - rewrite notin_singleton. intro. substs.
+          forwards~ Hin : get_some_inv H0.
+      Qed.
+
+      Lemma ok_kind_notin_T :
+        forall Gamma k X,
+          ok_kind Gamma k ->
+          X # Gamma ->
+          X \notin Tfv_k k.
+      Proof.
+        introv Hk Hfresh. unfolds Tfv_k.
+        destruct~ Hk. apply* ok_data_notin_T.
+      Qed.
+
+      Lemma assoc_data_in :
+        forall d T Ks,
+          mem (FTName T, Ks) d -> T \in Tfv_d d.
+      Proof.
+        introv Hassoc. unfolds Tfv_d.
+        induction Hassoc ; rew_listx~.
+        - rewrite~ in_union. rewrite~ in_singleton.
+        - destruct y. rewrite~ in_union.
+      Qed.
+
+      Lemma ok_type_notin_T :
+        forall Gamma T k X,
+          Gamma |= T ~:: k ->
+          X # Gamma ->
+          X \notin Tfv_ty T.
+      Proof with eauto using ok_data_notin_T, ok_kind_notin_T.
+        introv Htk Hfresh.
+        induction Htk; simpls...
+        { Case "TyAll". rewrite notin_union. splits...
+          pick_fresh Y. forwards~ Htk: H1 Y.
+          rewrite topen_notin_T in Htk ; simpls~. }
+        { Case "TyCon". rewrite notin_union. splits~.
+          forwards Hk: ok_type_ok_kind Htk.
+          forwards~ Hnin : ok_kind_notin_T X Hk.
+          assert (X <> T) by (intro ; substs ; apply Hnin ; applys* assoc_data_in).
+          auto. }
+      Qed.
+
+      Lemma env_Tbsubst_fresh :
+        forall Gamma X T,
+          ok_env Gamma ->
+          X # Gamma ->
+          Gamma = map (Tbsubst X T) Gamma.
+      Proof with eauto using ok_env_push.
+        introv Henv Hfresh.
+        induction Gamma using env_ind.
+        { Case "Empty". rewrite~ map_empty. }
+        { Case "Push". autorewrite with rew_env_map.
+          rewrite <- IHGamma...
+          destruct~ v ; repeat fequals ; unfold Tbsubst.
+          { SCase "BindCon".
+            apply ok_env_con_inv in Henv as (? & ? & ? & ? & Htk & ?). fequals.
+            - rewrite~ Tsubst_d_fresh. forwards~ Hnin : ok_data_notin_T X H0.
+            - rewrite~ Tsubst_ty_fresh. pick_fresh X'.
+              forwards~ Hnin : ok_type_notin_T X (Htk X').
+              rewrite topen_notin_T in Hnin ; simpls~.
+            - destruct t0 ; solve_var. inverts H. forwards* Hin : get_some_inv x1.
+              assert (Hnin: x1 # Gamma) by auto. contradiction. }
+          { SCase "BindTVar".
+            apply ok_env_tvar_inv in Henv. fequals.
+            rewrite~ Tsubst_k_fresh. apply* ok_kind_notin_T. }
+          { SCase "BindVar".
+            apply ok_env_var_inv in Henv. fequals.
+            rewrite~ Tsubst_ty_fresh. apply* ok_type_notin_T. } }
+      Qed.
+
+      Lemma assoc_Tsubst :
+        forall T T' S Ks d,
+          mem (FTName S, Ks) d ->
+          mem (Tsubst T (FTName T') (FTName S), Ks) (Tsubst_d T (FTName T') d).
+      Proof.
+        introv Hassoc. unfolds Tsubst_d.
+        induction Hassoc ; rew_listx~.
+      Qed.
+
+      Lemma assoc_Tsubst_inv :
+        forall Gamma T T' S Ks d,
+          ok_data Gamma d ->
+          T' # Gamma ->
+          T' <> S ->
+          mem (Tsubst T (FTName T') (FTName S), Ks) (Tsubst_d T (FTName T') d) ->
+          mem (FTName S, Ks) d.
+      Proof.
+        introv Hd Hfresh Hneq Hassoc. unfolds Tsubst_d.
+        induction Hd ; inverts Hassoc ; rew_listx~.
+        left. fequals. inverts H0.
+        rewrite~ (Tsubst_inj S T0 T T'). intro Heq ; substs.
+        forwards Hin : get_some_inv T0 ; eauto.
+      Qed.
+
+      Lemma ok_data_Tsubst :
+        forall G2 G1 T T' d,
+          ok_data (G1 & T ~ BindTName & G2) d ->
+          T' # G1 & T ~ BindTName & G2 ->
+          ok_env (G1 & T ~ BindTName & G2) ->
+          ok_data (G1 & T' ~ BindTName & map (Tbsubst T (FTName T')) G2)
+                  (Tsubst_d T (FTName T') d).
+      Proof with eauto with mcore.
+        introv Hd Hfresh Henv. assert (Henv' : ok_env G1)
+          by (applys ok_env_concat ; applys* ok_env_concat).
+        remember (G1 & T ~ BindTName & G2). unfolds Tsubst_d.
+        induction Hd; substs; rew_listx*.
+        asserts (S, Heq): (lcT (Tsubst T (FTName T') (FTName T0))). solve_var.
+        rewrite Heq. constructor~.
+        - rewrite <- Heq. folds (Tsubst_d T (FTName T') d). introv contra.
+          apply (assoc_Tsubst_inv (G1 & T ~ BindTName & G2)) in contra ; jauto.
+          intro ; substs. forwards~ Hin : get_some_inv H0.
+        - solve_var ; inverts~ Heq. binds_cases H0 ; auto.
+          apply~ binds_concat_left. apply binds_concat_left_ok...
+          replaces BindTName with (Tbsubst T (FTName T') BindTName)...
+        - remember (FTName T0). remember (G1 & T ~ BindTName & G2).
+          induction H1 ; substs.
+          + constructor.
+          + apply CCons with (d := Tsubst_d T (FTName T') d0)
+                             (ty := Tsubst_ty T (FTName T') ty) ; auto.
+            replaces (BindCon (Tsubst_d T (FTName T') d0) (Tsubst_ty T (FTName T') ty) (FTName S))
+              with (Tbsubst T (FTName T') (BindCon d0 ty (FTName T0))). rewrite~ <- Heq.
+            binds_cases H3 ; auto.
+            apply~ binds_concat_left. apply binds_concat_left_ok...
+            assert (T # G1). applys ok_push_inv...
+            rewrite~ (env_Tbsubst_fresh G1 T (FTName T'))...
+      Qed.
+
+      Lemma ok_kind_Tsubst :
+        forall G2 G1 T T' k,
+          ok_kind (G1 & T ~ BindTName & G2) k ->
+          ok_env  (G1 & T ~ BindTName & G2) ->
+          T' # G1 & T ~ BindTName & G2 ->
+          ok_kind (G1 & T' ~ BindTName & map (Tbsubst T (FTName T')) G2)
+                  (Tsubst_k T (FTName T') k).
+      Proof.
+        introv Hk. remember (G1 & T ~ BindTName & G2) as G.
+        induction Hk; intros; substs; constructor.
+        apply~ ok_data_Tsubst.
+      Qed.
+
+      Lemma ok_type_Tsubst :
+        forall G2 G1 T T' ty k,
+          G1 & T ~ BindTName & G2 |= ty ~:: k ->
+          T' # G1 & T ~ BindTName & G2 ->
+          ok_env  (G1 & T' ~ BindTName & map (Tbsubst T (FTName T')) G2) ->
+          G1 & T' ~ BindTName &
+            map (Tbsubst T (FTName T')) G2 |=
+                Tsubst_ty T (FTName T') ty ~:: Tsubst_k T (FTName T') k.
+      Proof with eauto with mcore.
+        introv Htk Hfresh Henv. assert (Henv' : ok_env G1)
+          by (applys ok_env_concat ; applys* ok_env_concat).
+        remember (G1 & T ~ BindTName & G2) as G. gen G2.
+        induction Htk; intros; substs; simpls...
+        { Case "TyFVar". constructor...
+          replaces (BindTVar (Tsubst_k T (FTName T') k))
+            with (Tbsubst T (FTName T') (BindTVar k))... binds_cases H0 ; auto.
+          apply~ binds_concat_left. apply* binds_concat_left_ok.
+          assert (T # G1) by (applys ok_push_inv ; applys* ok_concat_inv_l G2).
+          rewrite~ (env_Tbsubst_fresh G1 T (FTName T')). }
+        { Case "TyAll". apply_fresh KAll as X.
+          + apply ok_kind_Tsubst...
+          + replaces (BindTVar (Tsubst_k T (FTName T') k))
+              with (Tbsubst T (FTName T') (BindTVar k))...
+            rewrite <- Tsubst_ty_topen_comm. apply_ih_map_bind H1 ; auto.
+            constructor~. apply~ ok_kind_Tsubst... }
+        { Case "TyCon".
+          asserts (S, Heq): (lcT (Tsubst T (FTName T') (FTName T0))). solve_var.
+          simpls. rewrite Heq. apply KCon with (d := Tsubst_d T (FTName T') d) (Ks := Ks)...
+          rewrite <- Heq. applys~ assoc_Tsubst. }
+        { Case "TyData". constructor~. apply~ ok_data_Tsubst... }
+      Qed.
+
+      Lemma Tbsubst_ok_env :
+        forall G1 G2 T T',
+          ok_env (G1 & T ~ BindTName & G2) ->
+          T' # G1 & T ~ BindTName & G2 ->
+          ok_env (G1 & T' ~ BindTName & map (Tbsubst T (FTName T')) G2).
+      Proof with eauto using ok_data_Tsubst, ok_kind_Tsubst, ok_type_Tsubst with mcore.
+        introv Henv Hfresh. assert (Henv1 : ok_env G1)
+          by (applys ok_env_concat; applys* ok_env_concat).
+        induction G2 using env_ind.
+        { Case "Empty". autorewrite with rew_env_map rew_env_concat in *.
+          constructor~. }
+        { Case "Push". autorewrite with rew_env_map rew_env_concat in *.
+          specializes IHG2 (ok_env_push _ _ _ Henv).
+          lets [? Hdisj] : ok_push_inv (ok_env_ok _ Henv).
+          assert (ok_env (G1 & T ~ BindTName & G2)) by apply* ok_env_concat.
+          destruct v.
+          { SCase "BindTName". constructor~. }
+          { SCase "BindCon". forwards (L & T0 & Heq & Hd & Htk' & HT): ok_env_con_inv Henv.
+            substs. asserts (S, Heq): (lcT (Tsubst T (FTName T') (FTName T0))). solve_var.
+            simpls. rewrite Heq. apply_fresh EnvCon as X...
+            - replaces (BindTVar (KiData (Tsubst_d T (FTName T') d)))
+                with (Tbsubst T (FTName T') (BindTVar (KiData d))) ; auto.
+              replaces KiType with (Tsubst_k T (FTName T') KiType) ; auto.
+              rewrite <- Tsubst_ty_topen_comm.
+              apply_ih_map_bind ok_type_Tsubst ; try rewrite* concat_assoc ; auto.
+              constructor...
+            - solve_var ; inverts~ Heq. binds_cases HT ; auto.
+              apply~ binds_concat_left. apply* binds_concat_left_ok.
+              replaces BindTName with (Tbsubst T (FTName T') BindTName) ; eauto. }
+          { SCase "BindTVar". forwards Hk: ok_env_tvar_inv Henv. constructor... }
+          { SCase "BindVar". forwards Htk': ok_env_var_inv Henv. constructor~.
+            replaces KiType with (Tsubst_k T (FTName T') KiType)... }
+          (* { SCase "BindMatch". constructor~. } *)
+        }
+      Qed.
+
+      Lemma ok_term_Tsubst :
+        forall G2 G1 T T' t ty,
+          G1 & T ~ BindTName & G2 |= t ~: ty ->
+          T' # G1 & T ~ BindTName & G2 ->
+          G1 & T' ~ BindTName &
+            map (Tbsubst T (FTName T')) G2 |=
+                Tsubst_t T (FTName T') t ~: Tsubst_ty T (FTName T') ty.
+      Proof with eauto using Tbsubst_ok_env with mcore.
+        introv Htype. assert (Henv : ok_env G1)
+          by (applys ok_env_concat ; applys* ok_env_concat).
+        remember (G1 & T ~ BindTName & G2) as Gamma eqn:HGamma. gen G2.
+        induction Htype ; intros ; substs...
+        { Case "TmFVar". constructor...
+          replaces (BindVar (Tsubst_ty T (FTName T') ty))
+            with (Tbsubst T (FTName T') (BindVar ty))... binds_cases H0 ; auto.
+          apply~ binds_concat_left. apply* binds_concat_left_ok.
+          assert (T # G1) by (applys ok_push_inv ; applys* ok_concat_inv_l G2).
+          rewrite~ (env_Tbsubst_fresh G1 T (FTName T')). }
+        { Case "TmLam". apply_fresh TLam as x.
+          + replaces KiType with (Tsubst_k T (FTName T') KiType)...
+            apply ok_type_Tsubst...
+          + rewrite <- Tsubst_t_open_comm. folds (Tsubst_ty T (FTName T') ty1).
+            replaces (BindVar (Tsubst_ty T (FTName T') ty1))
+              with (Tbsubst T (FTName T') (BindVar ty1))...
+            apply_ih_map_bind H1 ; auto. }
+        { Case "TmTyLam". apply_fresh TTyLam as X.
+          + apply ok_kind_Tsubst...
+          + rewrite <- Tsubst_t_topen_comm. rewrite <- Tsubst_ty_topen_comm.
+            replaces (BindTVar (Tsubst_k T (FTName T') k))
+              with (Tbsubst T (FTName T') (BindTVar k))...
+            apply_ih_map_bind H1 ; auto. }
+        { Case "TmTyApp". rewrite Tsubst_ty_topen_distr. constructors*.
+          apply ok_type_Tsubst... }
+        { Case "TmCon".
+          asserts (S, Heq): (lcT (Tsubst T (FTName T') (FTName T0))). solve_var.
+          simpls. rewrite Heq.
+          apply TCon with (d := Tsubst_d T (FTName T') d) (ty1 := Tsubst_ty T (FTName T') ty1).
+          - replaces (BindCon (Tsubst_d T (FTName T') d) (Tsubst_ty T (FTName T') ty1) (FTName S))
+              with (Tbsubst T (FTName T') (BindCon d ty1 (FTName T0))). rewrite~ <- Heq.
+            binds_cases H ; auto.
+            apply~ binds_concat_left. apply* binds_concat_left_ok.
+            assert (T # G1) by (applys ok_push_inv ; applys* ok_concat_inv_l G2).
+            rewrite~ (env_Tbsubst_fresh G1 T (FTName T')).
+          - replaces (KiData (Tsubst_d T (FTName T') d)) with (Tsubst_k T (FTName T') (KiData d))...
+            apply* ok_type_Tsubst.
+          - replaces (KiData [(FTName S, FCon K :: [])])
+              with (Tsubst_k T (FTName T') (KiData [(FTName T0, FCon K :: [])])). rewrite~ <- Heq.
+            apply* ok_type_Tsubst.
+          - rewrite <- Tsubst_ty_topen_distr... }
+        { Case "TmType". apply_fresh TType as T0.
+          replaces BindTName with (Tbsubst T (FTName T') BindTName)...
+          rewrite~ Tsubst_t_Topen_comm. apply_ih_map_bind H0 ; auto. }
+        { Case "TmConDef".
+          asserts (S, Heq): (lcT (Tsubst T (FTName T') (FTName T0))). solve_var.
+          simpls. rewrite Heq. apply_fresh TConDef as X.
+          - apply ok_data_Tsubst...
+          - replaces KiType with (Tsubst_k T (FTName T') KiType)...
+            replaces (BindTVar (KiData (Tsubst_d T (FTName T') d)))
+              with (Tbsubst T (FTName T') (BindTVar (KiData d)))...
+            rewrite <- Tsubst_ty_topen_comm.
+            apply_ih_map_bind ok_type_Tsubst ; eauto ; try rewrite* concat_assoc.
+            constructor... apply ok_kind_Tsubst...
+          - solve_var ; inverts~ Heq.
+            binds_cases H1 ; auto.
+            apply~ binds_concat_left. apply binds_concat_left_ok...
+            replaces BindTName with (Tbsubst T (FTName T') BindTName)...
+          - replaces (BindCon (Tsubst_d T (FTName T') d) (Tsubst_ty T (FTName T') ty1) (FTName S))
+              with (Tbsubst T (FTName T') (BindCon d ty1 (FTName T0))). rewrite~ <- Heq.
+            rewrite Tsubst_t_Kopen_comm. apply_ih_map_bind H3 ; auto. }
+        { Case "TmSem". apply_fresh TSem as x.
+          + replaces KiType with (Tsubst_k T (FTName T') KiType)...
+            apply ok_type_Tsubst...
+          + apply ok_pat_Tsubst...
+          + rewrite <- Tsubst_t_open_comm.
+            replaces (BindVar (Tsubst_ty T (FTName T') ty1'))
+              with (Tbsubst T (FTName T') (BindVar ty1'))...
+            apply_ih_map_bind H2 ; auto. }
+        { Case "TmComp". constructor~. apply~ pats_compatible_Tsubst. }
+        { Case "TmSemApp". constructors*. apply~ pats_exhaustive_Tsubst. }
+      Qed.
+
+      Lemma ok_term_Topen_change :
+        forall T T' Gamma t ty,
+          T \notin Tfv_t t \u Tfv_ty ty ->
+          T' # Gamma & T ~ BindTName ->
+          Gamma & T ~ BindTName |= Topen_t 0 (FTName T) t ~: ty ->
+          Gamma & T' ~ BindTName |= Topen_t 0 (FTName T') t ~: ty.
+      Proof.
+        introv Hnin Hfresh Htype.
+        rewrite~ (Tsubst_t_intro T (FTName T')).
+        rewrite~ <- (Tsubst_ty_fresh T (FTName T')).
+        apply_empty~ ok_term_Tsubst.
+      Qed.
+
+
+      Lemma ok_data_con_strengthening :
+        forall K G2 G1 d' ty' T d,
+          K \notin Kfv_d d ->
+          ok_data (G1 & K ~ BindCon d' ty' T & G2) d ->
+          ok_data (G1 & G2) d.
+      Proof.
+        introv Hfv Hd. remember (G1 & K ~ BindCon d' ty' T & G2) as Gamma eqn:HGamma.
+        unfolds Kfv_d. induction Hd ; substs ; constructor ; rew_listx~ in Hfv.
+        - binds_cases H0 ; auto.
+        - induction* Ks. inverts H1. rew_listx~ in Hfv.
+          constructors~. binds_cases H8 ; eauto. notin_false.
+      Qed.
+
+      Lemma ok_kind_con_strengthening :
+        forall K G2 G1 d ty' T k,
+          K \notin Kfv_k k ->
+          ok_kind (G1 & K ~ BindCon d ty' T & G2) k ->
+          ok_kind (G1 & G2) k.
+      Proof with eauto using ok_data_con_strengthening with mcore.
+        introv Hfv Hk.
+        remember (G1 & K ~ BindCon d ty' T & G2) as Gamma eqn:HGamma.
+        induction Hk ; substs...
+      Qed.
+
+      Lemma ok_type_con_strengthening :
+        forall K G2 G1 d ty' T ty k,
+          K \notin Kfv_ty ty ->
+          G1 & K ~ BindCon d ty' T & G2 |= ty ~:: k ->
+          ok_env (G1 & G2) ->
+          G1 & G2 |= ty ~:: k.
+      Proof with eauto using ok_data_con_strengthening, ok_kind_con_strengthening with mcore.
+        introv Hfv Htk Henv.
+        remember (G1 & K ~ BindCon d ty' T & G2) as Gamma eqn:HGamma. gen G2.
+        induction Htk ; intros ; simpls ; substs...
+        { Case "TyFVar". constructor~. binds_cases H0 ; auto. }
+        { Case "TyAll". rewrite notin_union in Hfv ; destruct Hfv.
+          apply_fresh KAll as X...
+          apply_ih_bind H1 ; auto. rewrite topen_notin_K ; simpls~. constructors... }
+      Qed.
+
+      Lemma ok_data_notin_K :
+        forall Gamma d X,
+          ok_data Gamma d ->
+          X # Gamma ->
+          X \notin Kfv_d d.
+      Proof.
+        introv Hd Hfresh. unfolds Kfv_d.
+        induction Hd ; rew_listx~.
+        rewrite notin_union. splits*.
+        induction H1 ; rew_listx~ ; rewrite notin_union ; splits~.
+        - rewrite notin_singleton. intro. substs.
+          forwards~ Hin : get_some_inv H3.
+      Qed.
+
+      Lemma ok_kind_notin_K :
+        forall Gamma k X,
+          ok_kind Gamma k ->
+          X # Gamma ->
+          X \notin Kfv_k k.
+      Proof.
+        introv Hk Hfresh. unfolds Kfv_k.
+        destruct~ Hk. apply* ok_data_notin_K.
+      Qed.
+
+      Lemma ok_type_notin_K :
+        forall Gamma T k X,
+          Gamma |= T ~:: k ->
+          X # Gamma ->
+          X \notin Kfv_ty T.
+      Proof with eauto using ok_data_notin_K, ok_kind_notin_K.
+        introv Htk Hfresh.
+        induction Htk; simpls...
+        { Case "TyAll". rewrite notin_union. splits...
+          pick_fresh Y. forwards~ Htk: H1 Y.
+          rewrite topen_notin_K in Htk ; simpls~. }
+      Qed.
+
+      Lemma env_Kbsubst_fresh :
+        forall Gamma X K,
+          ok_env Gamma ->
+          X # Gamma ->
+          Gamma = map (Kbsubst X K) Gamma.
+      Proof with eauto using ok_env_push.
+        introv Henv Hfresh.
+        induction Gamma using env_ind.
+        { Case "Empty". rewrite~ map_empty. }
+        { Case "Push". autorewrite with rew_env_map.
+          rewrite <- IHGamma...
+          destruct~ v ; repeat fequals ; unfold Kbsubst.
+          { SCase "BindCon".
+            apply ok_env_con_inv in Henv as (? & ? & ? & ? & Htk & ?). fequals.
+            - rewrite~ Ksubst_d_fresh. forwards~ Hnin : ok_data_notin_K X H0.
+            - rewrite~ Ksubst_ty_fresh. pick_fresh X'.
+              forwards~ Hnin : ok_type_notin_K X (Htk X').
+              rewrite topen_notin_K in Hnin ; simpls~. }
+          { SCase "BindTVar".
+            apply ok_env_tvar_inv in Henv. fequals.
+            rewrite~ Ksubst_k_fresh. apply* ok_kind_notin_K. }
+          { SCase "BindVar".
+            apply ok_env_var_inv in Henv. fequals.
+            rewrite~ Ksubst_ty_fresh. apply* ok_type_notin_K. } }
+      Qed.
+
+      Lemma assoc_Ksubst :
+        forall K K' S Ks d,
+          mem (FTName S, Ks) d ->
+          mem (FTName S, LibList.map (Ksubst K (FCon K')) Ks) (Ksubst_d K (FCon K') d).
+      Proof.
+        introv Hassoc. unfolds Ksubst_d.
+        induction Hassoc ; rew_listx~.
+      Qed.
+
+      Lemma assoc_Ksubst_inv :
+        forall K K' S Ks d,
+          mem (FTName S, Ks) (Ksubst_d K (FCon K') d) ->
+          exists Ks', LibList.mem (FTName S, Ks') d.
+      Proof.
+        introv Hassoc. unfolds Ksubst_d.
+        induction d ; inverts Hassoc ; destruct a ; rew_listx in *.
+        - inverts H0. exists~.
+        - inverts H. destruct~ IHd as (Ks'&?). exists~ Ks'.
+      Qed.
+
+      Lemma mem_Ksubst_inv :
+        forall Gamma K K' S Ks T,
+          ok_cons Gamma Ks T ->
+          K' # Gamma ->
+          K' <> S ->
+          mem (Ksubst K (FCon K') (FCon S)) (LibList.map (Ksubst K (FCon K')) Ks) ->
+          mem (FCon S) Ks.
+      Proof.
+        introv HKs Hfresh Hneq Hmem.
+        induction HKs ; inverts Hmem ; rew_listx~ in *.
+        left. fequals.
+        rewrite~ (Ksubst_inj S K0 K K'). intro Heq ; substs.
+        forwards Hin : get_some_inv H0 ; eauto.
+      Qed.
+
+      Lemma ok_data_Ksubst :
+        forall G2 G1 K K' d' ty' T d,
+          ok_data (G1 & K ~ BindCon d' ty' T & G2) d ->
+          K' # G1 & K ~ BindCon d' ty' T & G2 ->
+          ok_env (G1 & K ~ BindCon d' ty' T & G2) ->
+          ok_data (G1 & K' ~ BindCon d' ty' T & map (Kbsubst K (FCon K')) G2)
+                  (Ksubst_d K (FCon K') d).
+      Proof with eauto with mcore.
+        introv Hd Hfresh Henv. assert (Henv' : ok_env G1)
+          by (applys ok_env_concat ; applys* ok_env_concat).
+        remember (G1 & K ~ BindCon d' ty' T & G2). unfolds Ksubst_d.
+        induction Hd; substs; rew_listx*. constructor~.
+        - introv contra. forwards* (Ks'&Hassoc): assoc_Ksubst_inv.
+        - binds_cases H0 ; auto.
+          apply~ binds_concat_left. apply binds_concat_left_ok...
+          replaces BindTName with (Kbsubst K (FCon K') BindTName)...
+        - remember (G1 & K ~ BindCon d' ty' T & G2).
+          induction H1 ; substs.
+          + constructor.
+          + asserts (S, Heq): (lcK (Ksubst K (FCon K') (FCon K0))). solve_var.
+            rew_listx. rewrite Heq.
+            apply CCons with (d := Ksubst_d K (FCon K') d0)
+                             (ty := Ksubst_ty K (FCon K') ty) ; auto.
+            * rewrite <- Heq. intro contra.
+              apply H2. applys* mem_Ksubst_inv contra. intro ; subst.
+              forwards~ ?: get_some_inv H3.
+            * assert (K # G1) by (applys ok_push_inv ; applys* ok_concat_inv_l G2).
+              solve_var ; inverts Heq.
+              ** forwards* Heqbind : binds_middle_eq_inv H3. inverts Heqbind.
+                 forwards (?&?&?&Hd'&Htk&?): ok_env_con_inv G1 K0 d' ty' T. applys~ ok_env_concat G2.
+                 pick_fresh X. forwards~ Hnin: ok_type_notin_K K0 (Htk X).
+                 rewrite topen_notin_K in Hnin ; simpls~. forwards~ Hnin': ok_data_notin_K K0 Hd'.
+                 rewrite~ Ksubst_d_fresh. rewrite~ Ksubst_ty_fresh.
+              ** replaces (BindCon (Ksubst_d K (FCon K') d0) (Ksubst_ty K (FCon K') ty) T1)
+                   with (Kbsubst K (FCon K') (BindCon d0 ty T1))...
+                 binds_cases H3 ; auto.
+                 apply~ binds_concat_left. apply binds_concat_left_ok...
+                 rewrite~ (env_Kbsubst_fresh G1 K (FCon K'))...
+      Qed.
+
+      Lemma ok_kind_Ksubst :
+        forall G2 G1 K K' d ty' T k,
+          ok_kind (G1 & K ~ BindCon d ty' T & G2) k ->
+          ok_env  (G1 & K ~ BindCon d ty' T & G2) ->
+          K' # G1 & K ~ BindCon d ty' T & G2 ->
+          ok_kind (G1 & K' ~ BindCon d ty' T & map (Kbsubst K (FCon K')) G2)
+                  (Ksubst_k K (FCon K') k).
+      Proof.
+        introv Hk. remember (G1 & K ~ BindCon d ty' T & G2) as G.
+        induction Hk; intros; substs; constructor.
+        apply~ ok_data_Ksubst.
+      Qed.
+
+      Lemma ok_type_Ksubst :
+        forall G2 G1 K K' d ty' T ty k,
+          G1 & K ~ BindCon d ty' T & G2 |= ty ~:: k ->
+          ok_env (G1 & K' ~ BindCon d ty' T & map (Kbsubst K (FCon K')) G2) ->
+          K' # G1 & K ~ BindCon d ty' T & G2 ->
+          G1 & K' ~ BindCon d ty' T &
+            map (Kbsubst K (FCon K')) G2 |=
+                Ksubst_ty K (FCon K') ty ~:: Ksubst_k K (FCon K') k.
+      Proof with eauto with mcore.
+        introv Htk Hfresh Henv. assert (Henv' : ok_env G1)
+          by (applys ok_env_concat ; applys* ok_env_concat).
+        remember (G1 & K ~ BindCon d ty' T & G2). gen G2.
+        induction Htk; intros; substs; simpls...
+        { Case "TyFVar". constructor...
+          replaces (BindTVar (Ksubst_k K (FCon K') k))
+            with (Kbsubst K (FCon K') (BindTVar k))... binds_cases H0 ; auto.
+          apply~ binds_concat_left. apply* binds_concat_left_ok.
+          assert (K # G1) by (applys ok_push_inv ; applys* ok_concat_inv_l G2).
+          rewrite~ (env_Kbsubst_fresh G1 K (FCon K')). }
+        { Case "TyAll". apply_fresh KAll as X.
+          + apply ok_kind_Ksubst...
+          + replaces (BindTVar (Ksubst_k K (FCon K') k))
+              with (Kbsubst K (FCon K') (BindTVar k))...
+            rewrite <- Ksubst_ty_topen_comm. apply_ih_map_bind H1 ; auto.
+            constructor... apply ok_kind_Ksubst... }
+        { Case "TyCon".
+          apply KCon with (d := Ksubst_d K (FCon K') d0) (Ks := LibList.map (Ksubst K (FCon K')) Ks)...
+          apply~ assoc_Ksubst. }
+        { Case "TyData". constructor~. apply~ ok_data_Ksubst. }
+      Qed.
+
+      Lemma Kbsubst_ok_env :
+        forall G1 G2 K K' d ty T,
+          ok_env (G1 & K ~ BindCon d ty T & G2) ->
+          K' # G1 & K ~ BindCon d ty T & G2 ->
+          ok_env (G1 & K' ~ BindCon d ty T & map (Kbsubst K (FCon K')) G2).
+      Proof with eauto using ok_data_Ksubst, ok_kind_Ksubst, ok_type_Ksubst with mcore.
+        introv Henv Hfresh. assert (Henv1 : ok_env G1)
+          by (applys ok_env_concat; applys* ok_env_concat).
+        forwards Henv': ok_env_concat Henv. forwards (?&?&?&?&?&?): ok_env_con_inv Henv'.
+        substs. induction G2 using env_ind.
+        { Case "Empty". autorewrite with rew_env_map rew_env_concat in *.
+          apply_fresh EnvCon... }
+        { Case "Push". autorewrite with rew_env_map rew_env_concat in *.
+          specializes IHG2 (ok_env_push _ _ _ Henv) ; auto.
+          lets [? Hdisj] : ok_push_inv (ok_env_ok _ Henv).
+          assert (ok_env (G1 & K ~ BindCon d ty (FTName x0) & G2)) by apply* ok_env_concat.
+          destruct v.
+          { SCase "BindTName". constructor~. }
+          { SCase "BindCon". forwards (L & T0 & Heq & Hd & Htk' & HT): ok_env_con_inv Henv.
+            substs. apply_fresh EnvCon as X...
+            - replaces (BindTVar (KiData (Ksubst_d K (FCon K') d0)))
+                with (Kbsubst K (FCon K') (BindTVar (KiData d0))) ; auto.
+              replaces KiType with (Ksubst_k K (FCon K') KiType) ; auto.
+              rewrite <- Ksubst_ty_topen_comm.
+              apply_ih_map_bind ok_type_Ksubst ; try rewrite* concat_assoc ; auto.
+              constructor...
+            - binds_cases HT ; auto.
+              apply~ binds_concat_left. apply* binds_concat_left_ok.
+              replaces BindTName with (Kbsubst K (FCon K') BindTName) ; eauto. }
+          { SCase "BindTVar". forwards Hk: ok_env_tvar_inv Henv. constructor... }
+          { SCase "BindVar". forwards Htk': ok_env_var_inv Henv. constructor~.
+            replaces KiType with (Ksubst_k K (FCon K') KiType)... }
+          (* { SCase "BindMatch". constructor~. } *)
+        }
+      Qed.
+
+      Lemma ok_term_Ksubst :
+        forall G2 G1 K K' d ty' T t ty,
+          G1 & K ~ BindCon d ty' T & G2 |= t ~: ty ->
+          K' # G1 & K ~ BindCon d ty' T & G2 ->
+          G1 & K' ~ BindCon d ty' T &
+            map (Kbsubst K (FCon K')) G2 |=
+                Ksubst_t K (FCon K') t ~: Ksubst_ty K (FCon K') ty.
+      Proof with eauto using Kbsubst_ok_env with mcore.
+        introv Htype. assert (Henv : ok_env G1)
+          by (applys ok_env_concat ; applys* ok_env_concat).
+        remember (G1 & K ~ BindCon d ty' T & G2). gen G2.
+        induction Htype ; intros ; substs...
+        { Case "TmFVar". constructor...
+          replaces (BindVar (Ksubst_ty K (FCon K') ty))
+            with (Kbsubst K (FCon K') (BindVar ty))... binds_cases H0 ; auto.
+          apply~ binds_concat_left. apply* binds_concat_left_ok.
+          assert (K # G1) by (applys ok_push_inv ; applys* ok_concat_inv_l G2).
+          rewrite~ (env_Kbsubst_fresh G1 K (FCon K')). }
+        { Case "TmLam". apply_fresh TLam as x.
+          + replaces KiType with (Ksubst_k K (FCon K') KiType)...
+            apply ok_type_Ksubst...
+          + rewrite <- Ksubst_t_open_comm. folds (Ksubst_ty K (FCon K') ty1).
+            replaces (BindVar (Ksubst_ty K (FCon K') ty1))
+              with (Kbsubst K (FCon K') (BindVar ty1))...
+            apply_ih_map_bind H1 ; auto. }
+        { Case "TmTyLam". apply_fresh TTyLam as X.
+          + apply ok_kind_Ksubst...
+          + rewrite <- Ksubst_t_topen_comm. rewrite <- Ksubst_ty_topen_comm.
+            replaces (BindTVar (Ksubst_k K (FCon K') k))
+              with (Kbsubst K (FCon K') (BindTVar k))...
+            apply_ih_map_bind H1 ; auto. }
+        { Case "TmTyApp". rewrite Ksubst_ty_topen_distr. constructors*.
+          apply ok_type_Ksubst... }
+        { Case "TmCon".
+          asserts (S, Heq): (lcK (Ksubst K (FCon K') (FCon K0))). solve_var.
+          simpls. rewrite Heq.
+          apply TCon with (d := Ksubst_d K (FCon K') d0) (ty1 := Ksubst_ty K (FCon K') ty1).
+          - assert (K # G1) by (applys ok_push_inv ; applys* ok_concat_inv_l G2).
+            solve_var ; inverts Heq.
+            + forwards* Heqbind : binds_middle_eq_inv H. inverts Heqbind.
+              forwards (?&?&?&Hd&Htk&?): ok_env_con_inv G1 S d ty'. apply* ok_env_concat.
+              pick_fresh X. forwards~ Hnin: ok_type_notin_K K0 (Htk X).
+              rewrite topen_notin_K in Hnin ; simpls~. forwards~ Hnin': ok_data_notin_K K0 Hd.
+              rewrite~ Ksubst_d_fresh. rewrite~ Ksubst_ty_fresh.
+            + replaces (BindCon (Ksubst_d K (FCon K') d0) (Ksubst_ty K (FCon K') ty1) (FTName T0))
+                with (Kbsubst K (FCon K') (BindCon d0 ty1 (FTName T0)))...
+              binds_cases H ; auto.
+              apply~ binds_concat_left. apply* binds_concat_left_ok.
+              rewrite~ (env_Kbsubst_fresh G1 K (FCon K')).
+          - replaces (KiData (Ksubst_d K (FCon K') d0)) with (Ksubst_k K (FCon K') (KiData d0))...
+            apply* ok_type_Ksubst.
+          - replaces (KiData [(FTName T0, FCon S :: [])])
+              with (Ksubst_k K (FCon K') (KiData [(FTName T0, FCon K0 :: [])])). rewrite~ <- Heq.
+            apply* ok_type_Ksubst.
+          - rewrite <- Ksubst_ty_topen_distr... }
+        { Case "TmType". apply_fresh TType as T0.
+          replaces BindTName with (Kbsubst K (FCon K') BindTName)...
+          rewrite~ Ksubst_t_Topen_comm. apply_ih_map_bind H0 ; auto. }
+        { Case "TmConDef". apply_fresh TConDef as X.
+          - apply~ ok_data_Ksubst...
+          - replaces KiType with (Ksubst_k K (FCon K') KiType)...
+            replaces (BindTVar (KiData (Ksubst_d K (FCon K') d0)))
+              with (Kbsubst K (FCon K') (BindTVar (KiData d0)))...
+            rewrite <- Ksubst_ty_topen_comm.
+            apply_ih_map_bind ok_type_Ksubst ; eauto ; try rewrite* concat_assoc.
+            constructor... apply ok_kind_Ksubst...
+          - binds_cases H1 ; auto.
+            apply~ binds_concat_left. apply binds_concat_left_ok...
+            replaces BindTName with (Kbsubst K (FCon K') BindTName)...
+          - replaces (BindCon (Ksubst_d K (FCon K') d0) (Ksubst_ty K (FCon K') ty1) (FTName T0))
+              with (Kbsubst K (FCon K') (BindCon d0 ty1 (FTName T0)))...
+            rewrite~ Ksubst_t_Kopen_comm. apply_ih_map_bind H3 ; auto. }
+        { Case "TmSem". apply_fresh TSem as x.
+          + replaces KiType with (Ksubst_k K (FCon K') KiType)...
+            apply ok_type_Ksubst...
+          + apply ok_pat_Ksubst...
+          + rewrite <- Ksubst_t_open_comm.
+            replaces (BindVar (Ksubst_ty K (FCon K') ty1'))
+              with (Kbsubst K (FCon K') (BindVar ty1'))...
+            apply_ih_map_bind H2 ; auto. }
+        { Case "TmComp". constructor~. apply~ pats_compatible_Ksubst. }
+        { Case "TmSemApp". constructors*. apply~ pats_exhaustive_Ksubst. }
+      Qed.
+
+      Lemma ok_term_Kopen_change :
+        forall K K' d ty' T Gamma t ty,
+          K \notin Kfv_t t \u Kfv_ty ty ->
+          K' # Gamma & K ~ BindCon d ty' T ->
+          Gamma & K ~ BindCon d ty' T |= Kopen_t 0 (FCon K) t ~: ty ->
+          Gamma & K' ~ BindCon d ty' T |= Kopen_t 0 (FCon K') t ~: ty.
+      Proof.
+        introv Hnin Hfresh Htype.
+        rewrite~ (Ksubst_t_intro K (FCon K')).
+        rewrite~ <- (Ksubst_ty_fresh K (FCon K')).
+        apply_empty~ ok_term_Ksubst.
+      Qed.
+
+    End TypingProps2.
+  End TypingProps1.
+End TypingProps.
